proof/uni/decl/prop_safety.v
@@ -2,6 +2,7 @@ Require Import Coq.Program.Equality.
 
 Require Import systemf.def_ott.
 Require Import systemf.prop_ln.
+Require Import systemf.prop_basic.
 
 Require Import uni.def_ott.
 Require Import uni.decl.def_extra.
@@ -12,22 +13,6 @@ Require Import uni.notations.
 Require Import uni.ltac_utils.
 
 Open Scope dbind.
-
-Lemma open_fexp_wrt_fexp_rec_lc_fexp : forall e2 e1 n,
-  lc_fexp e2 -> open_fexp_wrt_fexp_rec n e1 e2 = e2.
-Proof.
-  intros. apply open_fexp_wrt_fexp_rec_degree_fexp_wrt_fexp.
-  apply degree_fexp_wrt_fexp_O.
-  apply degree_fexp_wrt_fexp_of_lc_fexp. auto.
-Qed.
-
-Lemma open_fexp_wrt_ftyp_rec_lc_fexp : forall e T n,
-  lc_fexp e -> open_fexp_wrt_ftyp_rec n T e = e.
-Proof.
-  intros. apply open_fexp_wrt_ftyp_rec_degree_fexp_wrt_ftyp.
-  apply degree_fexp_wrt_ftyp_O.
-  apply degree_fexp_wrt_ftyp_of_lc_fexp. auto.
-Qed.
 
 Notation "Ψ ⊢ e : A" :=
   (f_typing Ψ e A) 
@@ -56,7 +41,7 @@ Fixpoint trans_env (Ψ : denv) : fenv :=
   | (X, (dbind_typ T)) :: Ψ' => (X, (fbind_typ (trans_typ T))) :: trans_env Ψ'
   end.
 
-Notation "ᵉ⟦ Ψ ⟧" := (trans_env Ψ) (at level 0, no associativity) : type_scope.
+Notation "⟦ Ψ ⟧" := (trans_env Ψ) (at level 0, no associativity) : type_scope.
 
 Lemma trans_typ_open_typ_wrt_typ_rec : forall A1 A2 n,
   trans_typ (open_typ_wrt_typ_rec n A2 A1) = open_ftyp_wrt_ftyp_rec n ᵗ⟦ A2 ⟧ ᵗ⟦ A1 ⟧.
@@ -90,7 +75,7 @@ Qed.
 #[local] Hint Resolve trans_typ_lc_ftyp : core.
 
 Theorem trans_env_notin_dom : forall Ψ X,
-  X `notin` dom Ψ -> X `notin` dom (trans_env Ψ).
+  X `notin` dom Ψ -> X `notin` dom ⟦ Ψ ⟧.
 Proof.
   intros Ψ. induction Ψ; auto.
   intros X H. destruct a. destruct d; simpl in *; auto.
@@ -129,7 +114,7 @@ Proof.
 Qed.
 
 Theorem trans_env_wf_tenv_wf_fenv : forall Ψ,
-  ⊢ᵈₜ Ψ -> f_wf_env ᵉ⟦ Ψ ⟧.
+  ⊢ᵈₜ Ψ -> f_wf_env ⟦ Ψ ⟧.
 Proof with eauto using trans_typ_wf.
   intros. induction H; simpl; eauto...
   constructor...
@@ -137,7 +122,7 @@ Proof with eauto using trans_typ_wf.
 Qed.
 
 Theorem trans_env_wf_env_wf_fenv : forall Ψ,
-  ⊢ᵈ Ψ -> f_wf_env ᵉ⟦ Ψ ⟧.
+  ⊢ᵈ Ψ -> f_wf_env ⟦ Ψ ⟧.
 Proof with eauto using trans_env_wf_tenv_wf_fenv.
   intros. induction H; simpl; eauto;
   try solve [apply trans_env_notin_dom in H0; apply wf_env_sub; auto]...
@@ -161,64 +146,64 @@ Inductive d_sub_elab : denv -> typ -> typ -> fexp -> Prop :=
       d_wf_env Ψ ->
       d_wf_typ Ψ (typ_var_f X) ->
       d_sub_elab Ψ (typ_var_f X) (typ_var_f X) (fexp_abs (ftyp_var_f X) (fexp_var_b 0))
-  | d_sub_elab__arrow : forall (Ψ:denv) (A1 A2 B1 B2:typ) (co1 co2:fexp),
-      d_sub_elab Ψ B1 A1 co1 ->
-      d_sub_elab Ψ A2 B2 co2 ->
+  | d_sub_elab__arrow : forall (Ψ:denv) (A1 A2 B1 B2:typ) (co1ᶠ co2ᶠ:fexp),
+      d_sub_elab Ψ B1 A1 co1ᶠ ->
+      d_sub_elab Ψ A2 B2 co2ᶠ ->
       d_sub_elab Ψ (typ_arrow A1 A2) (typ_arrow B1 B2)
         (fexp_abs (ftyp_arrow (trans_typ A1) (trans_typ A2))
                   (fexp_abs (trans_typ B1)
-                            (fexp_app co2
+                            (fexp_app co2ᶠ
                                       (fexp_app (fexp_var_b 1)
-                                                (fexp_app co1 (fexp_var_b 0))))))
-  | d_sub_elab__all : forall (L:vars) (Ψ:denv) (A B:typ) (co:fexp),
+                                                (fexp_app co1ᶠ (fexp_var_b 0))))))
+  | d_sub_elab__all : forall (L:vars) (Ψ:denv) (A B:typ) (coᶠ:fexp),
       ( forall X , X \notin L -> s_in X  (open_typ_wrt_typ  A   (typ_var_f X) ) ) ->
       ( forall X , X \notin L -> s_in X  (open_typ_wrt_typ  B   (typ_var_f X) ) ) ->
-      ( forall X , X \notin L -> d_sub_elab  ( X ~ dbind_stvar_empty  ++  Ψ )   (open_typ_wrt_typ  A   (typ_var_f X) )   (open_typ_wrt_typ  B   (typ_var_f X) ) (open_fexp_wrt_ftyp co (ftyp_var_f X)) ) ->
+      ( forall X , X \notin L -> d_sub_elab  ( X ~ dbind_stvar_empty  ++  Ψ )   (open_typ_wrt_typ  A   (typ_var_f X) )   (open_typ_wrt_typ  B   (typ_var_f X) ) (open_fexp_wrt_ftyp coᶠ (ftyp_var_f X)) ) ->
       d_sub_elab Ψ (typ_all A) (typ_all B)
-        (fexp_abs (trans_typ (typ_all A)) (fexp_tabs (fexp_app (open_fexp_wrt_ftyp co (ftyp_var_b 0)) (fexp_tapp (fexp_var_b 0) (ftyp_var_b 0)))))
-  | d_sub_elab__alll : forall (L:vars) (Ψ:denv) (A B T:typ) (co:fexp),
+        (fexp_abs (trans_typ (typ_all A)) (fexp_tabs (fexp_app coᶠ (fexp_tapp (fexp_var_b 0) (ftyp_var_b 0)))))
+  | d_sub_elab__alll : forall (L:vars) (Ψ:denv) (A B T:typ) (coᶠ:fexp),
       neq_all B ->
       neq_intersection B ->
       neq_union B -> 
       ( forall X , X \notin L -> s_in X  (open_typ_wrt_typ  A   (typ_var_f X) ) ) ->
       d_mono_typ Ψ T ->
-      d_sub_elab Ψ  (open_typ_wrt_typ  A   T )  B co ->
+      d_sub_elab Ψ  (open_typ_wrt_typ  A   T )  B coᶠ ->
       d_sub_elab Ψ (typ_all A) B
-        (fexp_abs (trans_typ (typ_all A)) (fexp_app co (fexp_tapp (fexp_var_b 0) (trans_typ T))))
-  | d_sub_elab__intersection1 : forall (Ψ:denv) (A B1 B2:typ) (co1 co2:fexp),
-      d_sub_elab Ψ A B1 co1 ->
-      d_sub_elab Ψ A B2 co2 ->
+        (fexp_abs (trans_typ (typ_all A)) (fexp_app coᶠ (fexp_tapp (fexp_var_b 0) (trans_typ T))))
+  | d_sub_elab__intersection1 : forall (Ψ:denv) (A B1 B2:typ) (co1ᶠ co2ᶠ:fexp),
+      d_sub_elab Ψ A B1 co1ᶠ ->
+      d_sub_elab Ψ A B2 co2ᶠ ->
       d_sub_elab Ψ A (typ_intersection B1 B2)
         (fexp_abs (trans_typ A)
-                  (fexp_pair (fexp_app co1 (fexp_var_b 0))
-                          (fexp_app co2 (fexp_var_b 0))))
-  | d_sub_elab__intersection2 : forall (Ψ:denv) (A1 A2 B:typ) (co:fexp),
-      d_sub_elab Ψ A1 B co ->
+                  (fexp_pair (fexp_app co1ᶠ (fexp_var_b 0))
+                          (fexp_app co2ᶠ (fexp_var_b 0))))
+  | d_sub_elab__intersection2 : forall (Ψ:denv) (A1 A2 B:typ) (coᶠ:fexp),
+      d_sub_elab Ψ A1 B coᶠ ->
       d_wf_typ Ψ A2 ->
       d_sub_elab Ψ (typ_intersection A1 A2) B
-        (fexp_abs (trans_typ (typ_intersection A1 A2)) (fexp_app co (fexp_proj1 (fexp_var_b 0))))
-  | d_sub_elab__intersection3 : forall (Ψ:denv) (A1 A2 B:typ) (co:fexp),
-      d_sub_elab Ψ A2 B co ->
+        (fexp_abs (trans_typ (typ_intersection A1 A2)) (fexp_app coᶠ (fexp_proj1 (fexp_var_b 0))))
+  | d_sub_elab__intersection3 : forall (Ψ:denv) (A1 A2 B:typ) (coᶠ:fexp),
+      d_sub_elab Ψ A2 B coᶠ ->
       d_wf_typ Ψ A1 ->
       d_sub_elab Ψ (typ_intersection A1 A2) B
-        (fexp_abs (trans_typ (typ_intersection A1 A2)) (fexp_app co (fexp_proj2 (fexp_var_b 0))))
-  | d_sub_elab__union1 : forall (Ψ:denv) (A B1 B2:typ) (co:fexp),
-      d_sub_elab Ψ A B1 co ->
+        (fexp_abs (trans_typ (typ_intersection A1 A2)) (fexp_app coᶠ (fexp_proj2 (fexp_var_b 0))))
+  | d_sub_elab__union1 : forall (Ψ:denv) (A B1 B2:typ) (coᶠ:fexp),
+      d_sub_elab Ψ A B1 coᶠ ->
       d_wf_typ Ψ B2 ->
       d_sub_elab Ψ A (typ_union B1 B2)
-        (fexp_abs (trans_typ A) (fexp_inl (fexp_app co (fexp_var_b 0))))
-  | d_sub_elab__union2 : forall (Ψ:denv) (A B1 B2:typ) (co:fexp),
-      d_sub_elab Ψ A B2 co ->
+        (fexp_abs (trans_typ A) (fexp_inl (fexp_app coᶠ (fexp_var_b 0))))
+  | d_sub_elab__union2 : forall (Ψ:denv) (A B1 B2:typ) (coᶠ:fexp),
+      d_sub_elab Ψ A B2 coᶠ ->
       d_wf_typ Ψ B1 ->
       d_sub_elab Ψ A (typ_union B1 B2)
-        (fexp_abs (trans_typ A) (fexp_inr (fexp_app co (fexp_var_b 0))))
-  | d_sub_elab__union3 : forall (Ψ:denv) (A1 A2 B:typ) (co1 co2:fexp),
-      d_sub_elab Ψ A1 B co1 ->
-      d_sub_elab Ψ A2 B co2 ->
+        (fexp_abs (trans_typ A) (fexp_inr (fexp_app coᶠ (fexp_var_b 0))))
+  | d_sub_elab__union3 : forall (Ψ:denv) (A1 A2 B:typ) (co1ᶠ co2ᶠ:fexp),
+      d_sub_elab Ψ A1 B co1ᶠ ->
+      d_sub_elab Ψ A2 B co2ᶠ ->
       d_sub_elab Ψ (typ_union A1 A2) B
-        (fexp_abs (trans_typ (typ_union A1 A2)) (fexp_case (fexp_var_b 0) (fexp_app co1 (fexp_var_b 0)) (fexp_app co2 (fexp_var_b 0)))).
+        (fexp_abs (trans_typ (typ_union A1 A2)) (fexp_case (fexp_var_b 0) (fexp_app co1ᶠ (fexp_var_b 0)) (fexp_app co2ᶠ (fexp_var_b 0)))).
 
-Notation "Ψ ⊢ A <: B ↪ co" := (d_sub_elab Ψ A B co) (at level 65, A at next level, B at next level, no associativity) : type_scope.
+Notation "Ψ ⊢ A <: B ↪ coᶠ" := (d_sub_elab Ψ A B coᶠ) (at level 65, A at next level, B at next level, no associativity) : type_scope.
 
 Inductive d_infabs_elab : denv -> typ -> typ -> typ -> fexp -> Prop := 
   | infabs_elab_bot : forall (Ψ:denv),
@@ -232,36 +217,36 @@ Inductive d_infabs_elab : denv -> typ -> typ -> typ -> fexp -> Prop :=
       d_wf_typ Ψ B ->
       d_infabs_elab Ψ (typ_arrow A B) A B
         (fexp_abs (trans_typ (typ_arrow A B)) (fexp_var_b 0))
-  | infabs_elab_all : forall (Ψ:denv) (A B C T:typ) (co:fexp),
+  | infabs_elab_all : forall (Ψ:denv) (A B C T:typ) (coᶠ:fexp),
       d_mono_typ Ψ T -> 
       d_wf_typ Ψ (typ_all A) ->
-      d_infabs_elab Ψ  (open_typ_wrt_typ  A   T ) B C co ->
+      d_infabs_elab Ψ  (open_typ_wrt_typ  A   T ) B C coᶠ ->
       d_infabs_elab Ψ (typ_all A) B C
         (fexp_abs (trans_typ (typ_all A))
-                  (fexp_app co (fexp_tapp (fexp_var_b 0) (trans_typ T))))
-  | infabs_elab_intersection1 : forall (Ψ:denv) (A1 A2 B C:typ) (co:fexp),
+                  (fexp_app coᶠ (fexp_tapp (fexp_var_b 0) (trans_typ T))))
+  | infabs_elab_intersection1 : forall (Ψ:denv) (A1 A2 B C:typ) (coᶠ:fexp),
       d_wf_typ Ψ A2 ->
-      d_infabs_elab Ψ A1 B C co ->
+      d_infabs_elab Ψ A1 B C coᶠ ->
       d_infabs_elab Ψ (typ_intersection A1 A2) B C
         (fexp_abs (trans_typ (typ_intersection A1 A2))
-                  (fexp_app co (fexp_proj1 (fexp_var_b 0))))
-  | infabs_elab_intersection2 : forall (Ψ:denv) (A1 A2 B C:typ) (co:fexp),
+                  (fexp_app coᶠ (fexp_proj1 (fexp_var_b 0))))
+  | infabs_elab_intersection2 : forall (Ψ:denv) (A1 A2 B C:typ) (coᶠ:fexp),
       d_wf_typ Ψ A1 ->
-      d_infabs_elab Ψ A2 B C co ->
+      d_infabs_elab Ψ A2 B C coᶠ ->
       d_infabs_elab Ψ (typ_intersection A1 A2) B C
         (fexp_abs (trans_typ (typ_intersection A1 A2))
-                  (fexp_app co (fexp_proj2 (fexp_var_b 0))))
-  | infabs_elab_union : forall (Ψ:denv) (A1 A2 B1 C1 B2 C2:typ) (co1 co2:fexp),
-      d_infabs_elab Ψ A1 B1 C1 co1 ->
-      d_infabs_elab Ψ A2 B2 C2 co2 ->
+                  (fexp_app coᶠ (fexp_proj2 (fexp_var_b 0))))
+  | infabs_elab_union : forall (Ψ:denv) (A1 A2 B1 C1 B2 C2:typ) (co1ᶠ co2ᶠ:fexp),
+      d_infabs_elab Ψ A1 B1 C1 co1ᶠ ->
+      d_infabs_elab Ψ A2 B2 C2 co2ᶠ ->
       d_infabs_elab Ψ (typ_union A1 A2) (typ_intersection B1 B2) (typ_union C1 C2)
         (fexp_abs (trans_typ (typ_union A1 A2))
                   (fexp_abs (trans_typ (typ_intersection B1 B2))
                             (fexp_case (fexp_var_b 1)
-                                      (fexp_inl (fexp_app co1 (fexp_proj1 (fexp_var_b 1))))
-                                      (fexp_inr (fexp_app co2 (fexp_proj2 (fexp_var_b 1))))))).
+                                      (fexp_inl (fexp_app co1ᶠ (fexp_proj1 (fexp_var_b 1))))
+                                      (fexp_inr (fexp_app co2ᶠ (fexp_proj2 (fexp_var_b 1))))))).
 
-Notation "Ψ ⊢ A ▹ B → C ↪ co" :=   (d_infabs_elab Ψ A B C co) 
+Notation "Ψ ⊢ A ▹ B → C ↪ coᶠ" :=   (d_infabs_elab Ψ A B C coᶠ) 
   (at level 65, A at next level, B at next level, C at next level, no associativity) : type_scope.
                             
 Inductive d_inftapp_elab : denv -> typ -> typ -> typ -> fexp -> fexp -> Prop := 
@@ -278,40 +263,40 @@ Inductive d_inftapp_elab : denv -> typ -> typ -> typ -> fexp -> fexp -> Prop :=
       d_inftapp_elab Ψ (typ_all A) B (open_typ_wrt_typ  A   B )  
         (fexp_abs (trans_typ (typ_all A)) (fexp_var_b 0))
         (fexp_abs (trans_typ (typ_all A)) (fexp_tapp (fexp_var_b 0) (trans_typ B)))
-  | inftapp_elab_intersection1 : forall (Ψ:denv) (A1 A2 B C1:typ) (co1 co2:fexp),
+  | inftapp_elab_intersection1 : forall (Ψ:denv) (A1 A2 B C1:typ) (co1ᶠ co2ᶠ:fexp),
       d_wf_typ Ψ A2 ->
-      d_inftapp_elab Ψ A1 B C1 co1 co2 ->
+      d_inftapp_elab Ψ A1 B C1 co1ᶠ co2ᶠ ->
       d_inftapp_elab Ψ (typ_intersection A1 A2) B C1
         (fexp_abs (trans_typ (typ_intersection A1 A2))
-                  (fexp_app co1 (fexp_proj1 (fexp_var_b 0))))
-        co2
-  | inftapp_elab_intersection2 : forall (Ψ:denv) (A1 A2 B C2:typ) (co1 co2:fexp),
+                  (fexp_app co1ᶠ (fexp_proj1 (fexp_var_b 0))))
+        co2ᶠ
+  | inftapp_elab_intersection2 : forall (Ψ:denv) (A1 A2 B C2:typ) (co1ᶠ co2ᶠ:fexp),
       d_wf_typ Ψ A1 ->
-      d_inftapp_elab Ψ A2 B C2 co1 co2 ->
+      d_inftapp_elab Ψ A2 B C2 co1ᶠ co2ᶠ ->
       d_inftapp_elab Ψ (typ_intersection A1 A2) B C2
         (fexp_abs (trans_typ (typ_intersection A1 A2))
-                  (fexp_app co1 (fexp_proj2 (fexp_var_b 0))))
-        co2
-  | inftapp_elab_intersection3 : forall (Ψ:denv) (A1 A2 B C1 C2:typ) (co1 co2 co3 co4:fexp),
-      d_inftapp_elab Ψ A1 B C1 co1 co2 ->
+                  (fexp_app co1ᶠ (fexp_proj2 (fexp_var_b 0))))
+        co2ᶠ
+  | inftapp_elab_intersection3 : forall (Ψ:denv) (A1 A2 B C1 C2:typ) (co1ᶠ co2ᶠ co3 co4:fexp),
+      d_inftapp_elab Ψ A1 B C1 co1ᶠ co2ᶠ ->
       d_inftapp_elab Ψ A2 B C2 co3 co4 ->
       d_inftapp_elab Ψ (typ_intersection A1 A2) B (typ_intersection C1 C2)
         (fexp_abs (trans_typ (typ_intersection A1 A2))
-                  (fexp_pair (fexp_app co2 (fexp_app co1 (fexp_proj1 (fexp_var_b 0))))
+                  (fexp_pair (fexp_app co2ᶠ (fexp_app co1ᶠ (fexp_proj1 (fexp_var_b 0))))
                               (fexp_app co4 (fexp_app co3 (fexp_proj2 (fexp_var_b 0))))))
         (fexp_abs (trans_typ ((typ_intersection C1 C2))) (fexp_var_b 0))
-  | inftapp_elab_union : forall (Ψ:denv) (A1 A2 B C1 C2:typ) (co1 co2 co3 co4:fexp),
-      d_inftapp_elab Ψ A1 B C1 co1 co2 ->
+  | inftapp_elab_union : forall (Ψ:denv) (A1 A2 B C1 C2:typ) (co1ᶠ co2ᶠ co3 co4:fexp),
+      d_inftapp_elab Ψ A1 B C1 co1ᶠ co2ᶠ ->
       d_inftapp_elab Ψ A2 B C2 co3 co4 ->
       d_inftapp_elab Ψ (typ_union A1 A2) B (typ_union C1 C2)
         (fexp_abs (trans_typ (typ_union A1 A2))
                   (fexp_case (fexp_var_b 0)
-                              (fexp_inl (fexp_app co2 (fexp_app co1 (fexp_var_b 0))))
+                              (fexp_inl (fexp_app co2ᶠ (fexp_app co1ᶠ (fexp_var_b 0))))
                               (fexp_inr (fexp_app co4 (fexp_app co3 (fexp_var_b 0))))))
         (fexp_abs (trans_typ (typ_union C1 C2)) (fexp_var_b 0)).
 
-Notation "Ψ ⊢ A ○ B ⇒⇒ C ↪ co1 | co2" :=
-    (d_inftapp_elab Ψ A B C co1 co2) 
+Notation "Ψ ⊢ A ○ B ⇒⇒ C ↪ co1ᶠ | co2ᶠ" :=
+    (d_inftapp_elab Ψ A B C co1ᶠ co2ᶠ) 
       (at level 65, A at next level, B at next level, C at next level, no associativity) : type_scope. 
 
 
@@ -329,12 +314,12 @@ Inductive d_chk_inf_elab : denv -> exp -> typing_mode -> typ -> fexp -> Prop :=
       d_wf_env Ψ ->
       d_chk_inf_elab Ψ exp_unit typingmode__inf typ_unit
         fexp_unit
-  | d_chk_inf_elab__inf_app : forall (Ψ:denv) (e1 e2:exp) (A B C:typ) (e1ᶠ co e2ᶠ:fexp),
+  | d_chk_inf_elab__inf_app : forall (Ψ:denv) (e1 e2:exp) (A B C:typ) (e1ᶠ coᶠ e2ᶠ:fexp),
       d_chk_inf_elab Ψ e1 typingmode__inf A e1ᶠ ->
-      d_infabs_elab Ψ A B C co ->
+      d_infabs_elab Ψ A B C coᶠ ->
       d_chk_inf_elab Ψ e2 typingmode__chk B e2ᶠ ->
       d_chk_inf_elab Ψ  ( (exp_app e1 e2) ) typingmode__inf C
-        (fexp_app (fexp_app co e1ᶠ) e2ᶠ)
+        (fexp_app (fexp_app coᶠ e1ᶠ) e2ᶠ)
   | d_chk_inf_elab__inf_abs_mono : forall (L:vars) (Ψ:denv) (e:exp) (A B:typ) (eᶠ:fexp),
       d_mono_typ Ψ (typ_arrow A B) ->
       ( forall x , x \notin  L  -> d_chk_inf_elab  ( x ~ (dbind_typ A)  ++  Ψ )  ( open_exp_wrt_exp e (exp_var_f x) ) typingmode__chk B (open_fexp_wrt_fexp eᶠ (fexp_var_f x)))  ->
@@ -345,12 +330,12 @@ Inductive d_chk_inf_elab : denv -> exp -> typing_mode -> typ -> fexp -> Prop :=
       ( forall X , X \notin  L  -> d_chk_inf_elab  ( X ~ dbind_tvar_empty  ++  Ψ ) (exp_anno  ( open_exp_wrt_typ e (typ_var_f X) )  ( open_typ_wrt_typ A (typ_var_f X) ) ) typingmode__chk ( open_typ_wrt_typ A (typ_var_f X) ) (open_fexp_wrt_ftyp eᶠ (ftyp_var_f X)))  ->
       d_chk_inf_elab Ψ (exp_tabs (exp_anno e A)) typingmode__inf (typ_all A)
         (fexp_tabs eᶠ)
-  | d_chk_inf_elab__inf_tapp : forall (Ψ:denv) (e:exp) (A B C:typ) (eᶠ co1 co2:fexp),
+  | d_chk_inf_elab__inf_tapp : forall (Ψ:denv) (e:exp) (A B C:typ) (eᶠ co1ᶠ co2ᶠ:fexp),
       d_wf_typ Ψ B ->
       d_chk_inf_elab Ψ e typingmode__inf A eᶠ ->
-      d_inftapp_elab Ψ A B C co1 co2 ->
+      d_inftapp_elab Ψ A B C co1ᶠ co2ᶠ ->
       d_chk_inf_elab Ψ (exp_tapp e B) typingmode__inf C
-        (fexp_app co2 (fexp_app co1 eᶠ))
+        (fexp_app co2ᶠ (fexp_app co1ᶠ eᶠ))
   | d_chk_inf_elab__chk_abs_top : forall (L:vars) (Ψ:denv) (e:exp) (eᶠ:fexp),
       ( forall x , x \notin  L  -> d_chk_inf_elab  ( x ~ (dbind_typ typ_bot)  ++  Ψ )   ( open_exp_wrt_exp e (exp_var_f x) ) typingmode__chk typ_top (open_fexp_wrt_fexp eᶠ (fexp_var_f x)))  ->
       d_chk_inf_elab Ψ (exp_abs e) typingmode__chk typ_top fexp_unit
@@ -359,11 +344,11 @@ Inductive d_chk_inf_elab : denv -> exp -> typing_mode -> typ -> fexp -> Prop :=
       ( forall x , x \notin  L  -> d_chk_inf_elab  ( x ~ (dbind_typ A)  ++  Ψ )  ( open_exp_wrt_exp e (exp_var_f x) ) typingmode__chk B (open_fexp_wrt_fexp eᶠ (fexp_var_f x)))  ->
       d_chk_inf_elab Ψ (exp_abs e) typingmode__chk (typ_arrow A B)
         (fexp_abs (trans_typ A) eᶠ)
-  | d_chk_inf_elab__chk_sub : forall (Ψ:denv) (e:exp) ( A B:typ) (eᶠ co:fexp),
+  | d_chk_inf_elab__chk_sub : forall (Ψ:denv) (e:exp) ( A B:typ) (eᶠ coᶠ:fexp),
       d_chk_inf_elab Ψ e typingmode__inf A eᶠ ->
-      d_sub_elab Ψ A B co ->
+      d_sub_elab Ψ A B coᶠ ->
       d_chk_inf_elab Ψ e typingmode__chk B
-        (fexp_app co eᶠ)
+        (fexp_app coᶠ eᶠ)
   | d_chk_inf_elab__chk_intersection : forall (Ψ:denv) (e:exp) (A1 A2:typ) (e1ᶠ e2ᶠ:fexp),
       d_chk_inf_elab Ψ e typingmode__chk A1 e1ᶠ ->
       d_chk_inf_elab Ψ e typingmode__chk A2 e2ᶠ ->
@@ -385,8 +370,8 @@ Inductive d_chk_inf_elab : denv -> exp -> typing_mode -> typ -> fexp -> Prop :=
 #[local] Hint Constructors f_typing : core.
 
 
-Theorem d_sub_elab_sound: forall Ψ A B co,
-  Ψ ⊢ A <: B ↪ co -> Ψ ⊢ A <: B.
+Theorem d_sub_elab_sound: forall Ψ A B coᶠ,
+  Ψ ⊢ A <: B ↪ coᶠ -> Ψ ⊢ A <: B.
 Proof.
   intros. induction H; eauto.
 Qed.
@@ -403,48 +388,66 @@ Proof.
 Qed.
 
 
-Lemma d_sub_elab_rename_dtvar : forall Ψ1 Ψ2 A B b X Y co,
+Lemma d_sub_elab_rename_dtvar : forall Ψ1 Ψ2 A B b X Y coᶠ,
   b = □ \/ b = ■ ->
-  Ψ2 ++ (X , b) :: Ψ1  ⊢ A <: B ↪ co ->
+  Ψ2 ++ (X , b) :: Ψ1  ⊢ A <: B ↪ coᶠ ->
   Y ∉ (dom (Ψ2 ++ (X, b) :: Ψ1)) ->
-  (map (subst_tvar_in_dbind `Y X) Ψ2) ++ (Y , b) :: Ψ1  ⊢ {`Y ᵗ/ₜ X} A <: {`Y ᵗ/ₜ X} B ↪ subst_typ_in_fexp (ftyp_var_f Y) X co.
-Proof with eauto 7 using d_wf_typ_rename_dtvar, d_wf_env_rename_dtvar.
-  intros. dependent induction H0; eauto; try solve [simpl; repeat rewrite trans_typ_rename_tvar; eauto using d_wf_typ_rename_dtvar, d_wf_env_rename_dtvar].
-  - admit.
-  - admit.
-  - admit.
-  - admit.
-  - admit.
-  - admit.
+  (map (subst_tvar_in_dbind `Y X) Ψ2) ++ (Y , b) :: Ψ1  ⊢ {`Y ᵗ/ₜ X} A <: {`Y ᵗ/ₜ X} B ↪ subst_typ_in_fexp (ftyp_var_f Y) X coᶠ.
+Proof with eauto 6 using d_wf_typ_rename_dtvar, d_wf_env_rename_dtvar.
+  intros. dependent induction H0; eauto; try solve [simpl; repeat rewrite trans_typ_rename_tvar; eauto 6 using d_wf_typ_rename_dtvar, d_wf_env_rename_dtvar].
+  - simpl. destruct_eq_atom; auto.
+    + econstructor; eauto... destruct H; eauto.
+    + econstructor; eauto... admit.
+  - simpl. repeat rewrite trans_typ_rename_tvar.
+    replace (ftyp_all ᵗ⟦ {` Y ᵗ/ₜ X} A ⟧) with (ᵗ⟦ typ_all ( {` Y ᵗ/ₜ X} A ) ⟧) by auto.
+    inst_cofinites_for d_sub_elab__all; intros; inst_cofinites_with X0; auto.
+    + rewrite subst_tvar_in_typ_open_typ_wrt_typ_fresh2...
+      apply s_in_subst_inv...
+    + rewrite subst_tvar_in_typ_open_typ_wrt_typ_fresh2...
+      apply s_in_subst_inv...
+    + rewrite subst_tvar_in_typ_open_typ_wrt_typ_fresh2...
+      rewrite subst_tvar_in_typ_open_typ_wrt_typ_fresh2...
+      admit.
+  - simpl. repeat rewrite trans_typ_rename_tvar.
+    inst_cofinites_for d_sub_elab__alll; intros; inst_cofinites_with X0; eauto...
+    + rewrite subst_tvar_in_typ_open_typ_wrt_typ_fresh2...
+      apply s_in_subst_inv...
+    + eapply d_mono_typ_rename_dtvar...
+      apply d_sub_elab_sound in H4. apply d_sub_d_wf_env in H4...
+    + rewrite <- subst_tvar_in_typ_open_typ_wrt_typ...
+  - simpl; repeat rewrite trans_typ_rename_tvar... econstructor...
+  - simpl; repeat rewrite trans_typ_rename_tvar... econstructor...
+  - simpl; repeat rewrite trans_typ_rename_tvar... econstructor...
 Admitted.
 
-Lemma d_sub_elab_rename_tvar_cons : forall Ψ A B X Y co b,
+Lemma d_sub_elab_rename_tvar_cons : forall Ψ A B X Y coᶠ b,
   b = □ \/ b = ■ ->
   Y `notin` dom ((X, b) :: Ψ) ->
-  (X , b) :: Ψ ⊢ A <: B ↪ co ->
-  (Y , b) :: Ψ ⊢ {`Y ᵗ/ₜ X} A <: {`Y ᵗ/ₜ X} B ↪ subst_typ_in_fexp (ftyp_var_f Y) X co.
+  (X , b) :: Ψ ⊢ A <: B ↪ coᶠ ->
+  (Y , b) :: Ψ ⊢ {`Y ᵗ/ₜ X} A <: {`Y ᵗ/ₜ X} B ↪ subst_typ_in_fexp (ftyp_var_f Y) X coᶠ.
 Proof.
   intros. rewrite_env ((map (subst_tvar_in_dbind `Y X) nil) ++ (Y , b) :: Ψ). 
   eapply d_sub_elab_rename_dtvar; eauto.
 Qed.
 
 Theorem d_sub_elab_complete: forall Ψ A B,
-  Ψ ⊢ A <: B -> exists co, Ψ ⊢ A <: B ↪ co.
+  Ψ ⊢ A <: B -> exists coᶠ, Ψ ⊢ A <: B ↪ coᶠ.
 Proof with auto.
   intros. induction H; eauto 4; try solve [destruct_conj; eauto 4].
   - pick fresh X. inst_cofinites_with_keep X.
-    destruct H3 as [co ?].
+    destruct H3 as [coᶠ ?].
     exists 
-      (fexp_abs (trans_typ (typ_all A)) (fexp_tabs (fexp_app (open_fexp_wrt_ftyp (close_fexp_wrt_ftyp X co) (ftyp_var_b 0)) (fexp_tapp (fexp_var_b 0) (ftyp_var_b 0))))).
+      (fexp_abs (trans_typ (typ_all A)) (fexp_tabs (fexp_app (close_fexp_wrt_ftyp X coᶠ) (fexp_tapp (fexp_var_b 0) (ftyp_var_b 0))))).
     inst_cofinites_for d_sub_elab__all; intros; inst_cofinites_with X0; auto.
     erewrite <- subst_tvar_in_typ_open_typ_wrt_typ_tvar2 with (X:=X)...
     erewrite <- subst_tvar_in_typ_open_typ_wrt_typ_tvar2 with (X:=X) (A:=B)...
-    admit.  (* *, d_sub_elab_rename_tvar *)
-Admitted.
+    erewrite (subst_typ_in_fexp_intro X (close_fexp_wrt_ftyp X coᶠ)) by apply close_fexp_wrt_ftyp_notin.
+    + rewrite open_fexp_wrt_ftyp_close_fexp_wrt_ftyp.
+      eapply d_sub_elab_rename_tvar_cons; eauto.
+Qed.
       
-
-Theorem sub_elab_lc_fexp : forall Ψ A B co,
-  Ψ ⊢ A <: B ↪ co -> lc_fexp co.
+Theorem sub_elab_lc_fexp : forall Ψ A B coᶠ,
+  Ψ ⊢ A <: B ↪ coᶠ -> lc_fexp coᶠ.
 Proof with eauto 4.
   intros. induction H...
   - apply lc_fexp_abs...
@@ -520,22 +523,34 @@ Proof with eauto 4.
     rewrite open_fexp_wrt_fexp_rec_lc_fexp; auto. *)
 Admitted.
       
-Theorem d_sub_elab_sound_f : forall Ψ A B co,
-  Ψ ⊢ A <: B ↪ co -> ᵉ⟦ Ψ ⟧ ⊢ co : ftyp_arrow ᵗ⟦ A ⟧ ᵗ⟦ B ⟧.
+Theorem d_sub_elab_sound_f : forall Ψ A B coᶠ,
+  Ψ ⊢ A <: B ↪ coᶠ -> ⟦ Ψ ⟧ ⊢ coᶠ : ftyp_arrow ᵗ⟦ A ⟧ ᵗ⟦ B ⟧.
 Proof with eauto 4.
   intros. induction H...
 Admitted.
 
 
-Theorem d_infabs_elab_sound_f : forall Ψ A B C co,
-  Ψ ⊢ A ▹ B → C ↪ co -> 
-  ᵉ⟦ Ψ ⟧ ⊢ co : ftyp_arrow ᵗ⟦ A ⟧ (ftyp_arrow ᵗ⟦ B ⟧ ᵗ⟦ C ⟧).
+Theorem d_infabs_complete : forall Ψ A B C,
+  Ψ ⊢ A ▹ B → C -> exists coᶠ, Ψ ⊢ A ▹ B → C ↪ coᶠ.
 Proof.
 Admitted.
 
-Theorem d_inftapp_elab_sound_f : forall Ψ A B C co1 co2,
-  Ψ ⊢ A ○ B ⇒⇒ C ↪ co1 | co2 ->
-  exists D : ftyp, ᵉ⟦ Ψ ⟧ ⊢ co1 : ftyp_arrow ᵗ⟦ A ⟧ D /\ ᵉ⟦ Ψ ⟧ ⊢ co2 : ftyp_arrow D ᵗ⟦ C ⟧.
+
+Theorem d_infabs_elab_sound_f : forall Ψ A B C coᶠ,
+  Ψ ⊢ A ▹ B → C ↪ coᶠ -> 
+  ⟦ Ψ ⟧ ⊢ coᶠ : ftyp_arrow ᵗ⟦ A ⟧ (ftyp_arrow ᵗ⟦ B ⟧ ᵗ⟦ C ⟧).
+Proof.
+Admitted.
+
+
+Theorem d_inftapp_elab_complete : forall Ψ A B C,
+  Ψ ⊢ A ○ B ⇒⇒ C -> exists co1ᶠ co2ᶠ, Ψ ⊢ A ○ B ⇒⇒ C ↪ co1ᶠ | co2ᶠ.
+Proof.
+Admitted.
+
+Theorem d_inftapp_elab_sound_f : forall Ψ A B C co1ᶠ co2ᶠ,
+  Ψ ⊢ A ○ B ⇒⇒ C ↪ co1ᶠ | co2ᶠ ->
+  exists D : ftyp, ⟦ Ψ ⟧ ⊢ co1ᶠ : ftyp_arrow ᵗ⟦ A ⟧ D /\ ⟦ Ψ ⟧ ⊢ co2ᶠ : ftyp_arrow D ᵗ⟦ C ⟧.
 Proof.
 Admitted.
 
@@ -545,8 +560,15 @@ Proof.
   intros. induction H; eauto; simpl.
 Admitted.
 
+
+Theorem d_chk_inf_elab_complete : forall Ψ e mode A,
+  d_chk_inf Ψ e mode A -> exists eᶠ, d_chk_inf_elab Ψ e mode A eᶠ.
+Proof.
+Admitted. 
+
+
 Theorem d_chk_inf_elab_sound_f : forall Ψ e A eᶠ mode,
-  d_chk_inf_elab Ψ e mode A eᶠ -> ᵉ⟦ Ψ ⟧ ⊢ eᶠ : ᵗ⟦ A ⟧.
+  d_chk_inf_elab Ψ e mode A eᶠ -> ⟦ Ψ ⟧ ⊢ eᶠ : ᵗ⟦ A ⟧.
 Proof.
 Admitted.
 
@@ -794,9 +816,9 @@ Proof with eauto with safety.
       apply typing_var; auto. admit. (* wf *)
   - apply typing_abs with (L:=dom Ψ).
     unfold open_fexp_wrt_fexp. simpl. intros.
-    assert (Hlc1: lc_fexp co1).
+    assert (Hlc1: lc_fexp co1ᶠ).
     { apply infabs_elab_lc_fexp in H. auto. }
-    assert (Hlc2: lc_fexp co2).
+    assert (Hlc2: lc_fexp co2ᶠ).
     { apply infabs_elab_lc_fexp in H0. auto. }
     repeat rewrite open_fexp_wrt_fexp_rec_lc_fexp; auto.
     apply typing_abs with (L:=dom Ψ `union` singleton x).
@@ -826,8 +848,8 @@ Admitted.
 
 
 
-Theorem inftapp_elab_lc_fexp : forall Ψ A B C co1 co2,
-  d_inftapp_elab Ψ A B C co1 co2 -> lc_fexp co1 /\ lc_fexp co2.
+Theorem inftapp_elab_lc_fexp : forall Ψ A B C co1ᶠ co2ᶠ,
+  d_inftapp_elab Ψ A B C co1ᶠ co2ᶠ -> lc_fexp co1ᶠ /\ lc_fexp co2ᶠ.
 Proof.
   intros. induction H; eauto with safety; simpl.
   - split; apply lc_fexp_abs; eauto with safety;
@@ -842,10 +864,10 @@ Proof.
       apply lc_fexp_tapp; eauto. apply trans_typ_lc_ftyp. eauto. 
 Admitted.
 
-Theorem inftapp_sound_f : forall Ψ A B C co1 co2,
-  d_inftapp_elab Ψ A B C co1 co2 -> exists D,
-  typing (trans_env Ψ) co1 (ftyp_arrow (trans_typ A) D) /\
-    typing (trans_env Ψ) co2 (ftyp_arrow D (trans_typ C)).
+Theorem inftapp_sound_f : forall Ψ A B C co1ᶠ co2ᶠ,
+  d_inftapp_elab Ψ A B C co1ᶠ co2ᶠ -> exists D,
+  typing (trans_env Ψ) co1ᶠ (ftyp_arrow (trans_typ A) D) /\
+    typing (trans_env Ψ) co2ᶠ (ftyp_arrow D (trans_typ C)).
 Proof with eauto with safety.
   intros. induction H; simpl; eauto.
   - exists (ftyp_all (ftyp_var_b 0)). split.
@@ -869,7 +891,7 @@ Proof with eauto with safety.
     exists x. split.
     + apply typing_abs with (L:=dom Ψ).  
       unfold open_fexp_wrt_fexp. simpl. intros.
-      assert (Hlc: lc_fexp co1 /\ lc_fexp co2).
+      assert (Hlc: lc_fexp co1ᶠ /\ lc_fexp co2ᶠ).
       { apply inftapp_elab_lc_fexp in H1. auto. }
       destruct Hlc as [Hlc1 Hlc2].
       rewrite open_fexp_wrt_fexp_rec_lc_fexp; auto.
@@ -882,7 +904,7 @@ Proof with eauto with safety.
     exists x. split.
     + apply typing_abs with (L:=dom Ψ).
       unfold open_fexp_wrt_fexp. simpl. intros.
-      assert (Hlc: lc_fexp co1 /\ lc_fexp co2).
+      assert (Hlc: lc_fexp co1ᶠ /\ lc_fexp co2ᶠ).
       { apply inftapp_elab_lc_fexp in H1. auto. }
       destruct Hlc as [Hlc1 Hlc2].
       rewrite open_fexp_wrt_fexp_rec_lc_fexp; auto.
@@ -896,7 +918,7 @@ Proof with eauto with safety.
     exists (trans_typ (typ_intersection C1 C2)). split.
     + apply typing_abs with (L:=dom Ψ).
       unfold open_fexp_wrt_fexp. simpl. intros.
-      assert (Hlc12: lc_fexp co1 /\ lc_fexp co2).
+      assert (Hlc12: lc_fexp co1ᶠ /\ lc_fexp co2ᶠ).
       { apply inftapp_elab_lc_fexp in H. auto. }
       destruct Hlc12 as [Hlc1 Hlc2].
       assert (Hlc34: lc_fexp co3 /\ lc_fexp co4).
@@ -924,7 +946,7 @@ Proof with eauto with safety.
     exists (trans_typ (typ_union C1 C2)). split.
     + apply typing_abs with (L:=dom Ψ).
       unfold open_fexp_wrt_fexp. simpl. intros.
-      assert (Hlc12: lc_fexp co1 /\ lc_fexp co2).
+      assert (Hlc12: lc_fexp co1ᶠ /\ lc_fexp co2ᶠ).
       { apply inftapp_elab_lc_fexp in H. auto. }
       destruct Hlc12 as [Hlc1 Hlc2].
       assert (Hlc34: lc_fexp co3 /\ lc_fexp co4).
