proof/systemf/prop_ln.v
@@ -2087,7 +2087,7 @@ Qed.
 
 Lemma close_ftyp_wrt_ftyp_rec_open_ftyp_wrt_ftyp_rec_mutual :
 (forall A1 X1 n1,
-  X1 `notin` fv_ftyp_in_ftyp A1 ->
+  X1 `notin` ftvar_in_ftyp A1 ->
   close_ftyp_wrt_ftyp_rec n1 X1 (open_ftyp_wrt_ftyp_rec n1 (ftyp_var_f X1) A1) = A1).
 Proof.
 apply_mutual_ind ftyp_mutind;
@@ -2100,7 +2100,7 @@ Qed.
 
 Lemma close_ftyp_wrt_ftyp_rec_open_ftyp_wrt_ftyp_rec :
 forall A1 X1 n1,
-  X1 `notin` fv_ftyp_in_ftyp A1 ->
+  X1 `notin` ftvar_in_ftyp A1 ->
   close_ftyp_wrt_ftyp_rec n1 X1 (open_ftyp_wrt_ftyp_rec n1 (ftyp_var_f X1) A1) = A1.
 Proof.
 pose proof close_ftyp_wrt_ftyp_rec_open_ftyp_wrt_ftyp_rec_mutual as H; intuition eauto.
@@ -2115,7 +2115,7 @@ Qed.
 
 Lemma close_fexp_wrt_ftyp_rec_open_fexp_wrt_ftyp_rec_mutual :
 (forall e1 X1 n1,
-  X1 `notin` fv_ftyp_in_fexp e1 ->
+  X1 `notin` ftvar_in_fexp e1 ->
   close_fexp_wrt_ftyp_rec n1 X1 (open_fexp_wrt_ftyp_rec n1 (ftyp_var_f X1) e1) = e1).
 Proof.
 apply_mutual_ind fexp_mutind;
@@ -2128,7 +2128,7 @@ Qed.
 
 Lemma close_fexp_wrt_ftyp_rec_open_fexp_wrt_ftyp_rec :
 forall e1 X1 n1,
-  X1 `notin` fv_ftyp_in_fexp e1 ->
+  X1 `notin` ftvar_in_fexp e1 ->
   close_fexp_wrt_ftyp_rec n1 X1 (open_fexp_wrt_ftyp_rec n1 (ftyp_var_f X1) e1) = e1.
 Proof.
 pose proof close_fexp_wrt_ftyp_rec_open_fexp_wrt_ftyp_rec_mutual as H; intuition eauto.
@@ -2143,7 +2143,7 @@ Qed.
 
 Lemma close_fexp_wrt_fexp_rec_open_fexp_wrt_fexp_rec_mutual :
 (forall e1 x1 n1,
-  x1 `notin` fv_fexp_in_fexp e1 ->
+  x1 `notin` fvar_in_fexp e1 ->
   close_fexp_wrt_fexp_rec n1 x1 (open_fexp_wrt_fexp_rec n1 (fexp_var_f x1) e1) = e1).
 Proof.
 apply_mutual_ind fexp_mutind;
@@ -2156,7 +2156,7 @@ Qed.
 
 Lemma close_fexp_wrt_fexp_rec_open_fexp_wrt_fexp_rec :
 forall e1 x1 n1,
-  x1 `notin` fv_fexp_in_fexp e1 ->
+  x1 `notin` fvar_in_fexp e1 ->
   close_fexp_wrt_fexp_rec n1 x1 (open_fexp_wrt_fexp_rec n1 (fexp_var_f x1) e1) = e1.
 Proof.
 pose proof close_fexp_wrt_fexp_rec_open_fexp_wrt_fexp_rec_mutual as H; intuition eauto.
@@ -2171,7 +2171,7 @@ Qed.
 
 Lemma close_fbind_wrt_ftyp_rec_open_fbind_wrt_ftyp_rec_mutual :
 (forall fb1 X1 n1,
-  X1 `notin` fv_ftyp_in_fbind fb1 ->
+  X1 `notin` ftvar_in_fbind fb1 ->
   close_fbind_wrt_ftyp_rec n1 X1 (open_fbind_wrt_ftyp_rec n1 (ftyp_var_f X1) fb1) = fb1).
 Proof.
 apply_mutual_ind fbind_mutind;
@@ -2184,7 +2184,7 @@ Qed.
 
 Lemma close_fbind_wrt_ftyp_rec_open_fbind_wrt_ftyp_rec :
 forall fb1 X1 n1,
-  X1 `notin` fv_ftyp_in_fbind fb1 ->
+  X1 `notin` ftvar_in_fbind fb1 ->
   close_fbind_wrt_ftyp_rec n1 X1 (open_fbind_wrt_ftyp_rec n1 (ftyp_var_f X1) fb1) = fb1.
 Proof.
 pose proof close_fbind_wrt_ftyp_rec_open_fbind_wrt_ftyp_rec_mutual as H; intuition eauto.
@@ -2197,7 +2197,7 @@ Qed.
 
 Lemma close_ftyp_wrt_ftyp_open_ftyp_wrt_ftyp :
 forall A1 X1,
-  X1 `notin` fv_ftyp_in_ftyp A1 ->
+  X1 `notin` ftvar_in_ftyp A1 ->
   close_ftyp_wrt_ftyp X1 (open_ftyp_wrt_ftyp A1 (ftyp_var_f X1)) = A1.
 Proof.
 unfold close_ftyp_wrt_ftyp; unfold open_ftyp_wrt_ftyp; default_simp.
@@ -2208,7 +2208,7 @@ Qed.
 
 Lemma close_fexp_wrt_ftyp_open_fexp_wrt_ftyp :
 forall e1 X1,
-  X1 `notin` fv_ftyp_in_fexp e1 ->
+  X1 `notin` ftvar_in_fexp e1 ->
   close_fexp_wrt_ftyp X1 (open_fexp_wrt_ftyp e1 (ftyp_var_f X1)) = e1.
 Proof.
 unfold close_fexp_wrt_ftyp; unfold open_fexp_wrt_ftyp; default_simp.
@@ -2219,7 +2219,7 @@ Qed.
 
 Lemma close_fexp_wrt_fexp_open_fexp_wrt_fexp :
 forall e1 x1,
-  x1 `notin` fv_fexp_in_fexp e1 ->
+  x1 `notin` fvar_in_fexp e1 ->
   close_fexp_wrt_fexp x1 (open_fexp_wrt_fexp e1 (fexp_var_f x1)) = e1.
 Proof.
 unfold close_fexp_wrt_fexp; unfold open_fexp_wrt_fexp; default_simp.
@@ -2230,7 +2230,7 @@ Qed.
 
 Lemma close_fbind_wrt_ftyp_open_fbind_wrt_ftyp :
 forall fb1 X1,
-  X1 `notin` fv_ftyp_in_fbind fb1 ->
+  X1 `notin` ftvar_in_fbind fb1 ->
   close_fbind_wrt_ftyp X1 (open_fbind_wrt_ftyp fb1 (ftyp_var_f X1)) = fb1.
 Proof.
 unfold close_fbind_wrt_ftyp; unfold open_fbind_wrt_ftyp; default_simp.
@@ -2387,8 +2387,8 @@ Qed.
 
 Lemma open_ftyp_wrt_ftyp_rec_inj_mutual :
 (forall A2 A1 X1 n1,
-  X1 `notin` fv_ftyp_in_ftyp A2 ->
-  X1 `notin` fv_ftyp_in_ftyp A1 ->
+  X1 `notin` ftvar_in_ftyp A2 ->
+  X1 `notin` ftvar_in_ftyp A1 ->
   open_ftyp_wrt_ftyp_rec n1 (ftyp_var_f X1) A2 = open_ftyp_wrt_ftyp_rec n1 (ftyp_var_f X1) A1 ->
   A2 = A1).
 Proof.
@@ -2405,8 +2405,8 @@ Qed.
 
 Lemma open_ftyp_wrt_ftyp_rec_inj :
 forall A2 A1 X1 n1,
-  X1 `notin` fv_ftyp_in_ftyp A2 ->
-  X1 `notin` fv_ftyp_in_ftyp A1 ->
+  X1 `notin` ftvar_in_ftyp A2 ->
+  X1 `notin` ftvar_in_ftyp A1 ->
   open_ftyp_wrt_ftyp_rec n1 (ftyp_var_f X1) A2 = open_ftyp_wrt_ftyp_rec n1 (ftyp_var_f X1) A1 ->
   A2 = A1.
 Proof.
@@ -2421,8 +2421,8 @@ Qed.
 
 Lemma open_fexp_wrt_ftyp_rec_inj_mutual :
 (forall e2 e1 X1 n1,
-  X1 `notin` fv_ftyp_in_fexp e2 ->
-  X1 `notin` fv_ftyp_in_fexp e1 ->
+  X1 `notin` ftvar_in_fexp e2 ->
+  X1 `notin` ftvar_in_fexp e1 ->
   open_fexp_wrt_ftyp_rec n1 (ftyp_var_f X1) e2 = open_fexp_wrt_ftyp_rec n1 (ftyp_var_f X1) e1 ->
   e2 = e1).
 Proof.
@@ -2439,8 +2439,8 @@ Qed.
 
 Lemma open_fexp_wrt_ftyp_rec_inj :
 forall e2 e1 X1 n1,
-  X1 `notin` fv_ftyp_in_fexp e2 ->
-  X1 `notin` fv_ftyp_in_fexp e1 ->
+  X1 `notin` ftvar_in_fexp e2 ->
+  X1 `notin` ftvar_in_fexp e1 ->
   open_fexp_wrt_ftyp_rec n1 (ftyp_var_f X1) e2 = open_fexp_wrt_ftyp_rec n1 (ftyp_var_f X1) e1 ->
   e2 = e1.
 Proof.
@@ -2455,8 +2455,8 @@ Qed.
 
 Lemma open_fexp_wrt_fexp_rec_inj_mutual :
 (forall e2 e1 x1 n1,
-  x1 `notin` fv_fexp_in_fexp e2 ->
-  x1 `notin` fv_fexp_in_fexp e1 ->
+  x1 `notin` fvar_in_fexp e2 ->
+  x1 `notin` fvar_in_fexp e1 ->
   open_fexp_wrt_fexp_rec n1 (fexp_var_f x1) e2 = open_fexp_wrt_fexp_rec n1 (fexp_var_f x1) e1 ->
   e2 = e1).
 Proof.
@@ -2473,8 +2473,8 @@ Qed.
 
 Lemma open_fexp_wrt_fexp_rec_inj :
 forall e2 e1 x1 n1,
-  x1 `notin` fv_fexp_in_fexp e2 ->
-  x1 `notin` fv_fexp_in_fexp e1 ->
+  x1 `notin` fvar_in_fexp e2 ->
+  x1 `notin` fvar_in_fexp e1 ->
   open_fexp_wrt_fexp_rec n1 (fexp_var_f x1) e2 = open_fexp_wrt_fexp_rec n1 (fexp_var_f x1) e1 ->
   e2 = e1.
 Proof.
@@ -2489,8 +2489,8 @@ Qed.
 
 Lemma open_fbind_wrt_ftyp_rec_inj_mutual :
 (forall fb2 fb1 X1 n1,
-  X1 `notin` fv_ftyp_in_fbind fb2 ->
-  X1 `notin` fv_ftyp_in_fbind fb1 ->
+  X1 `notin` ftvar_in_fbind fb2 ->
+  X1 `notin` ftvar_in_fbind fb1 ->
   open_fbind_wrt_ftyp_rec n1 (ftyp_var_f X1) fb2 = open_fbind_wrt_ftyp_rec n1 (ftyp_var_f X1) fb1 ->
   fb2 = fb1).
 Proof.
@@ -2507,8 +2507,8 @@ Qed.
 
 Lemma open_fbind_wrt_ftyp_rec_inj :
 forall fb2 fb1 X1 n1,
-  X1 `notin` fv_ftyp_in_fbind fb2 ->
-  X1 `notin` fv_ftyp_in_fbind fb1 ->
+  X1 `notin` ftvar_in_fbind fb2 ->
+  X1 `notin` ftvar_in_fbind fb1 ->
   open_fbind_wrt_ftyp_rec n1 (ftyp_var_f X1) fb2 = open_fbind_wrt_ftyp_rec n1 (ftyp_var_f X1) fb1 ->
   fb2 = fb1.
 Proof.
@@ -2521,8 +2521,8 @@ Qed.
 
 Lemma open_ftyp_wrt_ftyp_inj :
 forall A2 A1 X1,
-  X1 `notin` fv_ftyp_in_ftyp A2 ->
-  X1 `notin` fv_ftyp_in_ftyp A1 ->
+  X1 `notin` ftvar_in_ftyp A2 ->
+  X1 `notin` ftvar_in_ftyp A1 ->
   open_ftyp_wrt_ftyp A2 (ftyp_var_f X1) = open_ftyp_wrt_ftyp A1 (ftyp_var_f X1) ->
   A2 = A1.
 Proof.
@@ -2533,8 +2533,8 @@ Qed.
 
 Lemma open_fexp_wrt_ftyp_inj :
 forall e2 e1 X1,
-  X1 `notin` fv_ftyp_in_fexp e2 ->
-  X1 `notin` fv_ftyp_in_fexp e1 ->
+  X1 `notin` ftvar_in_fexp e2 ->
+  X1 `notin` ftvar_in_fexp e1 ->
   open_fexp_wrt_ftyp e2 (ftyp_var_f X1) = open_fexp_wrt_ftyp e1 (ftyp_var_f X1) ->
   e2 = e1.
 Proof.
@@ -2545,8 +2545,8 @@ Qed.
 
 Lemma open_fexp_wrt_fexp_inj :
 forall e2 e1 x1,
-  x1 `notin` fv_fexp_in_fexp e2 ->
-  x1 `notin` fv_fexp_in_fexp e1 ->
+  x1 `notin` fvar_in_fexp e2 ->
+  x1 `notin` fvar_in_fexp e1 ->
   open_fexp_wrt_fexp e2 (fexp_var_f x1) = open_fexp_wrt_fexp e1 (fexp_var_f x1) ->
   e2 = e1.
 Proof.
@@ -2557,8 +2557,8 @@ Qed.
 
 Lemma open_fbind_wrt_ftyp_inj :
 forall fb2 fb1 X1,
-  X1 `notin` fv_ftyp_in_fbind fb2 ->
-  X1 `notin` fv_ftyp_in_fbind fb1 ->
+  X1 `notin` ftvar_in_fbind fb2 ->
+  X1 `notin` ftvar_in_fbind fb1 ->
   open_fbind_wrt_ftyp fb2 (ftyp_var_f X1) = open_fbind_wrt_ftyp fb1 (ftyp_var_f X1) ->
   fb2 = fb1.
 Proof.
@@ -3264,7 +3264,7 @@ Ltac default_autorewrite ::= fail.
 Lemma close_ftyp_wrt_ftyp_rec_degree_ftyp_wrt_ftyp_mutual :
 (forall A1 X1 n1,
   degree_ftyp_wrt_ftyp n1 A1 ->
-  X1 `notin` fv_ftyp_in_ftyp A1 ->
+  X1 `notin` ftvar_in_ftyp A1 ->
   close_ftyp_wrt_ftyp_rec n1 X1 A1 = A1).
 Proof.
 apply_mutual_ind ftyp_mutind;
@@ -3278,7 +3278,7 @@ Qed.
 Lemma close_ftyp_wrt_ftyp_rec_degree_ftyp_wrt_ftyp :
 forall A1 X1 n1,
   degree_ftyp_wrt_ftyp n1 A1 ->
-  X1 `notin` fv_ftyp_in_ftyp A1 ->
+  X1 `notin` ftvar_in_ftyp A1 ->
   close_ftyp_wrt_ftyp_rec n1 X1 A1 = A1.
 Proof.
 pose proof close_ftyp_wrt_ftyp_rec_degree_ftyp_wrt_ftyp_mutual as H; intuition eauto.
@@ -3294,7 +3294,7 @@ Qed.
 Lemma close_fexp_wrt_ftyp_rec_degree_fexp_wrt_ftyp_mutual :
 (forall e1 X1 n1,
   degree_fexp_wrt_ftyp n1 e1 ->
-  X1 `notin` fv_ftyp_in_fexp e1 ->
+  X1 `notin` ftvar_in_fexp e1 ->
   close_fexp_wrt_ftyp_rec n1 X1 e1 = e1).
 Proof.
 apply_mutual_ind fexp_mutind;
@@ -3308,7 +3308,7 @@ Qed.
 Lemma close_fexp_wrt_ftyp_rec_degree_fexp_wrt_ftyp :
 forall e1 X1 n1,
   degree_fexp_wrt_ftyp n1 e1 ->
-  X1 `notin` fv_ftyp_in_fexp e1 ->
+  X1 `notin` ftvar_in_fexp e1 ->
   close_fexp_wrt_ftyp_rec n1 X1 e1 = e1.
 Proof.
 pose proof close_fexp_wrt_ftyp_rec_degree_fexp_wrt_ftyp_mutual as H; intuition eauto.
@@ -3324,7 +3324,7 @@ Qed.
 Lemma close_fexp_wrt_fexp_rec_degree_fexp_wrt_fexp_mutual :
 (forall e1 x1 n1,
   degree_fexp_wrt_fexp n1 e1 ->
-  x1 `notin` fv_fexp_in_fexp e1 ->
+  x1 `notin` fvar_in_fexp e1 ->
   close_fexp_wrt_fexp_rec n1 x1 e1 = e1).
 Proof.
 apply_mutual_ind fexp_mutind;
@@ -3338,7 +3338,7 @@ Qed.
 Lemma close_fexp_wrt_fexp_rec_degree_fexp_wrt_fexp :
 forall e1 x1 n1,
   degree_fexp_wrt_fexp n1 e1 ->
-  x1 `notin` fv_fexp_in_fexp e1 ->
+  x1 `notin` fvar_in_fexp e1 ->
   close_fexp_wrt_fexp_rec n1 x1 e1 = e1.
 Proof.
 pose proof close_fexp_wrt_fexp_rec_degree_fexp_wrt_fexp_mutual as H; intuition eauto.
@@ -3354,7 +3354,7 @@ Qed.
 Lemma close_fbind_wrt_ftyp_rec_degree_fbind_wrt_ftyp_mutual :
 (forall fb1 X1 n1,
   degree_fbind_wrt_ftyp n1 fb1 ->
-  X1 `notin` fv_ftyp_in_fbind fb1 ->
+  X1 `notin` ftvar_in_fbind fb1 ->
   close_fbind_wrt_ftyp_rec n1 X1 fb1 = fb1).
 Proof.
 apply_mutual_ind fbind_mutind;
@@ -3368,7 +3368,7 @@ Qed.
 Lemma close_fbind_wrt_ftyp_rec_degree_fbind_wrt_ftyp :
 forall fb1 X1 n1,
   degree_fbind_wrt_ftyp n1 fb1 ->
-  X1 `notin` fv_ftyp_in_fbind fb1 ->
+  X1 `notin` ftvar_in_fbind fb1 ->
   close_fbind_wrt_ftyp_rec n1 X1 fb1 = fb1.
 Proof.
 pose proof close_fbind_wrt_ftyp_rec_degree_fbind_wrt_ftyp_mutual as H; intuition eauto.
@@ -3382,7 +3382,7 @@ Qed.
 Lemma close_ftyp_wrt_ftyp_lc_ftyp :
 forall A1 X1,
   lc_ftyp A1 ->
-  X1 `notin` fv_ftyp_in_ftyp A1 ->
+  X1 `notin` ftvar_in_ftyp A1 ->
   close_ftyp_wrt_ftyp X1 A1 = A1.
 Proof.
 unfold close_ftyp_wrt_ftyp; default_simp.
@@ -3394,7 +3394,7 @@ Qed.
 Lemma close_fexp_wrt_ftyp_lc_fexp :
 forall e1 X1,
   lc_fexp e1 ->
-  X1 `notin` fv_ftyp_in_fexp e1 ->
+  X1 `notin` ftvar_in_fexp e1 ->
   close_fexp_wrt_ftyp X1 e1 = e1.
 Proof.
 unfold close_fexp_wrt_ftyp; default_simp.
@@ -3406,7 +3406,7 @@ Qed.
 Lemma close_fexp_wrt_fexp_lc_fexp :
 forall e1 x1,
   lc_fexp e1 ->
-  x1 `notin` fv_fexp_in_fexp e1 ->
+  x1 `notin` fvar_in_fexp e1 ->
   close_fexp_wrt_fexp x1 e1 = e1.
 Proof.
 unfold close_fexp_wrt_fexp; default_simp.
@@ -3418,7 +3418,7 @@ Qed.
 Lemma close_fbind_wrt_ftyp_lc_fbind :
 forall fb1 X1,
   lc_fbind fb1 ->
-  X1 `notin` fv_ftyp_in_fbind fb1 ->
+  X1 `notin` ftvar_in_fbind fb1 ->
   close_fbind_wrt_ftyp X1 fb1 = fb1.
 Proof.
 unfold close_fbind_wrt_ftyp; default_simp.
@@ -3592,9 +3592,9 @@ Ltac default_autorewrite ::= autorewrite with lngen.
 
 (* begin hide *)
 
-Lemma fv_ftyp_in_ftyp_close_ftyp_wrt_ftyp_rec_mutual :
+Lemma ftvar_in_ftyp_close_ftyp_wrt_ftyp_rec_mutual :
 (forall A1 X1 n1,
-  fv_ftyp_in_ftyp (close_ftyp_wrt_ftyp_rec n1 X1 A1) [=] remove X1 (fv_ftyp_in_ftyp A1)).
+  ftvar_in_ftyp (close_ftyp_wrt_ftyp_rec n1 X1 A1) [=] remove X1 (ftvar_in_ftyp A1)).
 Proof.
 apply_mutual_ind ftyp_mutind;
 default_simp; fsetdec.
@@ -3604,23 +3604,23 @@ Qed.
 
 (* begin hide *)
 
-Lemma fv_ftyp_in_ftyp_close_ftyp_wrt_ftyp_rec :
+Lemma ftvar_in_ftyp_close_ftyp_wrt_ftyp_rec :
 forall A1 X1 n1,
-  fv_ftyp_in_ftyp (close_ftyp_wrt_ftyp_rec n1 X1 A1) [=] remove X1 (fv_ftyp_in_ftyp A1).
+  ftvar_in_ftyp (close_ftyp_wrt_ftyp_rec n1 X1 A1) [=] remove X1 (ftvar_in_ftyp A1).
 Proof.
-pose proof fv_ftyp_in_ftyp_close_ftyp_wrt_ftyp_rec_mutual as H; intuition eauto.
+pose proof ftvar_in_ftyp_close_ftyp_wrt_ftyp_rec_mutual as H; intuition eauto.
 Qed.
 
-#[export] Hint Resolve fv_ftyp_in_ftyp_close_ftyp_wrt_ftyp_rec : lngen.
-#[export] Hint Rewrite fv_ftyp_in_ftyp_close_ftyp_wrt_ftyp_rec using solve [auto] : lngen.
+#[export] Hint Resolve ftvar_in_ftyp_close_ftyp_wrt_ftyp_rec : lngen.
+#[export] Hint Rewrite ftvar_in_ftyp_close_ftyp_wrt_ftyp_rec using solve [auto] : lngen.
 
 (* end hide *)
 
 (* begin hide *)
 
-Lemma fv_ftyp_in_fexp_close_fexp_wrt_ftyp_rec_mutual :
+Lemma ftvar_in_fexp_close_fexp_wrt_ftyp_rec_mutual :
 (forall e1 X1 n1,
-  fv_ftyp_in_fexp (close_fexp_wrt_ftyp_rec n1 X1 e1) [=] remove X1 (fv_ftyp_in_fexp e1)).
+  ftvar_in_fexp (close_fexp_wrt_ftyp_rec n1 X1 e1) [=] remove X1 (ftvar_in_fexp e1)).
 Proof.
 apply_mutual_ind fexp_mutind;
 default_simp; fsetdec.
@@ -3630,23 +3630,23 @@ Qed.
 
 (* begin hide *)
 
-Lemma fv_ftyp_in_fexp_close_fexp_wrt_ftyp_rec :
+Lemma ftvar_in_fexp_close_fexp_wrt_ftyp_rec :
 forall e1 X1 n1,
-  fv_ftyp_in_fexp (close_fexp_wrt_ftyp_rec n1 X1 e1) [=] remove X1 (fv_ftyp_in_fexp e1).
+  ftvar_in_fexp (close_fexp_wrt_ftyp_rec n1 X1 e1) [=] remove X1 (ftvar_in_fexp e1).
 Proof.
-pose proof fv_ftyp_in_fexp_close_fexp_wrt_ftyp_rec_mutual as H; intuition eauto.
+pose proof ftvar_in_fexp_close_fexp_wrt_ftyp_rec_mutual as H; intuition eauto.
 Qed.
 
-#[export] Hint Resolve fv_ftyp_in_fexp_close_fexp_wrt_ftyp_rec : lngen.
-#[export] Hint Rewrite fv_ftyp_in_fexp_close_fexp_wrt_ftyp_rec using solve [auto] : lngen.
+#[export] Hint Resolve ftvar_in_fexp_close_fexp_wrt_ftyp_rec : lngen.
+#[export] Hint Rewrite ftvar_in_fexp_close_fexp_wrt_ftyp_rec using solve [auto] : lngen.
 
 (* end hide *)
 
 (* begin hide *)
 
-Lemma fv_ftyp_in_fexp_close_fexp_wrt_fexp_rec_mutual :
+Lemma ftvar_in_fexp_close_fexp_wrt_fexp_rec_mutual :
 (forall e1 x1 n1,
-  fv_ftyp_in_fexp (close_fexp_wrt_fexp_rec n1 x1 e1) [=] fv_ftyp_in_fexp e1).
+  ftvar_in_fexp (close_fexp_wrt_fexp_rec n1 x1 e1) [=] ftvar_in_fexp e1).
 Proof.
 apply_mutual_ind fexp_mutind;
 default_simp; fsetdec.
@@ -3656,23 +3656,23 @@ Qed.
 
 (* begin hide *)
 
-Lemma fv_ftyp_in_fexp_close_fexp_wrt_fexp_rec :
+Lemma ftvar_in_fexp_close_fexp_wrt_fexp_rec :
 forall e1 x1 n1,
-  fv_ftyp_in_fexp (close_fexp_wrt_fexp_rec n1 x1 e1) [=] fv_ftyp_in_fexp e1.
+  ftvar_in_fexp (close_fexp_wrt_fexp_rec n1 x1 e1) [=] ftvar_in_fexp e1.
 Proof.
-pose proof fv_ftyp_in_fexp_close_fexp_wrt_fexp_rec_mutual as H; intuition eauto.
+pose proof ftvar_in_fexp_close_fexp_wrt_fexp_rec_mutual as H; intuition eauto.
 Qed.
 
-#[export] Hint Resolve fv_ftyp_in_fexp_close_fexp_wrt_fexp_rec : lngen.
-#[export] Hint Rewrite fv_ftyp_in_fexp_close_fexp_wrt_fexp_rec using solve [auto] : lngen.
+#[export] Hint Resolve ftvar_in_fexp_close_fexp_wrt_fexp_rec : lngen.
+#[export] Hint Rewrite ftvar_in_fexp_close_fexp_wrt_fexp_rec using solve [auto] : lngen.
 
 (* end hide *)
 
 (* begin hide *)
 
-Lemma fv_fexp_in_fexp_close_fexp_wrt_ftyp_rec_mutual :
+Lemma fvar_in_fexp_close_fexp_wrt_ftyp_rec_mutual :
 (forall e1 X1 n1,
-  fv_fexp_in_fexp (close_fexp_wrt_ftyp_rec n1 X1 e1) [=] fv_fexp_in_fexp e1).
+  fvar_in_fexp (close_fexp_wrt_ftyp_rec n1 X1 e1) [=] fvar_in_fexp e1).
 Proof.
 apply_mutual_ind fexp_mutind;
 default_simp; fsetdec.
@@ -3682,23 +3682,23 @@ Qed.
 
 (* begin hide *)
 
-Lemma fv_fexp_in_fexp_close_fexp_wrt_ftyp_rec :
+Lemma fvar_in_fexp_close_fexp_wrt_ftyp_rec :
 forall e1 X1 n1,
-  fv_fexp_in_fexp (close_fexp_wrt_ftyp_rec n1 X1 e1) [=] fv_fexp_in_fexp e1.
+  fvar_in_fexp (close_fexp_wrt_ftyp_rec n1 X1 e1) [=] fvar_in_fexp e1.
 Proof.
-pose proof fv_fexp_in_fexp_close_fexp_wrt_ftyp_rec_mutual as H; intuition eauto.
+pose proof fvar_in_fexp_close_fexp_wrt_ftyp_rec_mutual as H; intuition eauto.
 Qed.
 
-#[export] Hint Resolve fv_fexp_in_fexp_close_fexp_wrt_ftyp_rec : lngen.
-#[export] Hint Rewrite fv_fexp_in_fexp_close_fexp_wrt_ftyp_rec using solve [auto] : lngen.
+#[export] Hint Resolve fvar_in_fexp_close_fexp_wrt_ftyp_rec : lngen.
+#[export] Hint Rewrite fvar_in_fexp_close_fexp_wrt_ftyp_rec using solve [auto] : lngen.
 
 (* end hide *)
 
 (* begin hide *)
 
-Lemma fv_fexp_in_fexp_close_fexp_wrt_fexp_rec_mutual :
+Lemma fvar_in_fexp_close_fexp_wrt_fexp_rec_mutual :
 (forall e1 x1 n1,
-  fv_fexp_in_fexp (close_fexp_wrt_fexp_rec n1 x1 e1) [=] remove x1 (fv_fexp_in_fexp e1)).
+  fvar_in_fexp (close_fexp_wrt_fexp_rec n1 x1 e1) [=] remove x1 (fvar_in_fexp e1)).
 Proof.
 apply_mutual_ind fexp_mutind;
 default_simp; fsetdec.
@@ -3708,23 +3708,23 @@ Qed.
 
 (* begin hide *)
 
-Lemma fv_fexp_in_fexp_close_fexp_wrt_fexp_rec :
+Lemma fvar_in_fexp_close_fexp_wrt_fexp_rec :
 forall e1 x1 n1,
-  fv_fexp_in_fexp (close_fexp_wrt_fexp_rec n1 x1 e1) [=] remove x1 (fv_fexp_in_fexp e1).
+  fvar_in_fexp (close_fexp_wrt_fexp_rec n1 x1 e1) [=] remove x1 (fvar_in_fexp e1).
 Proof.
-pose proof fv_fexp_in_fexp_close_fexp_wrt_fexp_rec_mutual as H; intuition eauto.
+pose proof fvar_in_fexp_close_fexp_wrt_fexp_rec_mutual as H; intuition eauto.
 Qed.
 
-#[export] Hint Resolve fv_fexp_in_fexp_close_fexp_wrt_fexp_rec : lngen.
-#[export] Hint Rewrite fv_fexp_in_fexp_close_fexp_wrt_fexp_rec using solve [auto] : lngen.
+#[export] Hint Resolve fvar_in_fexp_close_fexp_wrt_fexp_rec : lngen.
+#[export] Hint Rewrite fvar_in_fexp_close_fexp_wrt_fexp_rec using solve [auto] : lngen.
 
 (* end hide *)
 
 (* begin hide *)
 
-Lemma fv_ftyp_in_fbind_close_fbind_wrt_ftyp_rec_mutual :
+Lemma ftvar_in_fbind_close_fbind_wrt_ftyp_rec_mutual :
 (forall fb1 X1 n1,
-  fv_ftyp_in_fbind (close_fbind_wrt_ftyp_rec n1 X1 fb1) [=] remove X1 (fv_ftyp_in_fbind fb1)).
+  ftvar_in_fbind (close_fbind_wrt_ftyp_rec n1 X1 fb1) [=] remove X1 (ftvar_in_fbind fb1)).
 Proof.
 apply_mutual_ind fbind_mutind;
 default_simp; fsetdec.
@@ -3734,83 +3734,83 @@ Qed.
 
 (* begin hide *)
 
-Lemma fv_ftyp_in_fbind_close_fbind_wrt_ftyp_rec :
+Lemma ftvar_in_fbind_close_fbind_wrt_ftyp_rec :
 forall fb1 X1 n1,
-  fv_ftyp_in_fbind (close_fbind_wrt_ftyp_rec n1 X1 fb1) [=] remove X1 (fv_ftyp_in_fbind fb1).
+  ftvar_in_fbind (close_fbind_wrt_ftyp_rec n1 X1 fb1) [=] remove X1 (ftvar_in_fbind fb1).
 Proof.
-pose proof fv_ftyp_in_fbind_close_fbind_wrt_ftyp_rec_mutual as H; intuition eauto.
+pose proof ftvar_in_fbind_close_fbind_wrt_ftyp_rec_mutual as H; intuition eauto.
 Qed.
 
-#[export] Hint Resolve fv_ftyp_in_fbind_close_fbind_wrt_ftyp_rec : lngen.
-#[export] Hint Rewrite fv_ftyp_in_fbind_close_fbind_wrt_ftyp_rec using solve [auto] : lngen.
+#[export] Hint Resolve ftvar_in_fbind_close_fbind_wrt_ftyp_rec : lngen.
+#[export] Hint Rewrite ftvar_in_fbind_close_fbind_wrt_ftyp_rec using solve [auto] : lngen.
 
 (* end hide *)
 
-Lemma fv_ftyp_in_ftyp_close_ftyp_wrt_ftyp :
+Lemma ftvar_in_ftyp_close_ftyp_wrt_ftyp :
 forall A1 X1,
-  fv_ftyp_in_ftyp (close_ftyp_wrt_ftyp X1 A1) [=] remove X1 (fv_ftyp_in_ftyp A1).
+  ftvar_in_ftyp (close_ftyp_wrt_ftyp X1 A1) [=] remove X1 (ftvar_in_ftyp A1).
 Proof.
 unfold close_ftyp_wrt_ftyp; default_simp.
 Qed.
 
-#[export] Hint Resolve fv_ftyp_in_ftyp_close_ftyp_wrt_ftyp : lngen.
-#[export] Hint Rewrite fv_ftyp_in_ftyp_close_ftyp_wrt_ftyp using solve [auto] : lngen.
+#[export] Hint Resolve ftvar_in_ftyp_close_ftyp_wrt_ftyp : lngen.
+#[export] Hint Rewrite ftvar_in_ftyp_close_ftyp_wrt_ftyp using solve [auto] : lngen.
 
-Lemma fv_ftyp_in_fexp_close_fexp_wrt_ftyp :
+Lemma ftvar_in_fexp_close_fexp_wrt_ftyp :
 forall e1 X1,
-  fv_ftyp_in_fexp (close_fexp_wrt_ftyp X1 e1) [=] remove X1 (fv_ftyp_in_fexp e1).
+  ftvar_in_fexp (close_fexp_wrt_ftyp X1 e1) [=] remove X1 (ftvar_in_fexp e1).
 Proof.
 unfold close_fexp_wrt_ftyp; default_simp.
 Qed.
 
-#[export] Hint Resolve fv_ftyp_in_fexp_close_fexp_wrt_ftyp : lngen.
-#[export] Hint Rewrite fv_ftyp_in_fexp_close_fexp_wrt_ftyp using solve [auto] : lngen.
+#[export] Hint Resolve ftvar_in_fexp_close_fexp_wrt_ftyp : lngen.
+#[export] Hint Rewrite ftvar_in_fexp_close_fexp_wrt_ftyp using solve [auto] : lngen.
 
-Lemma fv_ftyp_in_fexp_close_fexp_wrt_fexp :
+Lemma ftvar_in_fexp_close_fexp_wrt_fexp :
 forall e1 x1,
-  fv_ftyp_in_fexp (close_fexp_wrt_fexp x1 e1) [=] fv_ftyp_in_fexp e1.
+  ftvar_in_fexp (close_fexp_wrt_fexp x1 e1) [=] ftvar_in_fexp e1.
 Proof.
 unfold close_fexp_wrt_fexp; default_simp.
 Qed.
 
-#[export] Hint Resolve fv_ftyp_in_fexp_close_fexp_wrt_fexp : lngen.
-#[export] Hint Rewrite fv_ftyp_in_fexp_close_fexp_wrt_fexp using solve [auto] : lngen.
+#[export] Hint Resolve ftvar_in_fexp_close_fexp_wrt_fexp : lngen.
+#[export] Hint Rewrite ftvar_in_fexp_close_fexp_wrt_fexp using solve [auto] : lngen.
 
-Lemma fv_fexp_in_fexp_close_fexp_wrt_ftyp :
+Lemma fvar_in_fexp_close_fexp_wrt_ftyp :
 forall e1 X1,
-  fv_fexp_in_fexp (close_fexp_wrt_ftyp X1 e1) [=] fv_fexp_in_fexp e1.
+  fvar_in_fexp (close_fexp_wrt_ftyp X1 e1) [=] fvar_in_fexp e1.
 Proof.
 unfold close_fexp_wrt_ftyp; default_simp.
 Qed.
 
-#[export] Hint Resolve fv_fexp_in_fexp_close_fexp_wrt_ftyp : lngen.
-#[export] Hint Rewrite fv_fexp_in_fexp_close_fexp_wrt_ftyp using solve [auto] : lngen.
+#[export] Hint Resolve fvar_in_fexp_close_fexp_wrt_ftyp : lngen.
+#[export] Hint Rewrite fvar_in_fexp_close_fexp_wrt_ftyp using solve [auto] : lngen.
 
-Lemma fv_fexp_in_fexp_close_fexp_wrt_fexp :
+Lemma fvar_in_fexp_close_fexp_wrt_fexp :
 forall e1 x1,
-  fv_fexp_in_fexp (close_fexp_wrt_fexp x1 e1) [=] remove x1 (fv_fexp_in_fexp e1).
+  fvar_in_fexp (close_fexp_wrt_fexp x1 e1) [=] remove x1 (fvar_in_fexp e1).
 Proof.
 unfold close_fexp_wrt_fexp; default_simp.
 Qed.
 
-#[export] Hint Resolve fv_fexp_in_fexp_close_fexp_wrt_fexp : lngen.
-#[export] Hint Rewrite fv_fexp_in_fexp_close_fexp_wrt_fexp using solve [auto] : lngen.
+#[export] Hint Resolve fvar_in_fexp_close_fexp_wrt_fexp : lngen.
+#[export] Hint Rewrite fvar_in_fexp_close_fexp_wrt_fexp using solve [auto] : lngen.
 
-Lemma fv_ftyp_in_fbind_close_fbind_wrt_ftyp :
+Lemma ftvar_in_fbind_close_fbind_wrt_ftyp :
 forall fb1 X1,
-  fv_ftyp_in_fbind (close_fbind_wrt_ftyp X1 fb1) [=] remove X1 (fv_ftyp_in_fbind fb1).
+  ftvar_in_fbind (close_fbind_wrt_ftyp X1 fb1) [=] remove X1 (ftvar_in_fbind fb1).
 Proof.
 unfold close_fbind_wrt_ftyp; default_simp.
 Qed.
 
-#[export] Hint Resolve fv_ftyp_in_fbind_close_fbind_wrt_ftyp : lngen.
-#[export] Hint Rewrite fv_ftyp_in_fbind_close_fbind_wrt_ftyp using solve [auto] : lngen.
+#[export] Hint Resolve ftvar_in_fbind_close_fbind_wrt_ftyp : lngen.
+#[export] Hint Rewrite ftvar_in_fbind_close_fbind_wrt_ftyp using solve [auto] : lngen.
 
 (* begin hide *)
 
-Lemma fv_ftyp_in_ftyp_open_ftyp_wrt_ftyp_rec_lower_mutual :
+Lemma ftvar_in_ftyp_open_ftyp_wrt_ftyp_rec_lower_mutual :
 (forall A1 A2 n1,
-  fv_ftyp_in_ftyp A1 [<=] fv_ftyp_in_ftyp (open_ftyp_wrt_ftyp_rec n1 A2 A1)).
+  ftvar_in_ftyp A1 [<=] ftvar_in_ftyp (open_ftyp_wrt_ftyp_rec n1 A2 A1)).
 Proof.
 apply_mutual_ind ftyp_mutind;
 default_simp; fsetdec.
@@ -3820,22 +3820,22 @@ Qed.
 
 (* begin hide *)
 
-Lemma fv_ftyp_in_ftyp_open_ftyp_wrt_ftyp_rec_lower :
+Lemma ftvar_in_ftyp_open_ftyp_wrt_ftyp_rec_lower :
 forall A1 A2 n1,
-  fv_ftyp_in_ftyp A1 [<=] fv_ftyp_in_ftyp (open_ftyp_wrt_ftyp_rec n1 A2 A1).
+  ftvar_in_ftyp A1 [<=] ftvar_in_ftyp (open_ftyp_wrt_ftyp_rec n1 A2 A1).
 Proof.
-pose proof fv_ftyp_in_ftyp_open_ftyp_wrt_ftyp_rec_lower_mutual as H; intuition eauto.
+pose proof ftvar_in_ftyp_open_ftyp_wrt_ftyp_rec_lower_mutual as H; intuition eauto.
 Qed.
 
-#[export] Hint Resolve fv_ftyp_in_ftyp_open_ftyp_wrt_ftyp_rec_lower : lngen.
+#[export] Hint Resolve ftvar_in_ftyp_open_ftyp_wrt_ftyp_rec_lower : lngen.
 
 (* end hide *)
 
 (* begin hide *)
 
-Lemma fv_ftyp_in_fexp_open_fexp_wrt_ftyp_rec_lower_mutual :
+Lemma ftvar_in_fexp_open_fexp_wrt_ftyp_rec_lower_mutual :
 (forall e1 A1 n1,
-  fv_ftyp_in_fexp e1 [<=] fv_ftyp_in_fexp (open_fexp_wrt_ftyp_rec n1 A1 e1)).
+  ftvar_in_fexp e1 [<=] ftvar_in_fexp (open_fexp_wrt_ftyp_rec n1 A1 e1)).
 Proof.
 apply_mutual_ind fexp_mutind;
 default_simp; fsetdec.
@@ -3845,22 +3845,22 @@ Qed.
 
 (* begin hide *)
 
-Lemma fv_ftyp_in_fexp_open_fexp_wrt_ftyp_rec_lower :
+Lemma ftvar_in_fexp_open_fexp_wrt_ftyp_rec_lower :
 forall e1 A1 n1,
-  fv_ftyp_in_fexp e1 [<=] fv_ftyp_in_fexp (open_fexp_wrt_ftyp_rec n1 A1 e1).
+  ftvar_in_fexp e1 [<=] ftvar_in_fexp (open_fexp_wrt_ftyp_rec n1 A1 e1).
 Proof.
-pose proof fv_ftyp_in_fexp_open_fexp_wrt_ftyp_rec_lower_mutual as H; intuition eauto.
+pose proof ftvar_in_fexp_open_fexp_wrt_ftyp_rec_lower_mutual as H; intuition eauto.
 Qed.
 
-#[export] Hint Resolve fv_ftyp_in_fexp_open_fexp_wrt_ftyp_rec_lower : lngen.
+#[export] Hint Resolve ftvar_in_fexp_open_fexp_wrt_ftyp_rec_lower : lngen.
 
 (* end hide *)
 
 (* begin hide *)
 
-Lemma fv_ftyp_in_fexp_open_fexp_wrt_fexp_rec_lower_mutual :
+Lemma ftvar_in_fexp_open_fexp_wrt_fexp_rec_lower_mutual :
 (forall e1 e2 n1,
-  fv_ftyp_in_fexp e1 [<=] fv_ftyp_in_fexp (open_fexp_wrt_fexp_rec n1 e2 e1)).
+  ftvar_in_fexp e1 [<=] ftvar_in_fexp (open_fexp_wrt_fexp_rec n1 e2 e1)).
 Proof.
 apply_mutual_ind fexp_mutind;
 default_simp; fsetdec.
@@ -3870,22 +3870,22 @@ Qed.
 
 (* begin hide *)
 
-Lemma fv_ftyp_in_fexp_open_fexp_wrt_fexp_rec_lower :
+Lemma ftvar_in_fexp_open_fexp_wrt_fexp_rec_lower :
 forall e1 e2 n1,
-  fv_ftyp_in_fexp e1 [<=] fv_ftyp_in_fexp (open_fexp_wrt_fexp_rec n1 e2 e1).
+  ftvar_in_fexp e1 [<=] ftvar_in_fexp (open_fexp_wrt_fexp_rec n1 e2 e1).
 Proof.
-pose proof fv_ftyp_in_fexp_open_fexp_wrt_fexp_rec_lower_mutual as H; intuition eauto.
+pose proof ftvar_in_fexp_open_fexp_wrt_fexp_rec_lower_mutual as H; intuition eauto.
 Qed.
 
-#[export] Hint Resolve fv_ftyp_in_fexp_open_fexp_wrt_fexp_rec_lower : lngen.
+#[export] Hint Resolve ftvar_in_fexp_open_fexp_wrt_fexp_rec_lower : lngen.
 
 (* end hide *)
 
 (* begin hide *)
 
-Lemma fv_fexp_in_fexp_open_fexp_wrt_ftyp_rec_lower_mutual :
+Lemma fvar_in_fexp_open_fexp_wrt_ftyp_rec_lower_mutual :
 (forall e1 A1 n1,
-  fv_fexp_in_fexp e1 [<=] fv_fexp_in_fexp (open_fexp_wrt_ftyp_rec n1 A1 e1)).
+  fvar_in_fexp e1 [<=] fvar_in_fexp (open_fexp_wrt_ftyp_rec n1 A1 e1)).
 Proof.
 apply_mutual_ind fexp_mutind;
 default_simp; fsetdec.
@@ -3895,22 +3895,22 @@ Qed.
 
 (* begin hide *)
 
-Lemma fv_fexp_in_fexp_open_fexp_wrt_ftyp_rec_lower :
+Lemma fvar_in_fexp_open_fexp_wrt_ftyp_rec_lower :
 forall e1 A1 n1,
-  fv_fexp_in_fexp e1 [<=] fv_fexp_in_fexp (open_fexp_wrt_ftyp_rec n1 A1 e1).
+  fvar_in_fexp e1 [<=] fvar_in_fexp (open_fexp_wrt_ftyp_rec n1 A1 e1).
 Proof.
-pose proof fv_fexp_in_fexp_open_fexp_wrt_ftyp_rec_lower_mutual as H; intuition eauto.
+pose proof fvar_in_fexp_open_fexp_wrt_ftyp_rec_lower_mutual as H; intuition eauto.
 Qed.
 
-#[export] Hint Resolve fv_fexp_in_fexp_open_fexp_wrt_ftyp_rec_lower : lngen.
+#[export] Hint Resolve fvar_in_fexp_open_fexp_wrt_ftyp_rec_lower : lngen.
 
 (* end hide *)
 
 (* begin hide *)
 
-Lemma fv_fexp_in_fexp_open_fexp_wrt_fexp_rec_lower_mutual :
+Lemma fvar_in_fexp_open_fexp_wrt_fexp_rec_lower_mutual :
 (forall e1 e2 n1,
-  fv_fexp_in_fexp e1 [<=] fv_fexp_in_fexp (open_fexp_wrt_fexp_rec n1 e2 e1)).
+  fvar_in_fexp e1 [<=] fvar_in_fexp (open_fexp_wrt_fexp_rec n1 e2 e1)).
 Proof.
 apply_mutual_ind fexp_mutind;
 default_simp; fsetdec.
@@ -3920,22 +3920,22 @@ Qed.
 
 (* begin hide *)
 
-Lemma fv_fexp_in_fexp_open_fexp_wrt_fexp_rec_lower :
+Lemma fvar_in_fexp_open_fexp_wrt_fexp_rec_lower :
 forall e1 e2 n1,
-  fv_fexp_in_fexp e1 [<=] fv_fexp_in_fexp (open_fexp_wrt_fexp_rec n1 e2 e1).
+  fvar_in_fexp e1 [<=] fvar_in_fexp (open_fexp_wrt_fexp_rec n1 e2 e1).
 Proof.
-pose proof fv_fexp_in_fexp_open_fexp_wrt_fexp_rec_lower_mutual as H; intuition eauto.
+pose proof fvar_in_fexp_open_fexp_wrt_fexp_rec_lower_mutual as H; intuition eauto.
 Qed.
 
-#[export] Hint Resolve fv_fexp_in_fexp_open_fexp_wrt_fexp_rec_lower : lngen.
+#[export] Hint Resolve fvar_in_fexp_open_fexp_wrt_fexp_rec_lower : lngen.
 
 (* end hide *)
 
 (* begin hide *)
 
-Lemma fv_ftyp_in_fbind_open_fbind_wrt_ftyp_rec_lower_mutual :
+Lemma ftvar_in_fbind_open_fbind_wrt_ftyp_rec_lower_mutual :
 (forall fb1 A1 n1,
-  fv_ftyp_in_fbind fb1 [<=] fv_ftyp_in_fbind (open_fbind_wrt_ftyp_rec n1 A1 fb1)).
+  ftvar_in_fbind fb1 [<=] ftvar_in_fbind (open_fbind_wrt_ftyp_rec n1 A1 fb1)).
 Proof.
 apply_mutual_ind fbind_mutind;
 default_simp; fsetdec.
@@ -3945,76 +3945,76 @@ Qed.
 
 (* begin hide *)
 
-Lemma fv_ftyp_in_fbind_open_fbind_wrt_ftyp_rec_lower :
+Lemma ftvar_in_fbind_open_fbind_wrt_ftyp_rec_lower :
 forall fb1 A1 n1,
-  fv_ftyp_in_fbind fb1 [<=] fv_ftyp_in_fbind (open_fbind_wrt_ftyp_rec n1 A1 fb1).
+  ftvar_in_fbind fb1 [<=] ftvar_in_fbind (open_fbind_wrt_ftyp_rec n1 A1 fb1).
 Proof.
-pose proof fv_ftyp_in_fbind_open_fbind_wrt_ftyp_rec_lower_mutual as H; intuition eauto.
+pose proof ftvar_in_fbind_open_fbind_wrt_ftyp_rec_lower_mutual as H; intuition eauto.
 Qed.
 
-#[export] Hint Resolve fv_ftyp_in_fbind_open_fbind_wrt_ftyp_rec_lower : lngen.
+#[export] Hint Resolve ftvar_in_fbind_open_fbind_wrt_ftyp_rec_lower : lngen.
 
 (* end hide *)
 
-Lemma fv_ftyp_in_ftyp_open_ftyp_wrt_ftyp_lower :
+Lemma ftvar_in_ftyp_open_ftyp_wrt_ftyp_lower :
 forall A1 A2,
-  fv_ftyp_in_ftyp A1 [<=] fv_ftyp_in_ftyp (open_ftyp_wrt_ftyp A1 A2).
+  ftvar_in_ftyp A1 [<=] ftvar_in_ftyp (open_ftyp_wrt_ftyp A1 A2).
 Proof.
 unfold open_ftyp_wrt_ftyp; default_simp.
 Qed.
 
-#[export] Hint Resolve fv_ftyp_in_ftyp_open_ftyp_wrt_ftyp_lower : lngen.
+#[export] Hint Resolve ftvar_in_ftyp_open_ftyp_wrt_ftyp_lower : lngen.
 
-Lemma fv_ftyp_in_fexp_open_fexp_wrt_ftyp_lower :
+Lemma ftvar_in_fexp_open_fexp_wrt_ftyp_lower :
 forall e1 A1,
-  fv_ftyp_in_fexp e1 [<=] fv_ftyp_in_fexp (open_fexp_wrt_ftyp e1 A1).
+  ftvar_in_fexp e1 [<=] ftvar_in_fexp (open_fexp_wrt_ftyp e1 A1).
 Proof.
 unfold open_fexp_wrt_ftyp; default_simp.
 Qed.
 
-#[export] Hint Resolve fv_ftyp_in_fexp_open_fexp_wrt_ftyp_lower : lngen.
+#[export] Hint Resolve ftvar_in_fexp_open_fexp_wrt_ftyp_lower : lngen.
 
-Lemma fv_ftyp_in_fexp_open_fexp_wrt_fexp_lower :
+Lemma ftvar_in_fexp_open_fexp_wrt_fexp_lower :
 forall e1 e2,
-  fv_ftyp_in_fexp e1 [<=] fv_ftyp_in_fexp (open_fexp_wrt_fexp e1 e2).
+  ftvar_in_fexp e1 [<=] ftvar_in_fexp (open_fexp_wrt_fexp e1 e2).
 Proof.
 unfold open_fexp_wrt_fexp; default_simp.
 Qed.
 
-#[export] Hint Resolve fv_ftyp_in_fexp_open_fexp_wrt_fexp_lower : lngen.
+#[export] Hint Resolve ftvar_in_fexp_open_fexp_wrt_fexp_lower : lngen.
 
-Lemma fv_fexp_in_fexp_open_fexp_wrt_ftyp_lower :
+Lemma fvar_in_fexp_open_fexp_wrt_ftyp_lower :
 forall e1 A1,
-  fv_fexp_in_fexp e1 [<=] fv_fexp_in_fexp (open_fexp_wrt_ftyp e1 A1).
+  fvar_in_fexp e1 [<=] fvar_in_fexp (open_fexp_wrt_ftyp e1 A1).
 Proof.
 unfold open_fexp_wrt_ftyp; default_simp.
 Qed.
 
-#[export] Hint Resolve fv_fexp_in_fexp_open_fexp_wrt_ftyp_lower : lngen.
+#[export] Hint Resolve fvar_in_fexp_open_fexp_wrt_ftyp_lower : lngen.
 
-Lemma fv_fexp_in_fexp_open_fexp_wrt_fexp_lower :
+Lemma fvar_in_fexp_open_fexp_wrt_fexp_lower :
 forall e1 e2,
-  fv_fexp_in_fexp e1 [<=] fv_fexp_in_fexp (open_fexp_wrt_fexp e1 e2).
+  fvar_in_fexp e1 [<=] fvar_in_fexp (open_fexp_wrt_fexp e1 e2).
 Proof.
 unfold open_fexp_wrt_fexp; default_simp.
 Qed.
 
-#[export] Hint Resolve fv_fexp_in_fexp_open_fexp_wrt_fexp_lower : lngen.
+#[export] Hint Resolve fvar_in_fexp_open_fexp_wrt_fexp_lower : lngen.
 
-Lemma fv_ftyp_in_fbind_open_fbind_wrt_ftyp_lower :
+Lemma ftvar_in_fbind_open_fbind_wrt_ftyp_lower :
 forall fb1 A1,
-  fv_ftyp_in_fbind fb1 [<=] fv_ftyp_in_fbind (open_fbind_wrt_ftyp fb1 A1).
+  ftvar_in_fbind fb1 [<=] ftvar_in_fbind (open_fbind_wrt_ftyp fb1 A1).
 Proof.
 unfold open_fbind_wrt_ftyp; default_simp.
 Qed.
 
-#[export] Hint Resolve fv_ftyp_in_fbind_open_fbind_wrt_ftyp_lower : lngen.
+#[export] Hint Resolve ftvar_in_fbind_open_fbind_wrt_ftyp_lower : lngen.
 
 (* begin hide *)
 
-Lemma fv_ftyp_in_ftyp_open_ftyp_wrt_ftyp_rec_upper_mutual :
+Lemma ftvar_in_ftyp_open_ftyp_wrt_ftyp_rec_upper_mutual :
 (forall A1 A2 n1,
-  fv_ftyp_in_ftyp (open_ftyp_wrt_ftyp_rec n1 A2 A1) [<=] fv_ftyp_in_ftyp A2 `union` fv_ftyp_in_ftyp A1).
+  ftvar_in_ftyp (open_ftyp_wrt_ftyp_rec n1 A2 A1) [<=] ftvar_in_ftyp A2 `union` ftvar_in_ftyp A1).
 Proof.
 apply_mutual_ind ftyp_mutind;
 default_simp; fsetdec.
@@ -4024,22 +4024,22 @@ Qed.
 
 (* begin hide *)
 
-Lemma fv_ftyp_in_ftyp_open_ftyp_wrt_ftyp_rec_upper :
+Lemma ftvar_in_ftyp_open_ftyp_wrt_ftyp_rec_upper :
 forall A1 A2 n1,
-  fv_ftyp_in_ftyp (open_ftyp_wrt_ftyp_rec n1 A2 A1) [<=] fv_ftyp_in_ftyp A2 `union` fv_ftyp_in_ftyp A1.
+  ftvar_in_ftyp (open_ftyp_wrt_ftyp_rec n1 A2 A1) [<=] ftvar_in_ftyp A2 `union` ftvar_in_ftyp A1.
 Proof.
-pose proof fv_ftyp_in_ftyp_open_ftyp_wrt_ftyp_rec_upper_mutual as H; intuition eauto.
+pose proof ftvar_in_ftyp_open_ftyp_wrt_ftyp_rec_upper_mutual as H; intuition eauto.
 Qed.
 
-#[export] Hint Resolve fv_ftyp_in_ftyp_open_ftyp_wrt_ftyp_rec_upper : lngen.
+#[export] Hint Resolve ftvar_in_ftyp_open_ftyp_wrt_ftyp_rec_upper : lngen.
 
 (* end hide *)
 
 (* begin hide *)
 
-Lemma fv_ftyp_in_fexp_open_fexp_wrt_ftyp_rec_upper_mutual :
+Lemma ftvar_in_fexp_open_fexp_wrt_ftyp_rec_upper_mutual :
 (forall e1 A1 n1,
-  fv_ftyp_in_fexp (open_fexp_wrt_ftyp_rec n1 A1 e1) [<=] fv_ftyp_in_ftyp A1 `union` fv_ftyp_in_fexp e1).
+  ftvar_in_fexp (open_fexp_wrt_ftyp_rec n1 A1 e1) [<=] ftvar_in_ftyp A1 `union` ftvar_in_fexp e1).
 Proof.
 apply_mutual_ind fexp_mutind;
 default_simp; fsetdec.
@@ -4049,22 +4049,22 @@ Qed.
 
 (* begin hide *)
 
-Lemma fv_ftyp_in_fexp_open_fexp_wrt_ftyp_rec_upper :
+Lemma ftvar_in_fexp_open_fexp_wrt_ftyp_rec_upper :
 forall e1 A1 n1,
-  fv_ftyp_in_fexp (open_fexp_wrt_ftyp_rec n1 A1 e1) [<=] fv_ftyp_in_ftyp A1 `union` fv_ftyp_in_fexp e1.
+  ftvar_in_fexp (open_fexp_wrt_ftyp_rec n1 A1 e1) [<=] ftvar_in_ftyp A1 `union` ftvar_in_fexp e1.
 Proof.
-pose proof fv_ftyp_in_fexp_open_fexp_wrt_ftyp_rec_upper_mutual as H; intuition eauto.
+pose proof ftvar_in_fexp_open_fexp_wrt_ftyp_rec_upper_mutual as H; intuition eauto.
 Qed.
 
-#[export] Hint Resolve fv_ftyp_in_fexp_open_fexp_wrt_ftyp_rec_upper : lngen.
+#[export] Hint Resolve ftvar_in_fexp_open_fexp_wrt_ftyp_rec_upper : lngen.
 
 (* end hide *)
 
 (* begin hide *)
 
-Lemma fv_ftyp_in_fexp_open_fexp_wrt_fexp_rec_upper_mutual :
+Lemma ftvar_in_fexp_open_fexp_wrt_fexp_rec_upper_mutual :
 (forall e1 e2 n1,
-  fv_ftyp_in_fexp (open_fexp_wrt_fexp_rec n1 e2 e1) [<=] fv_ftyp_in_fexp e2 `union` fv_ftyp_in_fexp e1).
+  ftvar_in_fexp (open_fexp_wrt_fexp_rec n1 e2 e1) [<=] ftvar_in_fexp e2 `union` ftvar_in_fexp e1).
 Proof.
 apply_mutual_ind fexp_mutind;
 default_simp; fsetdec.
@@ -4074,22 +4074,22 @@ Qed.
 
 (* begin hide *)
 
-Lemma fv_ftyp_in_fexp_open_fexp_wrt_fexp_rec_upper :
+Lemma ftvar_in_fexp_open_fexp_wrt_fexp_rec_upper :
 forall e1 e2 n1,
-  fv_ftyp_in_fexp (open_fexp_wrt_fexp_rec n1 e2 e1) [<=] fv_ftyp_in_fexp e2 `union` fv_ftyp_in_fexp e1.
+  ftvar_in_fexp (open_fexp_wrt_fexp_rec n1 e2 e1) [<=] ftvar_in_fexp e2 `union` ftvar_in_fexp e1.
 Proof.
-pose proof fv_ftyp_in_fexp_open_fexp_wrt_fexp_rec_upper_mutual as H; intuition eauto.
+pose proof ftvar_in_fexp_open_fexp_wrt_fexp_rec_upper_mutual as H; intuition eauto.
 Qed.
 
-#[export] Hint Resolve fv_ftyp_in_fexp_open_fexp_wrt_fexp_rec_upper : lngen.
+#[export] Hint Resolve ftvar_in_fexp_open_fexp_wrt_fexp_rec_upper : lngen.
 
 (* end hide *)
 
 (* begin hide *)
 
-Lemma fv_fexp_in_fexp_open_fexp_wrt_ftyp_rec_upper_mutual :
+Lemma fvar_in_fexp_open_fexp_wrt_ftyp_rec_upper_mutual :
 (forall e1 A1 n1,
-  fv_fexp_in_fexp (open_fexp_wrt_ftyp_rec n1 A1 e1) [<=] fv_fexp_in_fexp e1).
+  fvar_in_fexp (open_fexp_wrt_ftyp_rec n1 A1 e1) [<=] fvar_in_fexp e1).
 Proof.
 apply_mutual_ind fexp_mutind;
 default_simp; fsetdec.
@@ -4099,22 +4099,22 @@ Qed.
 
 (* begin hide *)
 
-Lemma fv_fexp_in_fexp_open_fexp_wrt_ftyp_rec_upper :
+Lemma fvar_in_fexp_open_fexp_wrt_ftyp_rec_upper :
 forall e1 A1 n1,
-  fv_fexp_in_fexp (open_fexp_wrt_ftyp_rec n1 A1 e1) [<=] fv_fexp_in_fexp e1.
+  fvar_in_fexp (open_fexp_wrt_ftyp_rec n1 A1 e1) [<=] fvar_in_fexp e1.
 Proof.
-pose proof fv_fexp_in_fexp_open_fexp_wrt_ftyp_rec_upper_mutual as H; intuition eauto.
+pose proof fvar_in_fexp_open_fexp_wrt_ftyp_rec_upper_mutual as H; intuition eauto.
 Qed.
 
-#[export] Hint Resolve fv_fexp_in_fexp_open_fexp_wrt_ftyp_rec_upper : lngen.
+#[export] Hint Resolve fvar_in_fexp_open_fexp_wrt_ftyp_rec_upper : lngen.
 
 (* end hide *)
 
 (* begin hide *)
 
-Lemma fv_fexp_in_fexp_open_fexp_wrt_fexp_rec_upper_mutual :
+Lemma fvar_in_fexp_open_fexp_wrt_fexp_rec_upper_mutual :
 (forall e1 e2 n1,
-  fv_fexp_in_fexp (open_fexp_wrt_fexp_rec n1 e2 e1) [<=] fv_fexp_in_fexp e2 `union` fv_fexp_in_fexp e1).
+  fvar_in_fexp (open_fexp_wrt_fexp_rec n1 e2 e1) [<=] fvar_in_fexp e2 `union` fvar_in_fexp e1).
 Proof.
 apply_mutual_ind fexp_mutind;
 default_simp; fsetdec.
@@ -4124,22 +4124,22 @@ Qed.
 
 (* begin hide *)
 
-Lemma fv_fexp_in_fexp_open_fexp_wrt_fexp_rec_upper :
+Lemma fvar_in_fexp_open_fexp_wrt_fexp_rec_upper :
 forall e1 e2 n1,
-  fv_fexp_in_fexp (open_fexp_wrt_fexp_rec n1 e2 e1) [<=] fv_fexp_in_fexp e2 `union` fv_fexp_in_fexp e1.
+  fvar_in_fexp (open_fexp_wrt_fexp_rec n1 e2 e1) [<=] fvar_in_fexp e2 `union` fvar_in_fexp e1.
 Proof.
-pose proof fv_fexp_in_fexp_open_fexp_wrt_fexp_rec_upper_mutual as H; intuition eauto.
+pose proof fvar_in_fexp_open_fexp_wrt_fexp_rec_upper_mutual as H; intuition eauto.
 Qed.
 
-#[export] Hint Resolve fv_fexp_in_fexp_open_fexp_wrt_fexp_rec_upper : lngen.
+#[export] Hint Resolve fvar_in_fexp_open_fexp_wrt_fexp_rec_upper : lngen.
 
 (* end hide *)
 
 (* begin hide *)
 
-Lemma fv_ftyp_in_fbind_open_fbind_wrt_ftyp_rec_upper_mutual :
+Lemma ftvar_in_fbind_open_fbind_wrt_ftyp_rec_upper_mutual :
 (forall fb1 A1 n1,
-  fv_ftyp_in_fbind (open_fbind_wrt_ftyp_rec n1 A1 fb1) [<=] fv_ftyp_in_ftyp A1 `union` fv_ftyp_in_fbind fb1).
+  ftvar_in_fbind (open_fbind_wrt_ftyp_rec n1 A1 fb1) [<=] ftvar_in_ftyp A1 `union` ftvar_in_fbind fb1).
 Proof.
 apply_mutual_ind fbind_mutind;
 default_simp; fsetdec.
@@ -4149,77 +4149,77 @@ Qed.
 
 (* begin hide *)
 
-Lemma fv_ftyp_in_fbind_open_fbind_wrt_ftyp_rec_upper :
+Lemma ftvar_in_fbind_open_fbind_wrt_ftyp_rec_upper :
 forall fb1 A1 n1,
-  fv_ftyp_in_fbind (open_fbind_wrt_ftyp_rec n1 A1 fb1) [<=] fv_ftyp_in_ftyp A1 `union` fv_ftyp_in_fbind fb1.
+  ftvar_in_fbind (open_fbind_wrt_ftyp_rec n1 A1 fb1) [<=] ftvar_in_ftyp A1 `union` ftvar_in_fbind fb1.
 Proof.
-pose proof fv_ftyp_in_fbind_open_fbind_wrt_ftyp_rec_upper_mutual as H; intuition eauto.
+pose proof ftvar_in_fbind_open_fbind_wrt_ftyp_rec_upper_mutual as H; intuition eauto.
 Qed.
 
-#[export] Hint Resolve fv_ftyp_in_fbind_open_fbind_wrt_ftyp_rec_upper : lngen.
+#[export] Hint Resolve ftvar_in_fbind_open_fbind_wrt_ftyp_rec_upper : lngen.
 
 (* end hide *)
 
-Lemma fv_ftyp_in_ftyp_open_ftyp_wrt_ftyp_upper :
+Lemma ftvar_in_ftyp_open_ftyp_wrt_ftyp_upper :
 forall A1 A2,
-  fv_ftyp_in_ftyp (open_ftyp_wrt_ftyp A1 A2) [<=] fv_ftyp_in_ftyp A2 `union` fv_ftyp_in_ftyp A1.
+  ftvar_in_ftyp (open_ftyp_wrt_ftyp A1 A2) [<=] ftvar_in_ftyp A2 `union` ftvar_in_ftyp A1.
 Proof.
 unfold open_ftyp_wrt_ftyp; default_simp.
 Qed.
 
-#[export] Hint Resolve fv_ftyp_in_ftyp_open_ftyp_wrt_ftyp_upper : lngen.
+#[export] Hint Resolve ftvar_in_ftyp_open_ftyp_wrt_ftyp_upper : lngen.
 
-Lemma fv_ftyp_in_fexp_open_fexp_wrt_ftyp_upper :
+Lemma ftvar_in_fexp_open_fexp_wrt_ftyp_upper :
 forall e1 A1,
-  fv_ftyp_in_fexp (open_fexp_wrt_ftyp e1 A1) [<=] fv_ftyp_in_ftyp A1 `union` fv_ftyp_in_fexp e1.
+  ftvar_in_fexp (open_fexp_wrt_ftyp e1 A1) [<=] ftvar_in_ftyp A1 `union` ftvar_in_fexp e1.
 Proof.
 unfold open_fexp_wrt_ftyp; default_simp.
 Qed.
 
-#[export] Hint Resolve fv_ftyp_in_fexp_open_fexp_wrt_ftyp_upper : lngen.
+#[export] Hint Resolve ftvar_in_fexp_open_fexp_wrt_ftyp_upper : lngen.
 
-Lemma fv_ftyp_in_fexp_open_fexp_wrt_fexp_upper :
+Lemma ftvar_in_fexp_open_fexp_wrt_fexp_upper :
 forall e1 e2,
-  fv_ftyp_in_fexp (open_fexp_wrt_fexp e1 e2) [<=] fv_ftyp_in_fexp e2 `union` fv_ftyp_in_fexp e1.
+  ftvar_in_fexp (open_fexp_wrt_fexp e1 e2) [<=] ftvar_in_fexp e2 `union` ftvar_in_fexp e1.
 Proof.
 unfold open_fexp_wrt_fexp; default_simp.
 Qed.
 
-#[export] Hint Resolve fv_ftyp_in_fexp_open_fexp_wrt_fexp_upper : lngen.
+#[export] Hint Resolve ftvar_in_fexp_open_fexp_wrt_fexp_upper : lngen.
 
-Lemma fv_fexp_in_fexp_open_fexp_wrt_ftyp_upper :
+Lemma fvar_in_fexp_open_fexp_wrt_ftyp_upper :
 forall e1 A1,
-  fv_fexp_in_fexp (open_fexp_wrt_ftyp e1 A1) [<=] fv_fexp_in_fexp e1.
+  fvar_in_fexp (open_fexp_wrt_ftyp e1 A1) [<=] fvar_in_fexp e1.
 Proof.
 unfold open_fexp_wrt_ftyp; default_simp.
 Qed.
 
-#[export] Hint Resolve fv_fexp_in_fexp_open_fexp_wrt_ftyp_upper : lngen.
+#[export] Hint Resolve fvar_in_fexp_open_fexp_wrt_ftyp_upper : lngen.
 
-Lemma fv_fexp_in_fexp_open_fexp_wrt_fexp_upper :
+Lemma fvar_in_fexp_open_fexp_wrt_fexp_upper :
 forall e1 e2,
-  fv_fexp_in_fexp (open_fexp_wrt_fexp e1 e2) [<=] fv_fexp_in_fexp e2 `union` fv_fexp_in_fexp e1.
+  fvar_in_fexp (open_fexp_wrt_fexp e1 e2) [<=] fvar_in_fexp e2 `union` fvar_in_fexp e1.
 Proof.
 unfold open_fexp_wrt_fexp; default_simp.
 Qed.
 
-#[export] Hint Resolve fv_fexp_in_fexp_open_fexp_wrt_fexp_upper : lngen.
+#[export] Hint Resolve fvar_in_fexp_open_fexp_wrt_fexp_upper : lngen.
 
-Lemma fv_ftyp_in_fbind_open_fbind_wrt_ftyp_upper :
+Lemma ftvar_in_fbind_open_fbind_wrt_ftyp_upper :
 forall fb1 A1,
-  fv_ftyp_in_fbind (open_fbind_wrt_ftyp fb1 A1) [<=] fv_ftyp_in_ftyp A1 `union` fv_ftyp_in_fbind fb1.
+  ftvar_in_fbind (open_fbind_wrt_ftyp fb1 A1) [<=] ftvar_in_ftyp A1 `union` ftvar_in_fbind fb1.
 Proof.
 unfold open_fbind_wrt_ftyp; default_simp.
 Qed.
 
-#[export] Hint Resolve fv_ftyp_in_fbind_open_fbind_wrt_ftyp_upper : lngen.
+#[export] Hint Resolve ftvar_in_fbind_open_fbind_wrt_ftyp_upper : lngen.
 
 (* begin hide *)
 
-Lemma fv_ftyp_in_ftyp_subst_typ_in_ftyp_fresh_mutual :
+Lemma ftvar_in_ftyp_subst_typ_in_ftyp_fresh_mutual :
 (forall A1 A2 X1,
-  X1 `notin` fv_ftyp_in_ftyp A1 ->
-  fv_ftyp_in_ftyp (subst_typ_in_ftyp A2 X1 A1) [=] fv_ftyp_in_ftyp A1).
+  X1 `notin` ftvar_in_ftyp A1 ->
+  ftvar_in_ftyp (subst_typ_in_ftyp A2 X1 A1) [=] ftvar_in_ftyp A1).
 Proof.
 apply_mutual_ind ftyp_mutind;
 default_simp; fsetdec.
@@ -4227,23 +4227,23 @@ Qed.
 
 (* end hide *)
 
-Lemma fv_ftyp_in_ftyp_subst_typ_in_ftyp_fresh :
+Lemma ftvar_in_ftyp_subst_typ_in_ftyp_fresh :
 forall A1 A2 X1,
-  X1 `notin` fv_ftyp_in_ftyp A1 ->
-  fv_ftyp_in_ftyp (subst_typ_in_ftyp A2 X1 A1) [=] fv_ftyp_in_ftyp A1.
+  X1 `notin` ftvar_in_ftyp A1 ->
+  ftvar_in_ftyp (subst_typ_in_ftyp A2 X1 A1) [=] ftvar_in_ftyp A1.
 Proof.
-pose proof fv_ftyp_in_ftyp_subst_typ_in_ftyp_fresh_mutual as H; intuition eauto.
+pose proof ftvar_in_ftyp_subst_typ_in_ftyp_fresh_mutual as H; intuition eauto.
 Qed.
 
-#[export] Hint Resolve fv_ftyp_in_ftyp_subst_typ_in_ftyp_fresh : lngen.
-#[export] Hint Rewrite fv_ftyp_in_ftyp_subst_typ_in_ftyp_fresh using solve [auto] : lngen.
+#[export] Hint Resolve ftvar_in_ftyp_subst_typ_in_ftyp_fresh : lngen.
+#[export] Hint Rewrite ftvar_in_ftyp_subst_typ_in_ftyp_fresh using solve [auto] : lngen.
 
 (* begin hide *)
 
-Lemma fv_ftyp_in_fexp_subst_typ_in_fexp_fresh_mutual :
+Lemma ftvar_in_fexp_subst_typ_in_fexp_fresh_mutual :
 (forall e1 A1 X1,
-  X1 `notin` fv_ftyp_in_fexp e1 ->
-  fv_ftyp_in_fexp (subst_typ_in_fexp A1 X1 e1) [=] fv_ftyp_in_fexp e1).
+  X1 `notin` ftvar_in_fexp e1 ->
+  ftvar_in_fexp (subst_typ_in_fexp A1 X1 e1) [=] ftvar_in_fexp e1).
 Proof.
 apply_mutual_ind fexp_mutind;
 default_simp; fsetdec.
@@ -4251,22 +4251,22 @@ Qed.
 
 (* end hide *)
 
-Lemma fv_ftyp_in_fexp_subst_typ_in_fexp_fresh :
+Lemma ftvar_in_fexp_subst_typ_in_fexp_fresh :
 forall e1 A1 X1,
-  X1 `notin` fv_ftyp_in_fexp e1 ->
-  fv_ftyp_in_fexp (subst_typ_in_fexp A1 X1 e1) [=] fv_ftyp_in_fexp e1.
+  X1 `notin` ftvar_in_fexp e1 ->
+  ftvar_in_fexp (subst_typ_in_fexp A1 X1 e1) [=] ftvar_in_fexp e1.
 Proof.
-pose proof fv_ftyp_in_fexp_subst_typ_in_fexp_fresh_mutual as H; intuition eauto.
+pose proof ftvar_in_fexp_subst_typ_in_fexp_fresh_mutual as H; intuition eauto.
 Qed.
 
-#[export] Hint Resolve fv_ftyp_in_fexp_subst_typ_in_fexp_fresh : lngen.
-#[export] Hint Rewrite fv_ftyp_in_fexp_subst_typ_in_fexp_fresh using solve [auto] : lngen.
+#[export] Hint Resolve ftvar_in_fexp_subst_typ_in_fexp_fresh : lngen.
+#[export] Hint Rewrite ftvar_in_fexp_subst_typ_in_fexp_fresh using solve [auto] : lngen.
 
 (* begin hide *)
 
-Lemma fv_ftyp_in_fexp_subst_exp_in_fexp_fresh_mutual :
+Lemma ftvar_in_fexp_subst_exp_in_fexp_fresh_mutual :
 (forall e1 A1 X1,
-  fv_fexp_in_fexp (subst_typ_in_fexp A1 X1 e1) [=] fv_fexp_in_fexp e1).
+  fvar_in_fexp (subst_typ_in_fexp A1 X1 e1) [=] fvar_in_fexp e1).
 Proof.
 apply_mutual_ind fexp_mutind;
 default_simp; fsetdec.
@@ -4274,22 +4274,22 @@ Qed.
 
 (* end hide *)
 
-Lemma fv_ftyp_in_fexp_subst_exp_in_fexp_fresh :
+Lemma ftvar_in_fexp_subst_exp_in_fexp_fresh :
 forall e1 A1 X1,
-  fv_fexp_in_fexp (subst_typ_in_fexp A1 X1 e1) [=] fv_fexp_in_fexp e1.
+  fvar_in_fexp (subst_typ_in_fexp A1 X1 e1) [=] fvar_in_fexp e1.
 Proof.
-pose proof fv_ftyp_in_fexp_subst_exp_in_fexp_fresh_mutual as H; intuition eauto.
+pose proof ftvar_in_fexp_subst_exp_in_fexp_fresh_mutual as H; intuition eauto.
 Qed.
 
-#[export] Hint Resolve fv_ftyp_in_fexp_subst_exp_in_fexp_fresh : lngen.
-#[export] Hint Rewrite fv_ftyp_in_fexp_subst_exp_in_fexp_fresh using solve [auto] : lngen.
+#[export] Hint Resolve ftvar_in_fexp_subst_exp_in_fexp_fresh : lngen.
+#[export] Hint Rewrite ftvar_in_fexp_subst_exp_in_fexp_fresh using solve [auto] : lngen.
 
 (* begin hide *)
 
-Lemma fv_fexp_in_fexp_subst_exp_in_fexp_fresh_mutual :
+Lemma fvar_in_fexp_subst_exp_in_fexp_fresh_mutual :
 (forall e1 e2 x1,
-  x1 `notin` fv_fexp_in_fexp e1 ->
-  fv_fexp_in_fexp (subst_exp_in_fexp e2 x1 e1) [=] fv_fexp_in_fexp e1).
+  x1 `notin` fvar_in_fexp e1 ->
+  fvar_in_fexp (subst_exp_in_fexp e2 x1 e1) [=] fvar_in_fexp e1).
 Proof.
 apply_mutual_ind fexp_mutind;
 default_simp; fsetdec.
@@ -4297,23 +4297,23 @@ Qed.
 
 (* end hide *)
 
-Lemma fv_fexp_in_fexp_subst_exp_in_fexp_fresh :
+Lemma fvar_in_fexp_subst_exp_in_fexp_fresh :
 forall e1 e2 x1,
-  x1 `notin` fv_fexp_in_fexp e1 ->
-  fv_fexp_in_fexp (subst_exp_in_fexp e2 x1 e1) [=] fv_fexp_in_fexp e1.
+  x1 `notin` fvar_in_fexp e1 ->
+  fvar_in_fexp (subst_exp_in_fexp e2 x1 e1) [=] fvar_in_fexp e1.
 Proof.
-pose proof fv_fexp_in_fexp_subst_exp_in_fexp_fresh_mutual as H; intuition eauto.
+pose proof fvar_in_fexp_subst_exp_in_fexp_fresh_mutual as H; intuition eauto.
 Qed.
 
-#[export] Hint Resolve fv_fexp_in_fexp_subst_exp_in_fexp_fresh : lngen.
-#[export] Hint Rewrite fv_fexp_in_fexp_subst_exp_in_fexp_fresh using solve [auto] : lngen.
+#[export] Hint Resolve fvar_in_fexp_subst_exp_in_fexp_fresh : lngen.
+#[export] Hint Rewrite fvar_in_fexp_subst_exp_in_fexp_fresh using solve [auto] : lngen.
 
 (* begin hide *)
 
-Lemma fv_ftyp_in_fbind_subst_typ_in_fbind_fresh_mutual :
+Lemma ftvar_in_fbind_subst_typ_in_fbind_fresh_mutual :
 (forall fb1 A1 X1,
-  X1 `notin` fv_ftyp_in_fbind fb1 ->
-  fv_ftyp_in_fbind (subst_typ_in_fbind A1 X1 fb1) [=] fv_ftyp_in_fbind fb1).
+  X1 `notin` ftvar_in_fbind fb1 ->
+  ftvar_in_fbind (subst_typ_in_fbind A1 X1 fb1) [=] ftvar_in_fbind fb1).
 Proof.
 apply_mutual_ind fbind_mutind;
 default_simp; fsetdec.
@@ -4321,22 +4321,22 @@ Qed.
 
 (* end hide *)
 
-Lemma fv_ftyp_in_fbind_subst_typ_in_fbind_fresh :
+Lemma ftvar_in_fbind_subst_typ_in_fbind_fresh :
 forall fb1 A1 X1,
-  X1 `notin` fv_ftyp_in_fbind fb1 ->
-  fv_ftyp_in_fbind (subst_typ_in_fbind A1 X1 fb1) [=] fv_ftyp_in_fbind fb1.
+  X1 `notin` ftvar_in_fbind fb1 ->
+  ftvar_in_fbind (subst_typ_in_fbind A1 X1 fb1) [=] ftvar_in_fbind fb1.
 Proof.
-pose proof fv_ftyp_in_fbind_subst_typ_in_fbind_fresh_mutual as H; intuition eauto.
+pose proof ftvar_in_fbind_subst_typ_in_fbind_fresh_mutual as H; intuition eauto.
 Qed.
 
-#[export] Hint Resolve fv_ftyp_in_fbind_subst_typ_in_fbind_fresh : lngen.
-#[export] Hint Rewrite fv_ftyp_in_fbind_subst_typ_in_fbind_fresh using solve [auto] : lngen.
+#[export] Hint Resolve ftvar_in_fbind_subst_typ_in_fbind_fresh : lngen.
+#[export] Hint Rewrite ftvar_in_fbind_subst_typ_in_fbind_fresh using solve [auto] : lngen.
 
 (* begin hide *)
 
-Lemma fv_ftyp_in_ftyp_subst_typ_in_ftyp_lower_mutual :
+Lemma ftvar_in_ftyp_subst_typ_in_ftyp_lower_mutual :
 (forall A1 A2 X1,
-  remove X1 (fv_ftyp_in_ftyp A1) [<=] fv_ftyp_in_ftyp (subst_typ_in_ftyp A2 X1 A1)).
+  remove X1 (ftvar_in_ftyp A1) [<=] ftvar_in_ftyp (subst_typ_in_ftyp A2 X1 A1)).
 Proof.
 apply_mutual_ind ftyp_mutind;
 default_simp; fsetdec.
@@ -4344,20 +4344,20 @@ Qed.
 
 (* end hide *)
 
-Lemma fv_ftyp_in_ftyp_subst_typ_in_ftyp_lower :
+Lemma ftvar_in_ftyp_subst_typ_in_ftyp_lower :
 forall A1 A2 X1,
-  remove X1 (fv_ftyp_in_ftyp A1) [<=] fv_ftyp_in_ftyp (subst_typ_in_ftyp A2 X1 A1).
+  remove X1 (ftvar_in_ftyp A1) [<=] ftvar_in_ftyp (subst_typ_in_ftyp A2 X1 A1).
 Proof.
-pose proof fv_ftyp_in_ftyp_subst_typ_in_ftyp_lower_mutual as H; intuition eauto.
+pose proof ftvar_in_ftyp_subst_typ_in_ftyp_lower_mutual as H; intuition eauto.
 Qed.
 
-#[export] Hint Resolve fv_ftyp_in_ftyp_subst_typ_in_ftyp_lower : lngen.
+#[export] Hint Resolve ftvar_in_ftyp_subst_typ_in_ftyp_lower : lngen.
 
 (* begin hide *)
 
-Lemma fv_ftyp_in_fexp_subst_typ_in_fexp_lower_mutual :
+Lemma ftvar_in_fexp_subst_typ_in_fexp_lower_mutual :
 (forall e1 A1 X1,
-  remove X1 (fv_ftyp_in_fexp e1) [<=] fv_ftyp_in_fexp (subst_typ_in_fexp A1 X1 e1)).
+  remove X1 (ftvar_in_fexp e1) [<=] ftvar_in_fexp (subst_typ_in_fexp A1 X1 e1)).
 Proof.
 apply_mutual_ind fexp_mutind;
 default_simp; fsetdec.
@@ -4365,20 +4365,20 @@ Qed.
 
 (* end hide *)
 
-Lemma fv_ftyp_in_fexp_subst_typ_in_fexp_lower :
+Lemma ftvar_in_fexp_subst_typ_in_fexp_lower :
 forall e1 A1 X1,
-  remove X1 (fv_ftyp_in_fexp e1) [<=] fv_ftyp_in_fexp (subst_typ_in_fexp A1 X1 e1).
+  remove X1 (ftvar_in_fexp e1) [<=] ftvar_in_fexp (subst_typ_in_fexp A1 X1 e1).
 Proof.
-pose proof fv_ftyp_in_fexp_subst_typ_in_fexp_lower_mutual as H; intuition eauto.
+pose proof ftvar_in_fexp_subst_typ_in_fexp_lower_mutual as H; intuition eauto.
 Qed.
 
-#[export] Hint Resolve fv_ftyp_in_fexp_subst_typ_in_fexp_lower : lngen.
+#[export] Hint Resolve ftvar_in_fexp_subst_typ_in_fexp_lower : lngen.
 
 (* begin hide *)
 
-Lemma fv_ftyp_in_fexp_subst_exp_in_fexp_lower_mutual :
+Lemma ftvar_in_fexp_subst_exp_in_fexp_lower_mutual :
 (forall e1 e2 x1,
-  fv_ftyp_in_fexp e1 [<=] fv_ftyp_in_fexp (subst_exp_in_fexp e2 x1 e1)).
+  ftvar_in_fexp e1 [<=] ftvar_in_fexp (subst_exp_in_fexp e2 x1 e1)).
 Proof.
 apply_mutual_ind fexp_mutind;
 default_simp; fsetdec.
@@ -4386,20 +4386,20 @@ Qed.
 
 (* end hide *)
 
-Lemma fv_ftyp_in_fexp_subst_exp_in_fexp_lower :
+Lemma ftvar_in_fexp_subst_exp_in_fexp_lower :
 forall e1 e2 x1,
-  fv_ftyp_in_fexp e1 [<=] fv_ftyp_in_fexp (subst_exp_in_fexp e2 x1 e1).
+  ftvar_in_fexp e1 [<=] ftvar_in_fexp (subst_exp_in_fexp e2 x1 e1).
 Proof.
-pose proof fv_ftyp_in_fexp_subst_exp_in_fexp_lower_mutual as H; intuition eauto.
+pose proof ftvar_in_fexp_subst_exp_in_fexp_lower_mutual as H; intuition eauto.
 Qed.
 
-#[export] Hint Resolve fv_ftyp_in_fexp_subst_exp_in_fexp_lower : lngen.
+#[export] Hint Resolve ftvar_in_fexp_subst_exp_in_fexp_lower : lngen.
 
 (* begin hide *)
 
-Lemma fv_fexp_in_fexp_subst_typ_in_fexp_lower_mutual :
+Lemma fvar_in_fexp_subst_typ_in_fexp_lower_mutual :
 (forall e1 A1 X1,
-  fv_fexp_in_fexp e1 [<=] fv_fexp_in_fexp (subst_typ_in_fexp A1 X1 e1)).
+  fvar_in_fexp e1 [<=] fvar_in_fexp (subst_typ_in_fexp A1 X1 e1)).
 Proof.
 apply_mutual_ind fexp_mutind;
 default_simp; fsetdec.
@@ -4407,20 +4407,20 @@ Qed.
 
 (* end hide *)
 
-Lemma fv_fexp_in_fexp_subst_typ_in_fexp_lower :
+Lemma fvar_in_fexp_subst_typ_in_fexp_lower :
 forall e1 A1 X1,
-  fv_fexp_in_fexp e1 [<=] fv_fexp_in_fexp (subst_typ_in_fexp A1 X1 e1).
+  fvar_in_fexp e1 [<=] fvar_in_fexp (subst_typ_in_fexp A1 X1 e1).
 Proof.
-pose proof fv_fexp_in_fexp_subst_typ_in_fexp_lower_mutual as H; intuition eauto.
+pose proof fvar_in_fexp_subst_typ_in_fexp_lower_mutual as H; intuition eauto.
 Qed.
 
-#[export] Hint Resolve fv_fexp_in_fexp_subst_typ_in_fexp_lower : lngen.
+#[export] Hint Resolve fvar_in_fexp_subst_typ_in_fexp_lower : lngen.
 
 (* begin hide *)
 
-Lemma fv_fexp_in_fexp_subst_exp_in_fexp_lower_mutual :
+Lemma fvar_in_fexp_subst_exp_in_fexp_lower_mutual :
 (forall e1 e2 x1,
-  remove x1 (fv_fexp_in_fexp e1) [<=] fv_fexp_in_fexp (subst_exp_in_fexp e2 x1 e1)).
+  remove x1 (fvar_in_fexp e1) [<=] fvar_in_fexp (subst_exp_in_fexp e2 x1 e1)).
 Proof.
 apply_mutual_ind fexp_mutind;
 default_simp; fsetdec.
@@ -4428,20 +4428,20 @@ Qed.
 
 (* end hide *)
 
-Lemma fv_fexp_in_fexp_subst_exp_in_fexp_lower :
+Lemma fvar_in_fexp_subst_exp_in_fexp_lower :
 forall e1 e2 x1,
-  remove x1 (fv_fexp_in_fexp e1) [<=] fv_fexp_in_fexp (subst_exp_in_fexp e2 x1 e1).
+  remove x1 (fvar_in_fexp e1) [<=] fvar_in_fexp (subst_exp_in_fexp e2 x1 e1).
 Proof.
-pose proof fv_fexp_in_fexp_subst_exp_in_fexp_lower_mutual as H; intuition eauto.
+pose proof fvar_in_fexp_subst_exp_in_fexp_lower_mutual as H; intuition eauto.
 Qed.
 
-#[export] Hint Resolve fv_fexp_in_fexp_subst_exp_in_fexp_lower : lngen.
+#[export] Hint Resolve fvar_in_fexp_subst_exp_in_fexp_lower : lngen.
 
 (* begin hide *)
 
-Lemma fv_ftyp_in_fbind_subst_typ_in_fbind_lower_mutual :
+Lemma ftvar_in_fbind_subst_typ_in_fbind_lower_mutual :
 (forall fb1 A1 X1,
-  remove X1 (fv_ftyp_in_fbind fb1) [<=] fv_ftyp_in_fbind (subst_typ_in_fbind A1 X1 fb1)).
+  remove X1 (ftvar_in_fbind fb1) [<=] ftvar_in_fbind (subst_typ_in_fbind A1 X1 fb1)).
 Proof.
 apply_mutual_ind fbind_mutind;
 default_simp; fsetdec.
@@ -4449,22 +4449,22 @@ Qed.
 
 (* end hide *)
 
-Lemma fv_ftyp_in_fbind_subst_typ_in_fbind_lower :
+Lemma ftvar_in_fbind_subst_typ_in_fbind_lower :
 forall fb1 A1 X1,
-  remove X1 (fv_ftyp_in_fbind fb1) [<=] fv_ftyp_in_fbind (subst_typ_in_fbind A1 X1 fb1).
+  remove X1 (ftvar_in_fbind fb1) [<=] ftvar_in_fbind (subst_typ_in_fbind A1 X1 fb1).
 Proof.
-pose proof fv_ftyp_in_fbind_subst_typ_in_fbind_lower_mutual as H; intuition eauto.
+pose proof ftvar_in_fbind_subst_typ_in_fbind_lower_mutual as H; intuition eauto.
 Qed.
 
-#[export] Hint Resolve fv_ftyp_in_fbind_subst_typ_in_fbind_lower : lngen.
+#[export] Hint Resolve ftvar_in_fbind_subst_typ_in_fbind_lower : lngen.
 
 (* begin hide *)
 
-Lemma fv_ftyp_in_ftyp_subst_typ_in_ftyp_notin_mutual :
+Lemma ftvar_in_ftyp_subst_typ_in_ftyp_notin_mutual :
 (forall A1 A2 X1 X2,
-  X2 `notin` fv_ftyp_in_ftyp A1 ->
-  X2 `notin` fv_ftyp_in_ftyp A2 ->
-  X2 `notin` fv_ftyp_in_ftyp (subst_typ_in_ftyp A2 X1 A1)).
+  X2 `notin` ftvar_in_ftyp A1 ->
+  X2 `notin` ftvar_in_ftyp A2 ->
+  X2 `notin` ftvar_in_ftyp (subst_typ_in_ftyp A2 X1 A1)).
 Proof.
 apply_mutual_ind ftyp_mutind;
 default_simp; fsetdec.
@@ -4472,24 +4472,24 @@ Qed.
 
 (* end hide *)
 
-Lemma fv_ftyp_in_ftyp_subst_typ_in_ftyp_notin :
+Lemma ftvar_in_ftyp_subst_typ_in_ftyp_notin :
 forall A1 A2 X1 X2,
-  X2 `notin` fv_ftyp_in_ftyp A1 ->
-  X2 `notin` fv_ftyp_in_ftyp A2 ->
-  X2 `notin` fv_ftyp_in_ftyp (subst_typ_in_ftyp A2 X1 A1).
+  X2 `notin` ftvar_in_ftyp A1 ->
+  X2 `notin` ftvar_in_ftyp A2 ->
+  X2 `notin` ftvar_in_ftyp (subst_typ_in_ftyp A2 X1 A1).
 Proof.
-pose proof fv_ftyp_in_ftyp_subst_typ_in_ftyp_notin_mutual as H; intuition eauto.
+pose proof ftvar_in_ftyp_subst_typ_in_ftyp_notin_mutual as H; intuition eauto.
 Qed.
 
-#[export] Hint Resolve fv_ftyp_in_ftyp_subst_typ_in_ftyp_notin : lngen.
+#[export] Hint Resolve ftvar_in_ftyp_subst_typ_in_ftyp_notin : lngen.
 
 (* begin hide *)
 
-Lemma fv_ftyp_in_fexp_subst_typ_in_fexp_notin_mutual :
+Lemma ftvar_in_fexp_subst_typ_in_fexp_notin_mutual :
 (forall e1 A1 X1 X2,
-  X2 `notin` fv_ftyp_in_fexp e1 ->
-  X2 `notin` fv_ftyp_in_ftyp A1 ->
-  X2 `notin` fv_ftyp_in_fexp (subst_typ_in_fexp A1 X1 e1)).
+  X2 `notin` ftvar_in_fexp e1 ->
+  X2 `notin` ftvar_in_ftyp A1 ->
+  X2 `notin` ftvar_in_fexp (subst_typ_in_fexp A1 X1 e1)).
 Proof.
 apply_mutual_ind fexp_mutind;
 default_simp; fsetdec.
@@ -4497,24 +4497,24 @@ Qed.
 
 (* end hide *)
 
-Lemma fv_ftyp_in_fexp_subst_typ_in_fexp_notin :
+Lemma ftvar_in_fexp_subst_typ_in_fexp_notin :
 forall e1 A1 X1 X2,
-  X2 `notin` fv_ftyp_in_fexp e1 ->
-  X2 `notin` fv_ftyp_in_ftyp A1 ->
-  X2 `notin` fv_ftyp_in_fexp (subst_typ_in_fexp A1 X1 e1).
+  X2 `notin` ftvar_in_fexp e1 ->
+  X2 `notin` ftvar_in_ftyp A1 ->
+  X2 `notin` ftvar_in_fexp (subst_typ_in_fexp A1 X1 e1).
 Proof.
-pose proof fv_ftyp_in_fexp_subst_typ_in_fexp_notin_mutual as H; intuition eauto.
+pose proof ftvar_in_fexp_subst_typ_in_fexp_notin_mutual as H; intuition eauto.
 Qed.
 
-#[export] Hint Resolve fv_ftyp_in_fexp_subst_typ_in_fexp_notin : lngen.
+#[export] Hint Resolve ftvar_in_fexp_subst_typ_in_fexp_notin : lngen.
 
 (* begin hide *)
 
-Lemma fv_ftyp_in_fexp_subst_exp_in_fexp_notin_mutual :
+Lemma ftvar_in_fexp_subst_exp_in_fexp_notin_mutual :
 (forall e1 e2 x1 X1,
-  X1 `notin` fv_ftyp_in_fexp e1 ->
-  X1 `notin` fv_ftyp_in_fexp e2 ->
-  X1 `notin` fv_ftyp_in_fexp (subst_exp_in_fexp e2 x1 e1)).
+  X1 `notin` ftvar_in_fexp e1 ->
+  X1 `notin` ftvar_in_fexp e2 ->
+  X1 `notin` ftvar_in_fexp (subst_exp_in_fexp e2 x1 e1)).
 Proof.
 apply_mutual_ind fexp_mutind;
 default_simp; fsetdec.
@@ -4522,23 +4522,23 @@ Qed.
 
 (* end hide *)
 
-Lemma fv_ftyp_in_fexp_subst_exp_in_fexp_notin :
+Lemma ftvar_in_fexp_subst_exp_in_fexp_notin :
 forall e1 e2 x1 X1,
-  X1 `notin` fv_ftyp_in_fexp e1 ->
-  X1 `notin` fv_ftyp_in_fexp e2 ->
-  X1 `notin` fv_ftyp_in_fexp (subst_exp_in_fexp e2 x1 e1).
+  X1 `notin` ftvar_in_fexp e1 ->
+  X1 `notin` ftvar_in_fexp e2 ->
+  X1 `notin` ftvar_in_fexp (subst_exp_in_fexp e2 x1 e1).
 Proof.
-pose proof fv_ftyp_in_fexp_subst_exp_in_fexp_notin_mutual as H; intuition eauto.
+pose proof ftvar_in_fexp_subst_exp_in_fexp_notin_mutual as H; intuition eauto.
 Qed.
 
-#[export] Hint Resolve fv_ftyp_in_fexp_subst_exp_in_fexp_notin : lngen.
+#[export] Hint Resolve ftvar_in_fexp_subst_exp_in_fexp_notin : lngen.
 
 (* begin hide *)
 
-Lemma fv_fexp_in_fexp_subst_typ_in_fexp_notin_mutual :
+Lemma fvar_in_fexp_subst_typ_in_fexp_notin_mutual :
 (forall e1 A1 X1 x1,
-  x1 `notin` fv_fexp_in_fexp e1 ->
-  x1 `notin` fv_fexp_in_fexp (subst_typ_in_fexp A1 X1 e1)).
+  x1 `notin` fvar_in_fexp e1 ->
+  x1 `notin` fvar_in_fexp (subst_typ_in_fexp A1 X1 e1)).
 Proof.
 apply_mutual_ind fexp_mutind;
 default_simp; fsetdec.
@@ -4546,23 +4546,23 @@ Qed.
 
 (* end hide *)
 
-Lemma fv_fexp_in_fexp_subst_typ_in_fexp_notin :
+Lemma fvar_in_fexp_subst_typ_in_fexp_notin :
 forall e1 A1 X1 x1,
-  x1 `notin` fv_fexp_in_fexp e1 ->
-  x1 `notin` fv_fexp_in_fexp (subst_typ_in_fexp A1 X1 e1).
+  x1 `notin` fvar_in_fexp e1 ->
+  x1 `notin` fvar_in_fexp (subst_typ_in_fexp A1 X1 e1).
 Proof.
-pose proof fv_fexp_in_fexp_subst_typ_in_fexp_notin_mutual as H; intuition eauto.
+pose proof fvar_in_fexp_subst_typ_in_fexp_notin_mutual as H; intuition eauto.
 Qed.
 
-#[export] Hint Resolve fv_fexp_in_fexp_subst_typ_in_fexp_notin : lngen.
+#[export] Hint Resolve fvar_in_fexp_subst_typ_in_fexp_notin : lngen.
 
 (* begin hide *)
 
-Lemma fv_fexp_in_fexp_subst_exp_in_fexp_notin_mutual :
+Lemma fvar_in_fexp_subst_exp_in_fexp_notin_mutual :
 (forall e1 e2 x1 x2,
-  x2 `notin` fv_fexp_in_fexp e1 ->
-  x2 `notin` fv_fexp_in_fexp e2 ->
-  x2 `notin` fv_fexp_in_fexp (subst_exp_in_fexp e2 x1 e1)).
+  x2 `notin` fvar_in_fexp e1 ->
+  x2 `notin` fvar_in_fexp e2 ->
+  x2 `notin` fvar_in_fexp (subst_exp_in_fexp e2 x1 e1)).
 Proof.
 apply_mutual_ind fexp_mutind;
 default_simp; fsetdec.
@@ -4570,24 +4570,24 @@ Qed.
 
 (* end hide *)
 
-Lemma fv_fexp_in_fexp_subst_exp_in_fexp_notin :
+Lemma fvar_in_fexp_subst_exp_in_fexp_notin :
 forall e1 e2 x1 x2,
-  x2 `notin` fv_fexp_in_fexp e1 ->
-  x2 `notin` fv_fexp_in_fexp e2 ->
-  x2 `notin` fv_fexp_in_fexp (subst_exp_in_fexp e2 x1 e1).
+  x2 `notin` fvar_in_fexp e1 ->
+  x2 `notin` fvar_in_fexp e2 ->
+  x2 `notin` fvar_in_fexp (subst_exp_in_fexp e2 x1 e1).
 Proof.
-pose proof fv_fexp_in_fexp_subst_exp_in_fexp_notin_mutual as H; intuition eauto.
+pose proof fvar_in_fexp_subst_exp_in_fexp_notin_mutual as H; intuition eauto.
 Qed.
 
-#[export] Hint Resolve fv_fexp_in_fexp_subst_exp_in_fexp_notin : lngen.
+#[export] Hint Resolve fvar_in_fexp_subst_exp_in_fexp_notin : lngen.
 
 (* begin hide *)
 
-Lemma fv_ftyp_in_fbind_subst_typ_in_fbind_notin_mutual :
+Lemma ftvar_in_fbind_subst_typ_in_fbind_notin_mutual :
 (forall fb1 A1 X1 X2,
-  X2 `notin` fv_ftyp_in_fbind fb1 ->
-  X2 `notin` fv_ftyp_in_ftyp A1 ->
-  X2 `notin` fv_ftyp_in_fbind (subst_typ_in_fbind A1 X1 fb1)).
+  X2 `notin` ftvar_in_fbind fb1 ->
+  X2 `notin` ftvar_in_ftyp A1 ->
+  X2 `notin` ftvar_in_fbind (subst_typ_in_fbind A1 X1 fb1)).
 Proof.
 apply_mutual_ind fbind_mutind;
 default_simp; fsetdec.
@@ -4595,22 +4595,22 @@ Qed.
 
 (* end hide *)
 
-Lemma fv_ftyp_in_fbind_subst_typ_in_fbind_notin :
+Lemma ftvar_in_fbind_subst_typ_in_fbind_notin :
 forall fb1 A1 X1 X2,
-  X2 `notin` fv_ftyp_in_fbind fb1 ->
-  X2 `notin` fv_ftyp_in_ftyp A1 ->
-  X2 `notin` fv_ftyp_in_fbind (subst_typ_in_fbind A1 X1 fb1).
+  X2 `notin` ftvar_in_fbind fb1 ->
+  X2 `notin` ftvar_in_ftyp A1 ->
+  X2 `notin` ftvar_in_fbind (subst_typ_in_fbind A1 X1 fb1).
 Proof.
-pose proof fv_ftyp_in_fbind_subst_typ_in_fbind_notin_mutual as H; intuition eauto.
+pose proof ftvar_in_fbind_subst_typ_in_fbind_notin_mutual as H; intuition eauto.
 Qed.
 
-#[export] Hint Resolve fv_ftyp_in_fbind_subst_typ_in_fbind_notin : lngen.
+#[export] Hint Resolve ftvar_in_fbind_subst_typ_in_fbind_notin : lngen.
 
 (* begin hide *)
 
-Lemma fv_ftyp_in_ftyp_subst_typ_in_ftyp_upper_mutual :
+Lemma ftvar_in_ftyp_subst_typ_in_ftyp_upper_mutual :
 (forall A1 A2 X1,
-  fv_ftyp_in_ftyp (subst_typ_in_ftyp A2 X1 A1) [<=] fv_ftyp_in_ftyp A2 `union` remove X1 (fv_ftyp_in_ftyp A1)).
+  ftvar_in_ftyp (subst_typ_in_ftyp A2 X1 A1) [<=] ftvar_in_ftyp A2 `union` remove X1 (ftvar_in_ftyp A1)).
 Proof.
 apply_mutual_ind ftyp_mutind;
 default_simp; fsetdec.
@@ -4618,20 +4618,20 @@ Qed.
 
 (* end hide *)
 
-Lemma fv_ftyp_in_ftyp_subst_typ_in_ftyp_upper :
+Lemma ftvar_in_ftyp_subst_typ_in_ftyp_upper :
 forall A1 A2 X1,
-  fv_ftyp_in_ftyp (subst_typ_in_ftyp A2 X1 A1) [<=] fv_ftyp_in_ftyp A2 `union` remove X1 (fv_ftyp_in_ftyp A1).
+  ftvar_in_ftyp (subst_typ_in_ftyp A2 X1 A1) [<=] ftvar_in_ftyp A2 `union` remove X1 (ftvar_in_ftyp A1).
 Proof.
-pose proof fv_ftyp_in_ftyp_subst_typ_in_ftyp_upper_mutual as H; intuition eauto.
+pose proof ftvar_in_ftyp_subst_typ_in_ftyp_upper_mutual as H; intuition eauto.
 Qed.
 
-#[export] Hint Resolve fv_ftyp_in_ftyp_subst_typ_in_ftyp_upper : lngen.
+#[export] Hint Resolve ftvar_in_ftyp_subst_typ_in_ftyp_upper : lngen.
 
 (* begin hide *)
 
-Lemma fv_ftyp_in_fexp_subst_typ_in_fexp_upper_mutual :
+Lemma ftvar_in_fexp_subst_typ_in_fexp_upper_mutual :
 (forall e1 A1 X1,
-  fv_ftyp_in_fexp (subst_typ_in_fexp A1 X1 e1) [<=] fv_ftyp_in_ftyp A1 `union` remove X1 (fv_ftyp_in_fexp e1)).
+  ftvar_in_fexp (subst_typ_in_fexp A1 X1 e1) [<=] ftvar_in_ftyp A1 `union` remove X1 (ftvar_in_fexp e1)).
 Proof.
 apply_mutual_ind fexp_mutind;
 default_simp; fsetdec.
@@ -4639,20 +4639,20 @@ Qed.
 
 (* end hide *)
 
-Lemma fv_ftyp_in_fexp_subst_typ_in_fexp_upper :
+Lemma ftvar_in_fexp_subst_typ_in_fexp_upper :
 forall e1 A1 X1,
-  fv_ftyp_in_fexp (subst_typ_in_fexp A1 X1 e1) [<=] fv_ftyp_in_ftyp A1 `union` remove X1 (fv_ftyp_in_fexp e1).
+  ftvar_in_fexp (subst_typ_in_fexp A1 X1 e1) [<=] ftvar_in_ftyp A1 `union` remove X1 (ftvar_in_fexp e1).
 Proof.
-pose proof fv_ftyp_in_fexp_subst_typ_in_fexp_upper_mutual as H; intuition eauto.
+pose proof ftvar_in_fexp_subst_typ_in_fexp_upper_mutual as H; intuition eauto.
 Qed.
 
-#[export] Hint Resolve fv_ftyp_in_fexp_subst_typ_in_fexp_upper : lngen.
+#[export] Hint Resolve ftvar_in_fexp_subst_typ_in_fexp_upper : lngen.
 
 (* begin hide *)
 
-Lemma fv_ftyp_in_fexp_subst_exp_in_fexp_upper_mutual :
+Lemma ftvar_in_fexp_subst_exp_in_fexp_upper_mutual :
 (forall e1 e2 x1,
-  fv_ftyp_in_fexp (subst_exp_in_fexp e2 x1 e1) [<=] fv_ftyp_in_fexp e2 `union` fv_ftyp_in_fexp e1).
+  ftvar_in_fexp (subst_exp_in_fexp e2 x1 e1) [<=] ftvar_in_fexp e2 `union` ftvar_in_fexp e1).
 Proof.
 apply_mutual_ind fexp_mutind;
 default_simp; fsetdec.
@@ -4660,20 +4660,20 @@ Qed.
 
 (* end hide *)
 
-Lemma fv_ftyp_in_fexp_subst_exp_in_fexp_upper :
+Lemma ftvar_in_fexp_subst_exp_in_fexp_upper :
 forall e1 e2 x1,
-  fv_ftyp_in_fexp (subst_exp_in_fexp e2 x1 e1) [<=] fv_ftyp_in_fexp e2 `union` fv_ftyp_in_fexp e1.
+  ftvar_in_fexp (subst_exp_in_fexp e2 x1 e1) [<=] ftvar_in_fexp e2 `union` ftvar_in_fexp e1.
 Proof.
-pose proof fv_ftyp_in_fexp_subst_exp_in_fexp_upper_mutual as H; intuition eauto.
+pose proof ftvar_in_fexp_subst_exp_in_fexp_upper_mutual as H; intuition eauto.
 Qed.
 
-#[export] Hint Resolve fv_ftyp_in_fexp_subst_exp_in_fexp_upper : lngen.
+#[export] Hint Resolve ftvar_in_fexp_subst_exp_in_fexp_upper : lngen.
 
 (* begin hide *)
 
-Lemma fv_fexp_in_fexp_subst_typ_in_fexp_upper_mutual :
+Lemma fvar_in_fexp_subst_typ_in_fexp_upper_mutual :
 (forall e1 A1 X1,
-  fv_fexp_in_fexp (subst_typ_in_fexp A1 X1 e1) [<=] fv_fexp_in_fexp e1).
+  fvar_in_fexp (subst_typ_in_fexp A1 X1 e1) [<=] fvar_in_fexp e1).
 Proof.
 apply_mutual_ind fexp_mutind;
 default_simp; fsetdec.
@@ -4681,20 +4681,20 @@ Qed.
 
 (* end hide *)
 
-Lemma fv_fexp_in_fexp_subst_typ_in_fexp_upper :
+Lemma fvar_in_fexp_subst_typ_in_fexp_upper :
 forall e1 A1 X1,
-  fv_fexp_in_fexp (subst_typ_in_fexp A1 X1 e1) [<=] fv_fexp_in_fexp e1.
+  fvar_in_fexp (subst_typ_in_fexp A1 X1 e1) [<=] fvar_in_fexp e1.
 Proof.
-pose proof fv_fexp_in_fexp_subst_typ_in_fexp_upper_mutual as H; intuition eauto.
+pose proof fvar_in_fexp_subst_typ_in_fexp_upper_mutual as H; intuition eauto.
 Qed.
 
-#[export] Hint Resolve fv_fexp_in_fexp_subst_typ_in_fexp_upper : lngen.
+#[export] Hint Resolve fvar_in_fexp_subst_typ_in_fexp_upper : lngen.
 
 (* begin hide *)
 
-Lemma fv_fexp_in_fexp_subst_exp_in_fexp_upper_mutual :
+Lemma fvar_in_fexp_subst_exp_in_fexp_upper_mutual :
 (forall e1 e2 x1,
-  fv_fexp_in_fexp (subst_exp_in_fexp e2 x1 e1) [<=] fv_fexp_in_fexp e2 `union` remove x1 (fv_fexp_in_fexp e1)).
+  fvar_in_fexp (subst_exp_in_fexp e2 x1 e1) [<=] fvar_in_fexp e2 `union` remove x1 (fvar_in_fexp e1)).
 Proof.
 apply_mutual_ind fexp_mutind;
 default_simp; fsetdec.
@@ -4702,20 +4702,20 @@ Qed.
 
 (* end hide *)
 
-Lemma fv_fexp_in_fexp_subst_exp_in_fexp_upper :
+Lemma fvar_in_fexp_subst_exp_in_fexp_upper :
 forall e1 e2 x1,
-  fv_fexp_in_fexp (subst_exp_in_fexp e2 x1 e1) [<=] fv_fexp_in_fexp e2 `union` remove x1 (fv_fexp_in_fexp e1).
+  fvar_in_fexp (subst_exp_in_fexp e2 x1 e1) [<=] fvar_in_fexp e2 `union` remove x1 (fvar_in_fexp e1).
 Proof.
-pose proof fv_fexp_in_fexp_subst_exp_in_fexp_upper_mutual as H; intuition eauto.
+pose proof fvar_in_fexp_subst_exp_in_fexp_upper_mutual as H; intuition eauto.
 Qed.
 
-#[export] Hint Resolve fv_fexp_in_fexp_subst_exp_in_fexp_upper : lngen.
+#[export] Hint Resolve fvar_in_fexp_subst_exp_in_fexp_upper : lngen.
 
 (* begin hide *)
 
-Lemma fv_ftyp_in_fbind_subst_typ_in_fbind_upper_mutual :
+Lemma ftvar_in_fbind_subst_typ_in_fbind_upper_mutual :
 (forall fb1 A1 X1,
-  fv_ftyp_in_fbind (subst_typ_in_fbind A1 X1 fb1) [<=] fv_ftyp_in_ftyp A1 `union` remove X1 (fv_ftyp_in_fbind fb1)).
+  ftvar_in_fbind (subst_typ_in_fbind A1 X1 fb1) [<=] ftvar_in_ftyp A1 `union` remove X1 (ftvar_in_fbind fb1)).
 Proof.
 apply_mutual_ind fbind_mutind;
 default_simp; fsetdec.
@@ -4723,14 +4723,14 @@ Qed.
 
 (* end hide *)
 
-Lemma fv_ftyp_in_fbind_subst_typ_in_fbind_upper :
+Lemma ftvar_in_fbind_subst_typ_in_fbind_upper :
 forall fb1 A1 X1,
-  fv_ftyp_in_fbind (subst_typ_in_fbind A1 X1 fb1) [<=] fv_ftyp_in_ftyp A1 `union` remove X1 (fv_ftyp_in_fbind fb1).
+  ftvar_in_fbind (subst_typ_in_fbind A1 X1 fb1) [<=] ftvar_in_ftyp A1 `union` remove X1 (ftvar_in_fbind fb1).
 Proof.
-pose proof fv_ftyp_in_fbind_subst_typ_in_fbind_upper_mutual as H; intuition eauto.
+pose proof ftvar_in_fbind_subst_typ_in_fbind_upper_mutual as H; intuition eauto.
 Qed.
 
-#[export] Hint Resolve fv_ftyp_in_fbind_subst_typ_in_fbind_upper : lngen.
+#[export] Hint Resolve ftvar_in_fbind_subst_typ_in_fbind_upper : lngen.
 
 
 (* *********************************************************************** *)
@@ -4745,7 +4745,7 @@ Lemma subst_typ_in_ftyp_close_ftyp_wrt_ftyp_rec_mutual :
 (forall A2 A1 X1 X2 n1,
   degree_ftyp_wrt_ftyp n1 A1 ->
   X1 <> X2 ->
-  X2 `notin` fv_ftyp_in_ftyp A1 ->
+  X2 `notin` ftvar_in_ftyp A1 ->
   subst_typ_in_ftyp A1 X1 (close_ftyp_wrt_ftyp_rec n1 X2 A2) = close_ftyp_wrt_ftyp_rec n1 X2 (subst_typ_in_ftyp A1 X1 A2)).
 Proof.
 apply_mutual_ind ftyp_mutind;
@@ -4758,7 +4758,7 @@ Lemma subst_typ_in_ftyp_close_ftyp_wrt_ftyp_rec :
 forall A2 A1 X1 X2 n1,
   degree_ftyp_wrt_ftyp n1 A1 ->
   X1 <> X2 ->
-  X2 `notin` fv_ftyp_in_ftyp A1 ->
+  X2 `notin` ftvar_in_ftyp A1 ->
   subst_typ_in_ftyp A1 X1 (close_ftyp_wrt_ftyp_rec n1 X2 A2) = close_ftyp_wrt_ftyp_rec n1 X2 (subst_typ_in_ftyp A1 X1 A2).
 Proof.
 pose proof subst_typ_in_ftyp_close_ftyp_wrt_ftyp_rec_mutual as H; intuition eauto.
@@ -4772,7 +4772,7 @@ Lemma subst_typ_in_fexp_close_fexp_wrt_ftyp_rec_mutual :
 (forall e1 A1 X1 X2 n1,
   degree_ftyp_wrt_ftyp n1 A1 ->
   X1 <> X2 ->
-  X2 `notin` fv_ftyp_in_ftyp A1 ->
+  X2 `notin` ftvar_in_ftyp A1 ->
   subst_typ_in_fexp A1 X1 (close_fexp_wrt_ftyp_rec n1 X2 e1) = close_fexp_wrt_ftyp_rec n1 X2 (subst_typ_in_fexp A1 X1 e1)).
 Proof.
 apply_mutual_ind fexp_mutind;
@@ -4785,7 +4785,7 @@ Lemma subst_typ_in_fexp_close_fexp_wrt_ftyp_rec :
 forall e1 A1 X1 X2 n1,
   degree_ftyp_wrt_ftyp n1 A1 ->
   X1 <> X2 ->
-  X2 `notin` fv_ftyp_in_ftyp A1 ->
+  X2 `notin` ftvar_in_ftyp A1 ->
   subst_typ_in_fexp A1 X1 (close_fexp_wrt_ftyp_rec n1 X2 e1) = close_fexp_wrt_ftyp_rec n1 X2 (subst_typ_in_fexp A1 X1 e1).
 Proof.
 pose proof subst_typ_in_fexp_close_fexp_wrt_ftyp_rec_mutual as H; intuition eauto.
@@ -4819,7 +4819,7 @@ Qed.
 Lemma subst_exp_in_fexp_close_fexp_wrt_ftyp_rec_mutual :
 (forall e2 e1 X1 x1 n1,
   degree_fexp_wrt_ftyp n1 e1 ->
-  x1 `notin` fv_ftyp_in_fexp e1 ->
+  x1 `notin` ftvar_in_fexp e1 ->
   subst_exp_in_fexp e1 X1 (close_fexp_wrt_ftyp_rec n1 x1 e2) = close_fexp_wrt_ftyp_rec n1 x1 (subst_exp_in_fexp e1 X1 e2)).
 Proof.
 apply_mutual_ind fexp_mutind;
@@ -4831,7 +4831,7 @@ Qed.
 Lemma subst_exp_in_fexp_close_fexp_wrt_ftyp_rec :
 forall e2 e1 X1 x1 n1,
   degree_fexp_wrt_ftyp n1 e1 ->
-  x1 `notin` fv_ftyp_in_fexp e1 ->
+  x1 `notin` ftvar_in_fexp e1 ->
   subst_exp_in_fexp e1 X1 (close_fexp_wrt_ftyp_rec n1 x1 e2) = close_fexp_wrt_ftyp_rec n1 x1 (subst_exp_in_fexp e1 X1 e2).
 Proof.
 pose proof subst_exp_in_fexp_close_fexp_wrt_ftyp_rec_mutual as H; intuition eauto.
@@ -4845,7 +4845,7 @@ Lemma subst_exp_in_fexp_close_fexp_wrt_fexp_rec_mutual :
 (forall e2 e1 x1 x2 n1,
   degree_fexp_wrt_fexp n1 e1 ->
   x1 <> x2 ->
-  x2 `notin` fv_fexp_in_fexp e1 ->
+  x2 `notin` fvar_in_fexp e1 ->
   subst_exp_in_fexp e1 x1 (close_fexp_wrt_fexp_rec n1 x2 e2) = close_fexp_wrt_fexp_rec n1 x2 (subst_exp_in_fexp e1 x1 e2)).
 Proof.
 apply_mutual_ind fexp_mutind;
@@ -4858,7 +4858,7 @@ Lemma subst_exp_in_fexp_close_fexp_wrt_fexp_rec :
 forall e2 e1 x1 x2 n1,
   degree_fexp_wrt_fexp n1 e1 ->
   x1 <> x2 ->
-  x2 `notin` fv_fexp_in_fexp e1 ->
+  x2 `notin` fvar_in_fexp e1 ->
   subst_exp_in_fexp e1 x1 (close_fexp_wrt_fexp_rec n1 x2 e2) = close_fexp_wrt_fexp_rec n1 x2 (subst_exp_in_fexp e1 x1 e2).
 Proof.
 pose proof subst_exp_in_fexp_close_fexp_wrt_fexp_rec_mutual as H; intuition eauto.
@@ -4872,7 +4872,7 @@ Lemma subst_typ_in_fbind_close_fbind_wrt_ftyp_rec_mutual :
 (forall fb1 A1 X1 X2 n1,
   degree_ftyp_wrt_ftyp n1 A1 ->
   X1 <> X2 ->
-  X2 `notin` fv_ftyp_in_ftyp A1 ->
+  X2 `notin` ftvar_in_ftyp A1 ->
   subst_typ_in_fbind A1 X1 (close_fbind_wrt_ftyp_rec n1 X2 fb1) = close_fbind_wrt_ftyp_rec n1 X2 (subst_typ_in_fbind A1 X1 fb1)).
 Proof.
 apply_mutual_ind fbind_mutind;
@@ -4885,7 +4885,7 @@ Lemma subst_typ_in_fbind_close_fbind_wrt_ftyp_rec :
 forall fb1 A1 X1 X2 n1,
   degree_ftyp_wrt_ftyp n1 A1 ->
   X1 <> X2 ->
-  X2 `notin` fv_ftyp_in_ftyp A1 ->
+  X2 `notin` ftvar_in_ftyp A1 ->
   subst_typ_in_fbind A1 X1 (close_fbind_wrt_ftyp_rec n1 X2 fb1) = close_fbind_wrt_ftyp_rec n1 X2 (subst_typ_in_fbind A1 X1 fb1).
 Proof.
 pose proof subst_typ_in_fbind_close_fbind_wrt_ftyp_rec_mutual as H; intuition eauto.
@@ -4896,7 +4896,7 @@ Qed.
 Lemma subst_typ_in_ftyp_close_ftyp_wrt_ftyp :
 forall A2 A1 X1 X2,
   lc_ftyp A1 ->  X1 <> X2 ->
-  X2 `notin` fv_ftyp_in_ftyp A1 ->
+  X2 `notin` ftvar_in_ftyp A1 ->
   subst_typ_in_ftyp A1 X1 (close_ftyp_wrt_ftyp X2 A2) = close_ftyp_wrt_ftyp X2 (subst_typ_in_ftyp A1 X1 A2).
 Proof.
 unfold close_ftyp_wrt_ftyp; default_simp.
@@ -4907,7 +4907,7 @@ Qed.
 Lemma subst_typ_in_fexp_close_fexp_wrt_ftyp :
 forall e1 A1 X1 X2,
   lc_ftyp A1 ->  X1 <> X2 ->
-  X2 `notin` fv_ftyp_in_ftyp A1 ->
+  X2 `notin` ftvar_in_ftyp A1 ->
   subst_typ_in_fexp A1 X1 (close_fexp_wrt_ftyp X2 e1) = close_fexp_wrt_ftyp X2 (subst_typ_in_fexp A1 X1 e1).
 Proof.
 unfold close_fexp_wrt_ftyp; default_simp.
@@ -4926,7 +4926,7 @@ Qed.
 
 Lemma subst_exp_in_fexp_close_fexp_wrt_ftyp :
 forall e2 e1 X1 x1,
-  lc_fexp e1 ->  x1 `notin` fv_ftyp_in_fexp e1 ->
+  lc_fexp e1 ->  x1 `notin` ftvar_in_fexp e1 ->
   subst_exp_in_fexp e1 X1 (close_fexp_wrt_ftyp x1 e2) = close_fexp_wrt_ftyp x1 (subst_exp_in_fexp e1 X1 e2).
 Proof.
 unfold close_fexp_wrt_ftyp; default_simp.
@@ -4937,7 +4937,7 @@ Qed.
 Lemma subst_exp_in_fexp_close_fexp_wrt_fexp :
 forall e2 e1 x1 x2,
   lc_fexp e1 ->  x1 <> x2 ->
-  x2 `notin` fv_fexp_in_fexp e1 ->
+  x2 `notin` fvar_in_fexp e1 ->
   subst_exp_in_fexp e1 x1 (close_fexp_wrt_fexp x2 e2) = close_fexp_wrt_fexp x2 (subst_exp_in_fexp e1 x1 e2).
 Proof.
 unfold close_fexp_wrt_fexp; default_simp.
@@ -4948,7 +4948,7 @@ Qed.
 Lemma subst_typ_in_fbind_close_fbind_wrt_ftyp :
 forall fb1 A1 X1 X2,
   lc_ftyp A1 ->  X1 <> X2 ->
-  X2 `notin` fv_ftyp_in_ftyp A1 ->
+  X2 `notin` ftvar_in_ftyp A1 ->
   subst_typ_in_fbind A1 X1 (close_fbind_wrt_ftyp X2 fb1) = close_fbind_wrt_ftyp X2 (subst_typ_in_fbind A1 X1 fb1).
 Proof.
 unfold close_fbind_wrt_ftyp; default_simp.
@@ -5108,7 +5108,7 @@ Qed.
 
 Lemma subst_typ_in_ftyp_fresh_eq_mutual :
 (forall A2 A1 X1,
-  X1 `notin` fv_ftyp_in_ftyp A2 ->
+  X1 `notin` ftvar_in_ftyp A2 ->
   subst_typ_in_ftyp A1 X1 A2 = A2).
 Proof.
 apply_mutual_ind ftyp_mutind;
@@ -5119,7 +5119,7 @@ Qed.
 
 Lemma subst_typ_in_ftyp_fresh_eq :
 forall A2 A1 X1,
-  X1 `notin` fv_ftyp_in_ftyp A2 ->
+  X1 `notin` ftvar_in_ftyp A2 ->
   subst_typ_in_ftyp A1 X1 A2 = A2.
 Proof.
 pose proof subst_typ_in_ftyp_fresh_eq_mutual as H; intuition eauto.
@@ -5132,7 +5132,7 @@ Qed.
 
 Lemma subst_typ_in_fexp_fresh_eq_mutual :
 (forall e1 A1 X1,
-  X1 `notin` fv_ftyp_in_fexp e1 ->
+  X1 `notin` ftvar_in_fexp e1 ->
   subst_typ_in_fexp A1 X1 e1 = e1).
 Proof.
 apply_mutual_ind fexp_mutind;
@@ -5143,7 +5143,7 @@ Qed.
 
 Lemma subst_typ_in_fexp_fresh_eq :
 forall e1 A1 X1,
-  X1 `notin` fv_ftyp_in_fexp e1 ->
+  X1 `notin` ftvar_in_fexp e1 ->
   subst_typ_in_fexp A1 X1 e1 = e1.
 Proof.
 pose proof subst_typ_in_fexp_fresh_eq_mutual as H; intuition eauto.
@@ -5156,7 +5156,7 @@ Qed.
 
 Lemma subst_exp_in_fexp_fresh_eq_mutual :
 (forall e2 e1 x1,
-  x1 `notin` fv_fexp_in_fexp e2 ->
+  x1 `notin` fvar_in_fexp e2 ->
   subst_exp_in_fexp e1 x1 e2 = e2).
 Proof.
 apply_mutual_ind fexp_mutind;
@@ -5167,7 +5167,7 @@ Qed.
 
 Lemma subst_exp_in_fexp_fresh_eq :
 forall e2 e1 x1,
-  x1 `notin` fv_fexp_in_fexp e2 ->
+  x1 `notin` fvar_in_fexp e2 ->
   subst_exp_in_fexp e1 x1 e2 = e2.
 Proof.
 pose proof subst_exp_in_fexp_fresh_eq_mutual as H; intuition eauto.
@@ -5180,7 +5180,7 @@ Qed.
 
 Lemma subst_typ_in_fbind_fresh_eq_mutual :
 (forall fb1 A1 X1,
-  X1 `notin` fv_ftyp_in_fbind fb1 ->
+  X1 `notin` ftvar_in_fbind fb1 ->
   subst_typ_in_fbind A1 X1 fb1 = fb1).
 Proof.
 apply_mutual_ind fbind_mutind;
@@ -5191,7 +5191,7 @@ Qed.
 
 Lemma subst_typ_in_fbind_fresh_eq :
 forall fb1 A1 X1,
-  X1 `notin` fv_ftyp_in_fbind fb1 ->
+  X1 `notin` ftvar_in_fbind fb1 ->
   subst_typ_in_fbind A1 X1 fb1 = fb1.
 Proof.
 pose proof subst_typ_in_fbind_fresh_eq_mutual as H; intuition eauto.
@@ -5204,8 +5204,8 @@ Qed.
 
 Lemma subst_typ_in_ftyp_fresh_same_mutual :
 (forall A2 A1 X1,
-  X1 `notin` fv_ftyp_in_ftyp A1 ->
-  X1 `notin` fv_ftyp_in_ftyp (subst_typ_in_ftyp A1 X1 A2)).
+  X1 `notin` ftvar_in_ftyp A1 ->
+  X1 `notin` ftvar_in_ftyp (subst_typ_in_ftyp A1 X1 A2)).
 Proof.
 apply_mutual_ind ftyp_mutind;
 default_simp.
@@ -5215,8 +5215,8 @@ Qed.
 
 Lemma subst_typ_in_ftyp_fresh_same :
 forall A2 A1 X1,
-  X1 `notin` fv_ftyp_in_ftyp A1 ->
-  X1 `notin` fv_ftyp_in_ftyp (subst_typ_in_ftyp A1 X1 A2).
+  X1 `notin` ftvar_in_ftyp A1 ->
+  X1 `notin` ftvar_in_ftyp (subst_typ_in_ftyp A1 X1 A2).
 Proof.
 pose proof subst_typ_in_ftyp_fresh_same_mutual as H; intuition eauto.
 Qed.
@@ -5227,8 +5227,8 @@ Qed.
 
 Lemma subst_typ_in_fexp_fresh_same_mutual :
 (forall e1 A1 X1,
-  X1 `notin` fv_ftyp_in_ftyp A1 ->
-  X1 `notin` fv_ftyp_in_fexp (subst_typ_in_fexp A1 X1 e1)).
+  X1 `notin` ftvar_in_ftyp A1 ->
+  X1 `notin` ftvar_in_fexp (subst_typ_in_fexp A1 X1 e1)).
 Proof.
 apply_mutual_ind fexp_mutind;
 default_simp.
@@ -5238,8 +5238,8 @@ Qed.
 
 Lemma subst_typ_in_fexp_fresh_same :
 forall e1 A1 X1,
-  X1 `notin` fv_ftyp_in_ftyp A1 ->
-  X1 `notin` fv_ftyp_in_fexp (subst_typ_in_fexp A1 X1 e1).
+  X1 `notin` ftvar_in_ftyp A1 ->
+  X1 `notin` ftvar_in_fexp (subst_typ_in_fexp A1 X1 e1).
 Proof.
 pose proof subst_typ_in_fexp_fresh_same_mutual as H; intuition eauto.
 Qed.
@@ -5250,8 +5250,8 @@ Qed.
 
 Lemma subst_exp_in_fexp_fresh_same_mutual :
 (forall e2 e1 x1,
-  x1 `notin` fv_fexp_in_fexp e1 ->
-  x1 `notin` fv_fexp_in_fexp (subst_exp_in_fexp e1 x1 e2)).
+  x1 `notin` fvar_in_fexp e1 ->
+  x1 `notin` fvar_in_fexp (subst_exp_in_fexp e1 x1 e2)).
 Proof.
 apply_mutual_ind fexp_mutind;
 default_simp.
@@ -5261,8 +5261,8 @@ Qed.
 
 Lemma subst_exp_in_fexp_fresh_same :
 forall e2 e1 x1,
-  x1 `notin` fv_fexp_in_fexp e1 ->
-  x1 `notin` fv_fexp_in_fexp (subst_exp_in_fexp e1 x1 e2).
+  x1 `notin` fvar_in_fexp e1 ->
+  x1 `notin` fvar_in_fexp (subst_exp_in_fexp e1 x1 e2).
 Proof.
 pose proof subst_exp_in_fexp_fresh_same_mutual as H; intuition eauto.
 Qed.
@@ -5273,8 +5273,8 @@ Qed.
 
 Lemma subst_typ_in_fbind_fresh_same_mutual :
 (forall fb1 A1 X1,
-  X1 `notin` fv_ftyp_in_ftyp A1 ->
-  X1 `notin` fv_ftyp_in_fbind (subst_typ_in_fbind A1 X1 fb1)).
+  X1 `notin` ftvar_in_ftyp A1 ->
+  X1 `notin` ftvar_in_fbind (subst_typ_in_fbind A1 X1 fb1)).
 Proof.
 apply_mutual_ind fbind_mutind;
 default_simp.
@@ -5284,8 +5284,8 @@ Qed.
 
 Lemma subst_typ_in_fbind_fresh_same :
 forall fb1 A1 X1,
-  X1 `notin` fv_ftyp_in_ftyp A1 ->
-  X1 `notin` fv_ftyp_in_fbind (subst_typ_in_fbind A1 X1 fb1).
+  X1 `notin` ftvar_in_ftyp A1 ->
+  X1 `notin` ftvar_in_fbind (subst_typ_in_fbind A1 X1 fb1).
 Proof.
 pose proof subst_typ_in_fbind_fresh_same_mutual as H; intuition eauto.
 Qed.
@@ -5296,9 +5296,9 @@ Qed.
 
 Lemma subst_typ_in_ftyp_fresh_mutual :
 (forall A2 A1 X1 X2,
-  X1 `notin` fv_ftyp_in_ftyp A2 ->
-  X1 `notin` fv_ftyp_in_ftyp A1 ->
-  X1 `notin` fv_ftyp_in_ftyp (subst_typ_in_ftyp A1 X2 A2)).
+  X1 `notin` ftvar_in_ftyp A2 ->
+  X1 `notin` ftvar_in_ftyp A1 ->
+  X1 `notin` ftvar_in_ftyp (subst_typ_in_ftyp A1 X2 A2)).
 Proof.
 apply_mutual_ind ftyp_mutind;
 default_simp.
@@ -5308,9 +5308,9 @@ Qed.
 
 Lemma subst_typ_in_ftyp_fresh :
 forall A2 A1 X1 X2,
-  X1 `notin` fv_ftyp_in_ftyp A2 ->
-  X1 `notin` fv_ftyp_in_ftyp A1 ->
-  X1 `notin` fv_ftyp_in_ftyp (subst_typ_in_ftyp A1 X2 A2).
+  X1 `notin` ftvar_in_ftyp A2 ->
+  X1 `notin` ftvar_in_ftyp A1 ->
+  X1 `notin` ftvar_in_ftyp (subst_typ_in_ftyp A1 X2 A2).
 Proof.
 pose proof subst_typ_in_ftyp_fresh_mutual as H; intuition eauto.
 Qed.
@@ -5321,9 +5321,9 @@ Qed.
 
 Lemma subst_typ_in_fexp_fresh_mutual :
 (forall e1 A1 X1 X2,
-  X1 `notin` fv_ftyp_in_fexp e1 ->
-  X1 `notin` fv_ftyp_in_ftyp A1 ->
-  X1 `notin` fv_ftyp_in_fexp (subst_typ_in_fexp A1 X2 e1)).
+  X1 `notin` ftvar_in_fexp e1 ->
+  X1 `notin` ftvar_in_ftyp A1 ->
+  X1 `notin` ftvar_in_fexp (subst_typ_in_fexp A1 X2 e1)).
 Proof.
 apply_mutual_ind fexp_mutind;
 default_simp.
@@ -5333,9 +5333,9 @@ Qed.
 
 Lemma subst_typ_in_fexp_fresh :
 forall e1 A1 X1 X2,
-  X1 `notin` fv_ftyp_in_fexp e1 ->
-  X1 `notin` fv_ftyp_in_ftyp A1 ->
-  X1 `notin` fv_ftyp_in_fexp (subst_typ_in_fexp A1 X2 e1).
+  X1 `notin` ftvar_in_fexp e1 ->
+  X1 `notin` ftvar_in_ftyp A1 ->
+  X1 `notin` ftvar_in_fexp (subst_typ_in_fexp A1 X2 e1).
 Proof.
 pose proof subst_typ_in_fexp_fresh_mutual as H; intuition eauto.
 Qed.
@@ -5346,9 +5346,9 @@ Qed.
 
 Lemma subst_exp_in_fexp_fresh_mutual :
 (forall e2 e1 x1 x2,
-  x1 `notin` fv_fexp_in_fexp e2 ->
-  x1 `notin` fv_fexp_in_fexp e1 ->
-  x1 `notin` fv_fexp_in_fexp (subst_exp_in_fexp e1 x2 e2)).
+  x1 `notin` fvar_in_fexp e2 ->
+  x1 `notin` fvar_in_fexp e1 ->
+  x1 `notin` fvar_in_fexp (subst_exp_in_fexp e1 x2 e2)).
 Proof.
 apply_mutual_ind fexp_mutind;
 default_simp.
@@ -5358,9 +5358,9 @@ Qed.
 
 Lemma subst_exp_in_fexp_fresh :
 forall e2 e1 x1 x2,
-  x1 `notin` fv_fexp_in_fexp e2 ->
-  x1 `notin` fv_fexp_in_fexp e1 ->
-  x1 `notin` fv_fexp_in_fexp (subst_exp_in_fexp e1 x2 e2).
+  x1 `notin` fvar_in_fexp e2 ->
+  x1 `notin` fvar_in_fexp e1 ->
+  x1 `notin` fvar_in_fexp (subst_exp_in_fexp e1 x2 e2).
 Proof.
 pose proof subst_exp_in_fexp_fresh_mutual as H; intuition eauto.
 Qed.
@@ -5371,9 +5371,9 @@ Qed.
 
 Lemma subst_typ_in_fbind_fresh_mutual :
 (forall fb1 A1 X1 X2,
-  X1 `notin` fv_ftyp_in_fbind fb1 ->
-  X1 `notin` fv_ftyp_in_ftyp A1 ->
-  X1 `notin` fv_ftyp_in_fbind (subst_typ_in_fbind A1 X2 fb1)).
+  X1 `notin` ftvar_in_fbind fb1 ->
+  X1 `notin` ftvar_in_ftyp A1 ->
+  X1 `notin` ftvar_in_fbind (subst_typ_in_fbind A1 X2 fb1)).
 Proof.
 apply_mutual_ind fbind_mutind;
 default_simp.
@@ -5383,9 +5383,9 @@ Qed.
 
 Lemma subst_typ_in_fbind_fresh :
 forall fb1 A1 X1 X2,
-  X1 `notin` fv_ftyp_in_fbind fb1 ->
-  X1 `notin` fv_ftyp_in_ftyp A1 ->
-  X1 `notin` fv_ftyp_in_fbind (subst_typ_in_fbind A1 X2 fb1).
+  X1 `notin` ftvar_in_fbind fb1 ->
+  X1 `notin` ftvar_in_ftyp A1 ->
+  X1 `notin` ftvar_in_fbind (subst_typ_in_fbind A1 X2 fb1).
 Proof.
 pose proof subst_typ_in_fbind_fresh_mutual as H; intuition eauto.
 Qed.
@@ -5858,7 +5858,7 @@ Qed.
 
 Lemma subst_typ_in_ftyp_subst_typ_in_ftyp_mutual :
 (forall A1 A2 A3 X2 X1,
-  X2 `notin` fv_ftyp_in_ftyp A2 ->
+  X2 `notin` ftvar_in_ftyp A2 ->
   X2 <> X1 ->
   subst_typ_in_ftyp A2 X1 (subst_typ_in_ftyp A3 X2 A1) = subst_typ_in_ftyp (subst_typ_in_ftyp A2 X1 A3) X2 (subst_typ_in_ftyp A2 X1 A1)).
 Proof.
@@ -5870,7 +5870,7 @@ Qed.
 
 Lemma subst_typ_in_ftyp_subst_typ_in_ftyp :
 forall A1 A2 A3 X2 X1,
-  X2 `notin` fv_ftyp_in_ftyp A2 ->
+  X2 `notin` ftvar_in_ftyp A2 ->
   X2 <> X1 ->
   subst_typ_in_ftyp A2 X1 (subst_typ_in_ftyp A3 X2 A1) = subst_typ_in_ftyp (subst_typ_in_ftyp A2 X1 A3) X2 (subst_typ_in_ftyp A2 X1 A1).
 Proof.
@@ -5883,7 +5883,7 @@ Qed.
 
 Lemma subst_typ_in_fexp_subst_typ_in_fexp_mutual :
 (forall e1 A1 A2 X2 X1,
-  X2 `notin` fv_ftyp_in_ftyp A1 ->
+  X2 `notin` ftvar_in_ftyp A1 ->
   X2 <> X1 ->
   subst_typ_in_fexp A1 X1 (subst_typ_in_fexp A2 X2 e1) = subst_typ_in_fexp (subst_typ_in_ftyp A1 X1 A2) X2 (subst_typ_in_fexp A1 X1 e1)).
 Proof.
@@ -5895,7 +5895,7 @@ Qed.
 
 Lemma subst_typ_in_fexp_subst_typ_in_fexp :
 forall e1 A1 A2 X2 X1,
-  X2 `notin` fv_ftyp_in_ftyp A1 ->
+  X2 `notin` ftvar_in_ftyp A1 ->
   X2 <> X1 ->
   subst_typ_in_fexp A1 X1 (subst_typ_in_fexp A2 X2 e1) = subst_typ_in_fexp (subst_typ_in_ftyp A1 X1 A2) X2 (subst_typ_in_fexp A1 X1 e1).
 Proof.
@@ -5929,7 +5929,7 @@ Qed.
 
 Lemma subst_exp_in_fexp_subst_typ_in_fexp_mutual :
 (forall e1 e2 A1 X1 x1,
-  X1 `notin` fv_ftyp_in_fexp e2 ->
+  X1 `notin` ftvar_in_fexp e2 ->
   subst_exp_in_fexp e2 x1 (subst_typ_in_fexp A1 X1 e1) = subst_typ_in_fexp A1 X1 (subst_exp_in_fexp e2 x1 e1)).
 Proof.
 apply_mutual_ind fexp_mutind;
@@ -5940,7 +5940,7 @@ Qed.
 
 Lemma subst_exp_in_fexp_subst_typ_in_fexp :
 forall e1 e2 A1 X1 x1,
-  X1 `notin` fv_ftyp_in_fexp e2 ->
+  X1 `notin` ftvar_in_fexp e2 ->
   subst_exp_in_fexp e2 x1 (subst_typ_in_fexp A1 X1 e1) = subst_typ_in_fexp A1 X1 (subst_exp_in_fexp e2 x1 e1).
 Proof.
 pose proof subst_exp_in_fexp_subst_typ_in_fexp_mutual as H; intuition eauto.
@@ -5952,7 +5952,7 @@ Qed.
 
 Lemma subst_exp_in_fexp_subst_exp_in_fexp_mutual :
 (forall e1 e2 e3 x2 x1,
-  x2 `notin` fv_fexp_in_fexp e2 ->
+  x2 `notin` fvar_in_fexp e2 ->
   x2 <> x1 ->
   subst_exp_in_fexp e2 x1 (subst_exp_in_fexp e3 x2 e1) = subst_exp_in_fexp (subst_exp_in_fexp e2 x1 e3) x2 (subst_exp_in_fexp e2 x1 e1)).
 Proof.
@@ -5964,7 +5964,7 @@ Qed.
 
 Lemma subst_exp_in_fexp_subst_exp_in_fexp :
 forall e1 e2 e3 x2 x1,
-  x2 `notin` fv_fexp_in_fexp e2 ->
+  x2 `notin` fvar_in_fexp e2 ->
   x2 <> x1 ->
   subst_exp_in_fexp e2 x1 (subst_exp_in_fexp e3 x2 e1) = subst_exp_in_fexp (subst_exp_in_fexp e2 x1 e3) x2 (subst_exp_in_fexp e2 x1 e1).
 Proof.
@@ -5977,7 +5977,7 @@ Qed.
 
 Lemma subst_typ_in_fbind_subst_typ_in_fbind_mutual :
 (forall fb1 A1 A2 X2 X1,
-  X2 `notin` fv_ftyp_in_ftyp A1 ->
+  X2 `notin` ftvar_in_ftyp A1 ->
   X2 <> X1 ->
   subst_typ_in_fbind A1 X1 (subst_typ_in_fbind A2 X2 fb1) = subst_typ_in_fbind (subst_typ_in_ftyp A1 X1 A2) X2 (subst_typ_in_fbind A1 X1 fb1)).
 Proof.
@@ -5989,7 +5989,7 @@ Qed.
 
 Lemma subst_typ_in_fbind_subst_typ_in_fbind :
 forall fb1 A1 A2 X2 X1,
-  X2 `notin` fv_ftyp_in_ftyp A1 ->
+  X2 `notin` ftvar_in_ftyp A1 ->
   X2 <> X1 ->
   subst_typ_in_fbind A1 X1 (subst_typ_in_fbind A2 X2 fb1) = subst_typ_in_fbind (subst_typ_in_ftyp A1 X1 A2) X2 (subst_typ_in_fbind A1 X1 fb1).
 Proof.
@@ -6002,8 +6002,8 @@ Qed.
 
 Lemma subst_typ_in_ftyp_close_ftyp_wrt_ftyp_rec_open_ftyp_wrt_ftyp_rec_mutual :
 (forall A2 A1 X1 X2 n1,
-  X2 `notin` fv_ftyp_in_ftyp A2 ->
-  X2 `notin` fv_ftyp_in_ftyp A1 ->
+  X2 `notin` ftvar_in_ftyp A2 ->
+  X2 `notin` ftvar_in_ftyp A1 ->
   X2 <> X1 ->
   degree_ftyp_wrt_ftyp n1 A1 ->
   subst_typ_in_ftyp A1 X1 A2 = close_ftyp_wrt_ftyp_rec n1 X2 (subst_typ_in_ftyp A1 X1 (open_ftyp_wrt_ftyp_rec n1 (ftyp_var_f X2) A2))).
@@ -6018,8 +6018,8 @@ Qed.
 
 Lemma subst_typ_in_ftyp_close_ftyp_wrt_ftyp_rec_open_ftyp_wrt_ftyp_rec :
 forall A2 A1 X1 X2 n1,
-  X2 `notin` fv_ftyp_in_ftyp A2 ->
-  X2 `notin` fv_ftyp_in_ftyp A1 ->
+  X2 `notin` ftvar_in_ftyp A2 ->
+  X2 `notin` ftvar_in_ftyp A1 ->
   X2 <> X1 ->
   degree_ftyp_wrt_ftyp n1 A1 ->
   subst_typ_in_ftyp A1 X1 A2 = close_ftyp_wrt_ftyp_rec n1 X2 (subst_typ_in_ftyp A1 X1 (open_ftyp_wrt_ftyp_rec n1 (ftyp_var_f X2) A2)).
@@ -6035,8 +6035,8 @@ Qed.
 
 Lemma subst_typ_in_fexp_close_fexp_wrt_ftyp_rec_open_fexp_wrt_ftyp_rec_mutual :
 (forall e1 A1 X1 X2 n1,
-  X2 `notin` fv_ftyp_in_fexp e1 ->
-  X2 `notin` fv_ftyp_in_ftyp A1 ->
+  X2 `notin` ftvar_in_fexp e1 ->
+  X2 `notin` ftvar_in_ftyp A1 ->
   X2 <> X1 ->
   degree_ftyp_wrt_ftyp n1 A1 ->
   subst_typ_in_fexp A1 X1 e1 = close_fexp_wrt_ftyp_rec n1 X2 (subst_typ_in_fexp A1 X1 (open_fexp_wrt_ftyp_rec n1 (ftyp_var_f X2) e1))).
@@ -6051,8 +6051,8 @@ Qed.
 
 Lemma subst_typ_in_fexp_close_fexp_wrt_ftyp_rec_open_fexp_wrt_ftyp_rec :
 forall e1 A1 X1 X2 n1,
-  X2 `notin` fv_ftyp_in_fexp e1 ->
-  X2 `notin` fv_ftyp_in_ftyp A1 ->
+  X2 `notin` ftvar_in_fexp e1 ->
+  X2 `notin` ftvar_in_ftyp A1 ->
   X2 <> X1 ->
   degree_ftyp_wrt_ftyp n1 A1 ->
   subst_typ_in_fexp A1 X1 e1 = close_fexp_wrt_ftyp_rec n1 X2 (subst_typ_in_fexp A1 X1 (open_fexp_wrt_ftyp_rec n1 (ftyp_var_f X2) e1)).
@@ -6068,7 +6068,7 @@ Qed.
 
 Lemma subst_typ_in_fexp_close_fexp_wrt_fexp_rec_open_fexp_wrt_fexp_rec_mutual :
 (forall e1 A1 X1 x1 n1,
-  x1 `notin` fv_fexp_in_fexp e1 ->
+  x1 `notin` fvar_in_fexp e1 ->
   subst_typ_in_fexp A1 X1 e1 = close_fexp_wrt_fexp_rec n1 x1 (subst_typ_in_fexp A1 X1 (open_fexp_wrt_fexp_rec n1 (fexp_var_f x1) e1))).
 Proof.
 apply_mutual_ind fexp_mutrec;
@@ -6081,7 +6081,7 @@ Qed.
 
 Lemma subst_typ_in_fexp_close_fexp_wrt_fexp_rec_open_fexp_wrt_fexp_rec :
 forall e1 A1 X1 x1 n1,
-  x1 `notin` fv_fexp_in_fexp e1 ->
+  x1 `notin` fvar_in_fexp e1 ->
   subst_typ_in_fexp A1 X1 e1 = close_fexp_wrt_fexp_rec n1 x1 (subst_typ_in_fexp A1 X1 (open_fexp_wrt_fexp_rec n1 (fexp_var_f x1) e1)).
 Proof.
 pose proof subst_typ_in_fexp_close_fexp_wrt_fexp_rec_open_fexp_wrt_fexp_rec_mutual as H; intuition eauto.
@@ -6095,8 +6095,8 @@ Qed.
 
 Lemma subst_exp_in_fexp_close_fexp_wrt_ftyp_rec_open_fexp_wrt_ftyp_rec_mutual :
 (forall e2 e1 x1 X1 n1,
-  X1 `notin` fv_ftyp_in_fexp e2 ->
-  X1 `notin` fv_ftyp_in_fexp e1 ->
+  X1 `notin` ftvar_in_fexp e2 ->
+  X1 `notin` ftvar_in_fexp e1 ->
   degree_fexp_wrt_ftyp n1 e1 ->
   subst_exp_in_fexp e1 x1 e2 = close_fexp_wrt_ftyp_rec n1 X1 (subst_exp_in_fexp e1 x1 (open_fexp_wrt_ftyp_rec n1 (ftyp_var_f X1) e2))).
 Proof.
@@ -6110,8 +6110,8 @@ Qed.
 
 Lemma subst_exp_in_fexp_close_fexp_wrt_ftyp_rec_open_fexp_wrt_ftyp_rec :
 forall e2 e1 x1 X1 n1,
-  X1 `notin` fv_ftyp_in_fexp e2 ->
-  X1 `notin` fv_ftyp_in_fexp e1 ->
+  X1 `notin` ftvar_in_fexp e2 ->
+  X1 `notin` ftvar_in_fexp e1 ->
   degree_fexp_wrt_ftyp n1 e1 ->
   subst_exp_in_fexp e1 x1 e2 = close_fexp_wrt_ftyp_rec n1 X1 (subst_exp_in_fexp e1 x1 (open_fexp_wrt_ftyp_rec n1 (ftyp_var_f X1) e2)).
 Proof.
@@ -6126,8 +6126,8 @@ Qed.
 
 Lemma subst_exp_in_fexp_close_fexp_wrt_fexp_rec_open_fexp_wrt_fexp_rec_mutual :
 (forall e2 e1 x1 x2 n1,
-  x2 `notin` fv_fexp_in_fexp e2 ->
-  x2 `notin` fv_fexp_in_fexp e1 ->
+  x2 `notin` fvar_in_fexp e2 ->
+  x2 `notin` fvar_in_fexp e1 ->
   x2 <> x1 ->
   degree_fexp_wrt_fexp n1 e1 ->
   subst_exp_in_fexp e1 x1 e2 = close_fexp_wrt_fexp_rec n1 x2 (subst_exp_in_fexp e1 x1 (open_fexp_wrt_fexp_rec n1 (fexp_var_f x2) e2))).
@@ -6142,8 +6142,8 @@ Qed.
 
 Lemma subst_exp_in_fexp_close_fexp_wrt_fexp_rec_open_fexp_wrt_fexp_rec :
 forall e2 e1 x1 x2 n1,
-  x2 `notin` fv_fexp_in_fexp e2 ->
-  x2 `notin` fv_fexp_in_fexp e1 ->
+  x2 `notin` fvar_in_fexp e2 ->
+  x2 `notin` fvar_in_fexp e1 ->
   x2 <> x1 ->
   degree_fexp_wrt_fexp n1 e1 ->
   subst_exp_in_fexp e1 x1 e2 = close_fexp_wrt_fexp_rec n1 x2 (subst_exp_in_fexp e1 x1 (open_fexp_wrt_fexp_rec n1 (fexp_var_f x2) e2)).
@@ -6159,8 +6159,8 @@ Qed.
 
 Lemma subst_typ_in_fbind_close_fbind_wrt_ftyp_rec_open_fbind_wrt_ftyp_rec_mutual :
 (forall fb1 A1 X1 X2 n1,
-  X2 `notin` fv_ftyp_in_fbind fb1 ->
-  X2 `notin` fv_ftyp_in_ftyp A1 ->
+  X2 `notin` ftvar_in_fbind fb1 ->
+  X2 `notin` ftvar_in_ftyp A1 ->
   X2 <> X1 ->
   degree_ftyp_wrt_ftyp n1 A1 ->
   subst_typ_in_fbind A1 X1 fb1 = close_fbind_wrt_ftyp_rec n1 X2 (subst_typ_in_fbind A1 X1 (open_fbind_wrt_ftyp_rec n1 (ftyp_var_f X2) fb1))).
@@ -6175,8 +6175,8 @@ Qed.
 
 Lemma subst_typ_in_fbind_close_fbind_wrt_ftyp_rec_open_fbind_wrt_ftyp_rec :
 forall fb1 A1 X1 X2 n1,
-  X2 `notin` fv_ftyp_in_fbind fb1 ->
-  X2 `notin` fv_ftyp_in_ftyp A1 ->
+  X2 `notin` ftvar_in_fbind fb1 ->
+  X2 `notin` ftvar_in_ftyp A1 ->
   X2 <> X1 ->
   degree_ftyp_wrt_ftyp n1 A1 ->
   subst_typ_in_fbind A1 X1 fb1 = close_fbind_wrt_ftyp_rec n1 X2 (subst_typ_in_fbind A1 X1 (open_fbind_wrt_ftyp_rec n1 (ftyp_var_f X2) fb1)).
@@ -6190,8 +6190,8 @@ Qed.
 
 Lemma subst_typ_in_ftyp_close_ftyp_wrt_ftyp_open_ftyp_wrt_ftyp :
 forall A2 A1 X1 X2,
-  X2 `notin` fv_ftyp_in_ftyp A2 ->
-  X2 `notin` fv_ftyp_in_ftyp A1 ->
+  X2 `notin` ftvar_in_ftyp A2 ->
+  X2 `notin` ftvar_in_ftyp A1 ->
   X2 <> X1 ->
   lc_ftyp A1 ->
   subst_typ_in_ftyp A1 X1 A2 = close_ftyp_wrt_ftyp X2 (subst_typ_in_ftyp A1 X1 (open_ftyp_wrt_ftyp A2 (ftyp_var_f X2))).
@@ -6203,8 +6203,8 @@ Qed.
 
 Lemma subst_typ_in_fexp_close_fexp_wrt_ftyp_open_fexp_wrt_ftyp :
 forall e1 A1 X1 X2,
-  X2 `notin` fv_ftyp_in_fexp e1 ->
-  X2 `notin` fv_ftyp_in_ftyp A1 ->
+  X2 `notin` ftvar_in_fexp e1 ->
+  X2 `notin` ftvar_in_ftyp A1 ->
   X2 <> X1 ->
   lc_ftyp A1 ->
   subst_typ_in_fexp A1 X1 e1 = close_fexp_wrt_ftyp X2 (subst_typ_in_fexp A1 X1 (open_fexp_wrt_ftyp e1 (ftyp_var_f X2))).
@@ -6216,7 +6216,7 @@ Qed.
 
 Lemma subst_typ_in_fexp_close_fexp_wrt_fexp_open_fexp_wrt_fexp :
 forall e1 A1 X1 x1,
-  x1 `notin` fv_fexp_in_fexp e1 ->
+  x1 `notin` fvar_in_fexp e1 ->
   lc_ftyp A1 ->
   subst_typ_in_fexp A1 X1 e1 = close_fexp_wrt_fexp x1 (subst_typ_in_fexp A1 X1 (open_fexp_wrt_fexp e1 (fexp_var_f x1))).
 Proof.
@@ -6227,8 +6227,8 @@ Qed.
 
 Lemma subst_exp_in_fexp_close_fexp_wrt_ftyp_open_fexp_wrt_ftyp :
 forall e2 e1 x1 X1,
-  X1 `notin` fv_ftyp_in_fexp e2 ->
-  X1 `notin` fv_ftyp_in_fexp e1 ->
+  X1 `notin` ftvar_in_fexp e2 ->
+  X1 `notin` ftvar_in_fexp e1 ->
   lc_fexp e1 ->
   subst_exp_in_fexp e1 x1 e2 = close_fexp_wrt_ftyp X1 (subst_exp_in_fexp e1 x1 (open_fexp_wrt_ftyp e2 (ftyp_var_f X1))).
 Proof.
@@ -6239,8 +6239,8 @@ Qed.
 
 Lemma subst_exp_in_fexp_close_fexp_wrt_fexp_open_fexp_wrt_fexp :
 forall e2 e1 x1 x2,
-  x2 `notin` fv_fexp_in_fexp e2 ->
-  x2 `notin` fv_fexp_in_fexp e1 ->
+  x2 `notin` fvar_in_fexp e2 ->
+  x2 `notin` fvar_in_fexp e1 ->
   x2 <> x1 ->
   lc_fexp e1 ->
   subst_exp_in_fexp e1 x1 e2 = close_fexp_wrt_fexp x2 (subst_exp_in_fexp e1 x1 (open_fexp_wrt_fexp e2 (fexp_var_f x2))).
@@ -6252,8 +6252,8 @@ Qed.
 
 Lemma subst_typ_in_fbind_close_fbind_wrt_ftyp_open_fbind_wrt_ftyp :
 forall fb1 A1 X1 X2,
-  X2 `notin` fv_ftyp_in_fbind fb1 ->
-  X2 `notin` fv_ftyp_in_ftyp A1 ->
+  X2 `notin` ftvar_in_fbind fb1 ->
+  X2 `notin` ftvar_in_ftyp A1 ->
   X2 <> X1 ->
   lc_ftyp A1 ->
   subst_typ_in_fbind A1 X1 fb1 = close_fbind_wrt_ftyp X2 (subst_typ_in_fbind A1 X1 (open_fbind_wrt_ftyp fb1 (ftyp_var_f X2))).
@@ -6266,7 +6266,7 @@ Qed.
 Lemma subst_typ_in_ftyp_ftyp_all :
 forall X2 A2 A1 X1,
   lc_ftyp A1 ->
-  X2 `notin` fv_ftyp_in_ftyp A1 `union` fv_ftyp_in_ftyp A2 `union` singleton X1 ->
+  X2 `notin` ftvar_in_ftyp A1 `union` ftvar_in_ftyp A2 `union` singleton X1 ->
   subst_typ_in_ftyp A1 X1 (ftyp_all A2) = ftyp_all (close_ftyp_wrt_ftyp X2 (subst_typ_in_ftyp A1 X1 (open_ftyp_wrt_ftyp A2 (ftyp_var_f X2)))).
 Proof.
 default_simp.
@@ -6277,7 +6277,7 @@ Qed.
 Lemma subst_typ_in_fexp_fexp_abs :
 forall x1 A2 e1 A1 X1,
   lc_ftyp A1 ->
-  x1 `notin` fv_fexp_in_fexp e1 ->
+  x1 `notin` fvar_in_fexp e1 ->
   subst_typ_in_fexp A1 X1 (fexp_abs A2 e1) = fexp_abs (subst_typ_in_ftyp A1 X1 A2) (close_fexp_wrt_fexp x1 (subst_typ_in_fexp A1 X1 (open_fexp_wrt_fexp e1 (fexp_var_f x1)))).
 Proof.
 default_simp.
@@ -6288,7 +6288,7 @@ Qed.
 Lemma subst_typ_in_fexp_fexp_tabs :
 forall X2 e1 A1 X1,
   lc_ftyp A1 ->
-  X2 `notin` fv_ftyp_in_ftyp A1 `union` fv_ftyp_in_fexp e1 `union` singleton X1 ->
+  X2 `notin` ftvar_in_ftyp A1 `union` ftvar_in_fexp e1 `union` singleton X1 ->
   subst_typ_in_fexp A1 X1 (fexp_tabs e1) = fexp_tabs (close_fexp_wrt_ftyp X2 (subst_typ_in_fexp A1 X1 (open_fexp_wrt_ftyp e1 (ftyp_var_f X2)))).
 Proof.
 default_simp.
@@ -6299,8 +6299,8 @@ Qed.
 Lemma subst_typ_in_fexp_fexp_case :
 forall x1 y1 e1 e2 e3 A1 X1,
   lc_ftyp A1 ->
-  x1 `notin` fv_fexp_in_fexp e2 ->
-  y1 `notin` fv_fexp_in_fexp e3 ->
+  x1 `notin` fvar_in_fexp e2 ->
+  y1 `notin` fvar_in_fexp e3 ->
   subst_typ_in_fexp A1 X1 (fexp_case e1 e2 e3) = fexp_case (subst_typ_in_fexp A1 X1 e1) (close_fexp_wrt_fexp x1 (subst_typ_in_fexp A1 X1 (open_fexp_wrt_fexp e2 (fexp_var_f x1)))) (close_fexp_wrt_fexp y1 (subst_typ_in_fexp A1 X1 (open_fexp_wrt_fexp e3 (fexp_var_f y1)))).
 Proof.
 default_simp.
@@ -6311,7 +6311,7 @@ Qed.
 Lemma subst_exp_in_fexp_fexp_abs :
 forall x2 A1 e2 e1 x1,
   lc_fexp e1 ->
-  x2 `notin` fv_fexp_in_fexp e1 `union` fv_fexp_in_fexp e2 `union` singleton x1 ->
+  x2 `notin` fvar_in_fexp e1 `union` fvar_in_fexp e2 `union` singleton x1 ->
   subst_exp_in_fexp e1 x1 (fexp_abs A1 e2) = fexp_abs (A1) (close_fexp_wrt_fexp x2 (subst_exp_in_fexp e1 x1 (open_fexp_wrt_fexp e2 (fexp_var_f x2)))).
 Proof.
 default_simp.
@@ -6322,7 +6322,7 @@ Qed.
 Lemma subst_exp_in_fexp_fexp_tabs :
 forall X1 e2 e1 x1,
   lc_fexp e1 ->
-  X1 `notin` fv_ftyp_in_fexp e1 `union` fv_ftyp_in_fexp e2 ->
+  X1 `notin` ftvar_in_fexp e1 `union` ftvar_in_fexp e2 ->
   subst_exp_in_fexp e1 x1 (fexp_tabs e2) = fexp_tabs (close_fexp_wrt_ftyp X1 (subst_exp_in_fexp e1 x1 (open_fexp_wrt_ftyp e2 (ftyp_var_f X1)))).
 Proof.
 default_simp.
@@ -6333,8 +6333,8 @@ Qed.
 Lemma subst_exp_in_fexp_fexp_case :
 forall x2 y1 e2 e3 e4 e1 x1,
   lc_fexp e1 ->
-  x2 `notin` fv_fexp_in_fexp e1 `union` fv_fexp_in_fexp e3 `union` singleton x1 ->
-  y1 `notin` fv_fexp_in_fexp e1 `union` fv_fexp_in_fexp e4 `union` singleton x1 ->
+  x2 `notin` fvar_in_fexp e1 `union` fvar_in_fexp e3 `union` singleton x1 ->
+  y1 `notin` fvar_in_fexp e1 `union` fvar_in_fexp e4 `union` singleton x1 ->
   subst_exp_in_fexp e1 x1 (fexp_case e2 e3 e4) = fexp_case (subst_exp_in_fexp e1 x1 e2) (close_fexp_wrt_fexp x2 (subst_exp_in_fexp e1 x1 (open_fexp_wrt_fexp e3 (fexp_var_f x2)))) (close_fexp_wrt_fexp y1 (subst_exp_in_fexp e1 x1 (open_fexp_wrt_fexp e4 (fexp_var_f y1)))).
 Proof.
 default_simp.
@@ -6346,7 +6346,7 @@ Qed.
 
 Lemma subst_typ_in_ftyp_intro_rec_mutual :
 (forall A1 X1 A2 n1,
-  X1 `notin` fv_ftyp_in_ftyp A1 ->
+  X1 `notin` ftvar_in_ftyp A1 ->
   open_ftyp_wrt_ftyp_rec n1 A2 A1 = subst_typ_in_ftyp A2 X1 (open_ftyp_wrt_ftyp_rec n1 (ftyp_var_f X1) A1)).
 Proof.
 apply_mutual_ind ftyp_mutind;
@@ -6357,7 +6357,7 @@ Qed.
 
 Lemma subst_typ_in_ftyp_intro_rec :
 forall A1 X1 A2 n1,
-  X1 `notin` fv_ftyp_in_ftyp A1 ->
+  X1 `notin` ftvar_in_ftyp A1 ->
   open_ftyp_wrt_ftyp_rec n1 A2 A1 = subst_typ_in_ftyp A2 X1 (open_ftyp_wrt_ftyp_rec n1 (ftyp_var_f X1) A1).
 Proof.
 pose proof subst_typ_in_ftyp_intro_rec_mutual as H; intuition eauto.
@@ -6370,7 +6370,7 @@ Qed.
 
 Lemma subst_typ_in_fexp_intro_rec_mutual :
 (forall e1 X1 A1 n1,
-  X1 `notin` fv_ftyp_in_fexp e1 ->
+  X1 `notin` ftvar_in_fexp e1 ->
   open_fexp_wrt_ftyp_rec n1 A1 e1 = subst_typ_in_fexp A1 X1 (open_fexp_wrt_ftyp_rec n1 (ftyp_var_f X1) e1)).
 Proof.
 apply_mutual_ind fexp_mutind;
@@ -6381,7 +6381,7 @@ Qed.
 
 Lemma subst_typ_in_fexp_intro_rec :
 forall e1 X1 A1 n1,
-  X1 `notin` fv_ftyp_in_fexp e1 ->
+  X1 `notin` ftvar_in_fexp e1 ->
   open_fexp_wrt_ftyp_rec n1 A1 e1 = subst_typ_in_fexp A1 X1 (open_fexp_wrt_ftyp_rec n1 (ftyp_var_f X1) e1).
 Proof.
 pose proof subst_typ_in_fexp_intro_rec_mutual as H; intuition eauto.
@@ -6394,7 +6394,7 @@ Qed.
 
 Lemma subst_exp_in_fexp_intro_rec_mutual :
 (forall e1 x1 e2 n1,
-  x1 `notin` fv_fexp_in_fexp e1 ->
+  x1 `notin` fvar_in_fexp e1 ->
   open_fexp_wrt_fexp_rec n1 e2 e1 = subst_exp_in_fexp e2 x1 (open_fexp_wrt_fexp_rec n1 (fexp_var_f x1) e1)).
 Proof.
 apply_mutual_ind fexp_mutind;
@@ -6405,7 +6405,7 @@ Qed.
 
 Lemma subst_exp_in_fexp_intro_rec :
 forall e1 x1 e2 n1,
-  x1 `notin` fv_fexp_in_fexp e1 ->
+  x1 `notin` fvar_in_fexp e1 ->
   open_fexp_wrt_fexp_rec n1 e2 e1 = subst_exp_in_fexp e2 x1 (open_fexp_wrt_fexp_rec n1 (fexp_var_f x1) e1).
 Proof.
 pose proof subst_exp_in_fexp_intro_rec_mutual as H; intuition eauto.
@@ -6418,7 +6418,7 @@ Qed.
 
 Lemma subst_typ_in_fbind_intro_rec_mutual :
 (forall fb1 X1 A1 n1,
-  X1 `notin` fv_ftyp_in_fbind fb1 ->
+  X1 `notin` ftvar_in_fbind fb1 ->
   open_fbind_wrt_ftyp_rec n1 A1 fb1 = subst_typ_in_fbind A1 X1 (open_fbind_wrt_ftyp_rec n1 (ftyp_var_f X1) fb1)).
 Proof.
 apply_mutual_ind fbind_mutind;
@@ -6429,7 +6429,7 @@ Qed.
 
 Lemma subst_typ_in_fbind_intro_rec :
 forall fb1 X1 A1 n1,
-  X1 `notin` fv_ftyp_in_fbind fb1 ->
+  X1 `notin` ftvar_in_fbind fb1 ->
   open_fbind_wrt_ftyp_rec n1 A1 fb1 = subst_typ_in_fbind A1 X1 (open_fbind_wrt_ftyp_rec n1 (ftyp_var_f X1) fb1).
 Proof.
 pose proof subst_typ_in_fbind_intro_rec_mutual as H; intuition eauto.
@@ -6440,7 +6440,7 @@ Qed.
 
 Lemma subst_typ_in_ftyp_intro :
 forall X1 A1 A2,
-  X1 `notin` fv_ftyp_in_ftyp A1 ->
+  X1 `notin` ftvar_in_ftyp A1 ->
   open_ftyp_wrt_ftyp A1 A2 = subst_typ_in_ftyp A2 X1 (open_ftyp_wrt_ftyp A1 (ftyp_var_f X1)).
 Proof.
 unfold open_ftyp_wrt_ftyp; default_simp.
@@ -6450,7 +6450,7 @@ Qed.
 
 Lemma subst_typ_in_fexp_intro :
 forall X1 e1 A1,
-  X1 `notin` fv_ftyp_in_fexp e1 ->
+  X1 `notin` ftvar_in_fexp e1 ->
   open_fexp_wrt_ftyp e1 A1 = subst_typ_in_fexp A1 X1 (open_fexp_wrt_ftyp e1 (ftyp_var_f X1)).
 Proof.
 unfold open_fexp_wrt_ftyp; default_simp.
@@ -6460,7 +6460,7 @@ Qed.
 
 Lemma subst_exp_in_fexp_intro :
 forall x1 e1 e2,
-  x1 `notin` fv_fexp_in_fexp e1 ->
+  x1 `notin` fvar_in_fexp e1 ->
   open_fexp_wrt_fexp e1 e2 = subst_exp_in_fexp e2 x1 (open_fexp_wrt_fexp e1 (fexp_var_f x1)).
 Proof.
 unfold open_fexp_wrt_fexp; default_simp.
@@ -6470,7 +6470,7 @@ Qed.
 
 Lemma subst_typ_in_fbind_intro :
 forall X1 fb1 A1,
-  X1 `notin` fv_ftyp_in_fbind fb1 ->
+  X1 `notin` ftvar_in_fbind fb1 ->
   open_fbind_wrt_ftyp fb1 A1 = subst_typ_in_fbind A1 X1 (open_fbind_wrt_ftyp fb1 (ftyp_var_f X1)).
 Proof.
 unfold open_fbind_wrt_ftyp; default_simp.
